<?xml version="1.0"?>


<!DOCTYPE rdf:RDF [
    <!ENTITY owl "http://www.w3.org/2002/07/owl#" >
    <!ENTITY xsd "http://www.w3.org/2001/XMLSchema#" >
    <!ENTITY rdfs "http://www.w3.org/2000/01/rdf-schema#" >
    <!ENTITY rdf "http://www.w3.org/1999/02/22-rdf-syntax-ns#" >
    <!ENTITY oboInOwl "http://www.geneontology.org/formats/oboInOwl#" >
    <!ENTITY ero "http://www.cubrc.org/ontologies/KDD/Upper/ExtendedRelationOntology#" >
]>


<rdf:RDF xmlns="http://www.cubrc.org/ontologies/KDD/Mid/EventOntology#"
     xml:base="http://www.cubrc.org/ontologies/KDD/Mid/EventOntology"
     xmlns:rdfs="http://www.w3.org/2000/01/rdf-schema#"
     xmlns:owl="http://www.w3.org/2002/07/owl#"
     xmlns:xsd="http://www.w3.org/2001/XMLSchema#"
     xmlns:rdf="http://www.w3.org/1999/02/22-rdf-syntax-ns#"
     xmlns:oboInOwl="http://www.geneontology.org/formats/oboInOwl#"
     xmlns:ero="http://www.cubrc.org/ontologies/KDD/Upper/ExtendedRelationOntology#">
    <owl:Ontology rdf:about="http://www.cubrc.org/ontologies/KDD/Mid/EventOntology">
        <owl:versionInfo rdf:datatype="&xsd;string">Created with TopBraid Composer</owl:versionInfo>
        <owl:imports rdf:resource="http://www.cubrc.org/ontologies/KDD/Upper/ExtendedRelationOntology"/>
    </owl:Ontology>
    


    <!-- 
    ///////////////////////////////////////////////////////////////////////////////////////
    //
    // Classes
    //
    ///////////////////////////////////////////////////////////////////////////////////////
     -->

    


    <!-- http://www.cubrc.org/ontologies/KDD/Mid/EventOntology#Act -->

    <owl:Class rdf:about="http://www.cubrc.org/ontologies/KDD/Mid/EventOntology#Act">
        <rdfs:label rdf:datatype="&xsd;string">Act</rdfs:label>
        <rdfs:subClassOf rdf:resource="http://www.ifomis.org/bfo/1.1/span#Process"/>
        <rdfs:comment rdf:datatype="&xsd;string">A Process in which at least one Agent plays a causative role.</rdfs:comment>
        <rdfs:comment rdf:datatype="&xsd;string">INCIDENT INCIDENT INCIDENT event happenning</rdfs:comment>
    </owl:Class>
    


    <!-- http://www.cubrc.org/ontologies/KDD/Mid/EventOntology#ActOfAccessoryToACriminalAct -->

    <owl:Class rdf:about="http://www.cubrc.org/ontologies/KDD/Mid/EventOntology#ActOfAccessoryToACriminalAct">
        <rdfs:label>Act Of Accessory To A Criminal Act</rdfs:label>
        <rdfs:subClassOf rdf:resource="http://www.cubrc.org/ontologies/KDD/Mid/EventOntology#CriminalAct"/>
        <rdfs:comment>Definition: A Criminal Act in which a person helps or encourages a criminal in some way, or simply by failing to report the crime to proper authority. The assistance to the criminal may be of any type, including emotional or financial assistance as well as physical assistance or concealment. (derived from http://en.wikipedia.org/wiki/Accessory_(legal_term). Comment: In this case the person realizes the role of Accessory)</rdfs:comment>
    </owl:Class>
    


    <!-- http://www.cubrc.org/ontologies/KDD/Mid/EventOntology#ActOfAcquital -->

    <owl:Class rdf:about="http://www.cubrc.org/ontologies/KDD/Mid/EventOntology#ActOfAcquital">
        <rdfs:label>Act Of Acquital</rdfs:label>
        <rdfs:subClassOf rdf:resource="http://www.cubrc.org/ontologies/KDD/Mid/EventOntology#LegalSystemAct"/>
        <rdfs:comment>Definition: A Legal System Act of issuing a release of a liability of a defendant in a Lawsuit or a judgment of not guilty against a defendant in a Criminal Trial (derived from http://www.id.uscourts.gov/glossary.htm)</rdfs:comment>
    </owl:Class>
    


    <!-- http://www.cubrc.org/ontologies/KDD/Mid/EventOntology#ActOfAdvising -->

    <owl:Class rdf:about="http://www.cubrc.org/ontologies/KDD/Mid/EventOntology#ActOfAdvising">
        <rdfs:label rdf:datatype="&xsd;string">Act Of Advising</rdfs:label>
        <rdfs:subClassOf rdf:resource="http://www.cubrc.org/ontologies/KDD/Mid/EventOntology#ActOfDirectiveCommunication"/>
    </owl:Class>
    


    <!-- http://www.cubrc.org/ontologies/KDD/Mid/EventOntology#ActOfAidingAndAbettingACriminal -->

    <owl:Class rdf:about="http://www.cubrc.org/ontologies/KDD/Mid/EventOntology#ActOfAidingAndAbettingACriminal">
        <rdfs:label>Act Of Aiding And Abetting A Criminal</rdfs:label>
        <rdfs:subClassOf rdf:resource="http://www.cubrc.org/ontologies/KDD/Mid/EventOntology#CriminalAct"/>
        <rdfs:comment>Definition: A Criminal Act in which a person actively participates in the commission of a crime but takes no part in the actual criminal offense, such as being the driver for a bank robbery (derived from http://en.wikipedia.org/wiki/Aid_and_abet) Comment: In this case a person realizes the role of Accomplice.</rdfs:comment>
    </owl:Class>
    


    <!-- http://www.cubrc.org/ontologies/KDD/Mid/EventOntology#ActOfAirAssault -->

    <owl:Class rdf:about="http://www.cubrc.org/ontologies/KDD/Mid/EventOntology#ActOfAirAssault">
        <rdfs:label>Conduct an Air Assault</rdfs:label>
        <rdfs:subClassOf rdf:resource="http://www.cubrc.org/ontologies/KDD/Mid/EventOntology#ActOfAttack"/>
        <rdfs:comment>Definition: An Act of Attack which secures a defendable airhead or other key terrain from which to conduct lodgment activities or follow-on tactical operations (derived from The Army Universal Task List FM 7-15 February 2009).</rdfs:comment>
    </owl:Class>
    


    <!-- http://www.cubrc.org/ontologies/KDD/Mid/EventOntology#ActOfAirToSurfaceFire -->

    <owl:Class rdf:about="http://www.cubrc.org/ontologies/KDD/Mid/EventOntology#ActOfAirToSurfaceFire">
        <rdfs:label>Air to Surface Attack</rdfs:label>
        <rdfs:subClassOf rdf:resource="http://www.cubrc.org/ontologies/KDD/Mid/EventOntology#ActOfIndirectFire"/>
        <rdfs:comment>Definition: An Act of Indirect Fire in which fixed- and rotary-wing aircraft-mounted weapon systems are used to destroy, suppress, or neutralize equipment (including aircraft on the ground), materiel, personnel, fortifications, and facilities (derived from The Army Universal Task List FM 7-15 February 2009).</rdfs:comment>
    </owl:Class>
    


    <!-- http://www.cubrc.org/ontologies/KDD/Mid/EventOntology#ActOfAmphibiousAssault -->

    <owl:Class rdf:about="http://www.cubrc.org/ontologies/KDD/Mid/EventOntology#ActOfAmphibiousAssault">
        <rdfs:label>Conduct an Amphibious Assault</rdfs:label>
        <rdfs:subClassOf rdf:resource="http://www.cubrc.org/ontologies/KDD/Mid/EventOntology#ActOfAttack"/>
        <rdfs:comment>Definition: An Act of Attack which secures a defendable beachhead from which to conduct lodgment activities (derived from The Army Universal Task List FM 7-15 February 2009).</rdfs:comment>
    </owl:Class>
    


    <!-- http://www.cubrc.org/ontologies/KDD/Mid/EventOntology#ActOfAntiTerrorism -->

    <owl:Class rdf:about="http://www.cubrc.org/ontologies/KDD/Mid/EventOntology#ActOfAntiTerrorism">
        <rdfs:label>Apply Anti-Terrorism Measure</rdfs:label>
        <rdfs:subClassOf rdf:resource="http://www.cubrc.org/ontologies/KDD/Mid/EventOntology#ActOfProtectionWarfighting"/>
        <rdfs:comment>Definition: An Act of Protection Warfighting that consists of defensive measures used to reduce the vulnerability of individuals and property to terrorist acts, to include limited response and containment by local military and civilian forces (derived from The Army Universal Task List FM 7-15 February 2009).</rdfs:comment>
    </owl:Class>
    


    <!-- http://www.cubrc.org/ontologies/KDD/Mid/EventOntology#ActOfApologizing -->

    <owl:Class rdf:about="http://www.cubrc.org/ontologies/KDD/Mid/EventOntology#ActOfApologizing">
        <rdfs:label rdf:datatype="&xsd;string">Act Of Apologizing</rdfs:label>
        <rdfs:subClassOf rdf:resource="http://www.cubrc.org/ontologies/KDD/Mid/EventOntology#ActOfExpressiveCommunication"/>
    </owl:Class>
    


    <!-- http://www.cubrc.org/ontologies/KDD/Mid/EventOntology#ActOfApproachMarch -->

    <owl:Class rdf:about="http://www.cubrc.org/ontologies/KDD/Mid/EventOntology#ActOfApproachMarch">
        <rdfs:label>Approach March</rdfs:label>
        <rdfs:subClassOf rdf:resource="http://www.cubrc.org/ontologies/KDD/Mid/EventOntology#ActOfForceMovement"/>
        <rdfs:comment>Definition: An Act of Force Movement in which a combat unit advances with the objective of direct contact with the enemy and ends with the unit being located in an attack position, assembly area, or assault position; or it transitions to an attack (derived from The Army Universal Task List FM 7-15 February 2009).</rdfs:comment>
    </owl:Class>
    


    <!-- http://www.cubrc.org/ontologies/KDD/Mid/EventOntology#ActOfAreaClearance -->

    <owl:Class rdf:about="http://www.cubrc.org/ontologies/KDD/Mid/EventOntology#ActOfAreaClearance">
        <rdfs:label>Conduct Area Clearance</rdfs:label>
        <rdfs:subClassOf rdf:resource="http://www.cubrc.org/ontologies/KDD/Mid/EventOntology#ActOfClearing"/>
        <rdfs:comment>Definition: An Act of Clearance wherein the total elimination or neutralization of an obstacle or portions of an obstacle in a designated area occurs (derived from The Army Universal Task List FM 7-15 February 2009).</rdfs:comment>
    </owl:Class>
    


    <!-- http://www.cubrc.org/ontologies/KDD/Mid/EventOntology#ActOfAreaOccupation -->

    <owl:Class rdf:about="http://www.cubrc.org/ontologies/KDD/Mid/EventOntology#ActOfAreaOccupation">
        <rdfs:label>Occupy an Area</rdfs:label>
        <rdfs:subClassOf rdf:resource="http://www.cubrc.org/ontologies/KDD/Mid/EventOntology#ActOfMovementAndManeuverWarfighting"/>
        <rdfs:comment>Definition: An Act of Military Force in which some Force moves into and secures an area from which to conduct future operations (derived from The Army Universal Task List FM 7-15 February 2009).</rdfs:comment>
    </owl:Class>
    


    <!-- http://www.cubrc.org/ontologies/KDD/Mid/EventOntology#ActOfAreaReconnaissance -->

    <owl:Class rdf:about="http://www.cubrc.org/ontologies/KDD/Mid/EventOntology#ActOfAreaReconnaissance">
        <rdfs:label>Conduct an Area Reconnaissance</rdfs:label>
        <rdfs:subClassOf rdf:resource="http://www.cubrc.org/ontologies/KDD/Mid/EventOntology#ActOfReconnaissance"/>
        <rdfs:comment>Definition: An Act of Reconnaissance in which a directed effort is made to obtain detailed information concerning the terrain or enemy activity within a prescribed area not defined by boundaries, such as a town, ridgeline, woods, or other feature critical to operations to include underwater reconnaissance, search, or recovery (derived from The Army Universal Task List FM 7-15 February 2009).</rdfs:comment>
    </owl:Class>
    


    <!-- http://www.cubrc.org/ontologies/KDD/Mid/EventOntology#ActOfArmsSmuggling -->

    <owl:Class rdf:about="http://www.cubrc.org/ontologies/KDD/Mid/EventOntology#ActOfArmsSmuggling">
        <rdfs:subClassOf rdf:resource="http://www.cubrc.org/ontologies/KDD/Mid/EventOntology#ActOfSmuggling"/>
        <rdfs:comment rdf:datatype="&xsd;string">Definition: An Act of Smuggling of firearms across borders (Source: http://www.ice.gov/firearms-explosives-smuggling/)</rdfs:comment>
    </owl:Class>
    


    <!-- http://www.cubrc.org/ontologies/KDD/Mid/EventOntology#ActOfArmsTrafficking -->

    <owl:Class rdf:about="http://www.cubrc.org/ontologies/KDD/Mid/EventOntology#ActOfArmsTrafficking">
        <rdfs:label>Act Of Arms Trafficking</rdfs:label>
        <rdfs:subClassOf rdf:resource="http://www.cubrc.org/ontologies/KDD/Mid/EventOntology#ActOfBlackMarketTrafficking"/>
        <rdfs:comment>Definition: An Act of Black Market Trafficking  involving the illegal distribution and sale of contraband weapons or ammunition. (derived from http://en.wikipedia.org/wiki/Arms_trafficking).</rdfs:comment>
    </owl:Class>
    


    <!-- http://www.cubrc.org/ontologies/KDD/Mid/EventOntology#ActOfArraignment -->

    <owl:Class rdf:about="http://www.cubrc.org/ontologies/KDD/Mid/EventOntology#ActOfArraignment">
        <rdfs:label>Act Of Arraignment</rdfs:label>
        <rdfs:subClassOf rdf:resource="http://www.cubrc.org/ontologies/KDD/Mid/EventOntology#Hearing"/>
        <rdfs:comment>Definition: A Hearing at which the person accused of having violated criminal law is brought before the court to plead to the criminal charge in the indictment (derived from http://www.id.uscourts.gov/glossary.htm)</rdfs:comment>
    </owl:Class>
    


    <!-- http://www.cubrc.org/ontologies/KDD/Mid/EventOntology#ActOfArson -->

    <owl:Class rdf:about="http://www.cubrc.org/ontologies/KDD/Mid/EventOntology#ActOfArson">
        <rdfs:label>Act Of Arson</rdfs:label>
        <rdfs:subClassOf rdf:resource="http://www.cubrc.org/ontologies/KDD/Mid/EventOntology#CriminalActAgainstProperty"/>
        <rdfs:comment>Definition: A Criminal Act Against Property of maliciously setting fire to the property of another or of burning ones own property for an improper purpose, as to collect insurance. (derived from JC3IEDM-MIRD-DMWG-Edition_3.0.2_20090514).</rdfs:comment>
    </owl:Class>
    


    <!-- http://www.cubrc.org/ontologies/KDD/Mid/EventOntology#ActOfArtifactEmployment -->

    <owl:Class rdf:about="http://www.cubrc.org/ontologies/KDD/Mid/EventOntology#ActOfArtifactEmployment">
        <rdfs:label rdf:datatype="&xsd;string">Act Of Artifact Employment</rdfs:label>
        <rdfs:subClassOf rdf:resource="http://www.cubrc.org/ontologies/KDD/Mid/EventOntology#IntentionalAct"/>
        <rdfs:comment rdf:datatype="&xsd;string">An Intentional Act of using an Artifact</rdfs:comment>
    </owl:Class>
    


    <!-- http://www.cubrc.org/ontologies/KDD/Mid/EventOntology#ActOfAssassination -->

    <owl:Class rdf:about="http://www.cubrc.org/ontologies/KDD/Mid/EventOntology#ActOfAssassination">
        <rdfs:label rdf:datatype="&xsd;string">Act Of Assassination</rdfs:label>
        <rdfs:subClassOf rdf:resource="http://www.cubrc.org/ontologies/KDD/Mid/EventOntology#ActOfMurder"/>
        <rdfs:comment rdf:datatype="&xsd;string">Definition: An Act of Murder of a prominent person (derived from JC3IEDM-MIRD-DMWG-Edition_3.0.2_20090514)</rdfs:comment>
    </owl:Class>
    


    <!-- http://www.cubrc.org/ontologies/KDD/Mid/EventOntology#ActOfAssault -->

    <owl:Class rdf:about="http://www.cubrc.org/ontologies/KDD/Mid/EventOntology#ActOfAssault">
        <rdfs:label>Act Of Assault</rdfs:label>
        <rdfs:subClassOf rdf:resource="http://www.cubrc.org/ontologies/KDD/Mid/EventOntology#CriminalActAgainstThePerson"/>
        <rdfs:comment>Definition: A Criminal Act Against the Person involving the an act of violence against another person or involving the threat of violence caused by an immediate show of force. (derived from http://en.wikipedia.org/wiki/Assault)</rdfs:comment>
    </owl:Class>
    


    <!-- http://www.cubrc.org/ontologies/KDD/Mid/EventOntology#ActOfAssociation -->

    <owl:Class rdf:about="http://www.cubrc.org/ontologies/KDD/Mid/EventOntology#ActOfAssociation">
        <rdfs:label rdf:datatype="&xsd;string">Act of Association</rdfs:label>
        <rdfs:subClassOf rdf:resource="http://www.cubrc.org/ontologies/KDD/Mid/EventOntology#SocialAct"/>
        <rdfs:comment rdf:datatype="&xsd;string">Definition: A Social Act wherein an Agent unites with some other Agent in an Intentional Act, enterprise or business. (derived from http://en.wiktionary.org/wiki/associate)</rdfs:comment>
    </owl:Class>
    


    <!-- http://www.cubrc.org/ontologies/KDD/Mid/EventOntology#ActOfAttack -->

    <owl:Class rdf:about="http://www.cubrc.org/ontologies/KDD/Mid/EventOntology#ActOfAttack">
        <rdfs:label>Conduct an Attack</rdfs:label>
        <rdfs:subClassOf rdf:resource="http://www.cubrc.org/ontologies/KDD/Mid/EventOntology#ActOfOffensiveOperation"/>
        <rdfs:comment>Definition: An Act of Offensive Operation that destroys or defeats enemy forces, seizes and secures terrain, or both. Attacks incorporate coordinated movement supported by direct and indirect fires. They may be either decisive or shaping operations. Attacks may be hasty or deliberate, depending on the time available for assessing the situation, planning, and preparing (derived from The Army Universal Task List FM 7-15 February 2009).</rdfs:comment>
    </owl:Class>
    


    <!-- http://www.cubrc.org/ontologies/KDD/Mid/EventOntology#ActOfAttempt -->

    <owl:Class rdf:about="http://www.cubrc.org/ontologies/KDD/Mid/EventOntology#ActOfAttempt">
        <rdfs:label>Act Of Attempt</rdfs:label>
        <rdfs:subClassOf rdf:resource="http://www.cubrc.org/ontologies/KDD/Mid/EventOntology#InchoateCriminalAct"/>
        <rdfs:comment>Definition: An Inchoate Criminal Act in which the Agent has failed to commit the full offense, but has the direct and specific intent to commit that full offense. (derived from http://en.wikipedia.org/wiki/Attempt_(crime))</rdfs:comment>
    </owl:Class>
    


    <!-- http://www.cubrc.org/ontologies/KDD/Mid/EventOntology#ActOfAttemptedAssassination -->

    <owl:Class rdf:about="http://www.cubrc.org/ontologies/KDD/Mid/EventOntology#ActOfAttemptedAssassination">
        <rdfs:label>Act Of Attempted Assassination</rdfs:label>
        <rdfs:subClassOf rdf:resource="http://www.cubrc.org/ontologies/KDD/Mid/EventOntology#ActOfAttemptedMurder"/>
        <rdfs:comment>Definition: An Act Of Attempted Murder of a prominent Person (derived from JC3IEDM-MIRD-DMWG-Edition_3.0.2_20090514)</rdfs:comment>
    </owl:Class>
    


    <!-- http://www.cubrc.org/ontologies/KDD/Mid/EventOntology#ActOfAttemptedMurder -->

    <owl:Class rdf:about="http://www.cubrc.org/ontologies/KDD/Mid/EventOntology#ActOfAttemptedMurder">
        <rdfs:label>Act Of Attempted Murder</rdfs:label>
        <rdfs:subClassOf rdf:resource="http://www.cubrc.org/ontologies/KDD/Mid/EventOntology#ActOfAttempt"/>
        <rdfs:comment>Definition: An Act Of Attempt of unlawfully killing of one human being by another, especially with premeditated malice. (derived from JC3IEDM-MIRD-DMWG_Edition_3.0.2_20090514)</rdfs:comment>
    </owl:Class>
    


    <!-- http://www.cubrc.org/ontologies/KDD/Mid/EventOntology#ActOfAttemptedRape -->

    <owl:Class rdf:about="http://www.cubrc.org/ontologies/KDD/Mid/EventOntology#ActOfAttemptedRape">
        <rdfs:label>Act Of Attempted Rape</rdfs:label>
        <rdfs:subClassOf rdf:resource="http://www.cubrc.org/ontologies/KDD/Mid/EventOntology#ActOfAttempt"/>
        <rdfs:comment>Definition: An Act Of Attempt of forcing another person to submit to sexual intercourse. (derived from JC3IEDM-MIRD-DMWG-Edition_3.0.2_20090514)</rdfs:comment>
    </owl:Class>
    


    <!-- http://www.cubrc.org/ontologies/KDD/Mid/EventOntology#ActOfAttemptedRobbery -->

    <owl:Class rdf:about="http://www.cubrc.org/ontologies/KDD/Mid/EventOntology#ActOfAttemptedRobbery">
        <rdfs:label>Act Of Attempted Robbery</rdfs:label>
        <rdfs:subClassOf rdf:resource="http://www.cubrc.org/ontologies/KDD/Mid/EventOntology#ActOfAttempt"/>
        <rdfs:comment>Definition: An Act Of Attempt of robbing a person or place. (derived from JC3IEDM-MIRD-DMWG-Edition_3.0.2_20090514)</rdfs:comment>
    </owl:Class>
    


    <!-- http://www.cubrc.org/ontologies/KDD/Mid/EventOntology#ActOfAttemptedSuicide -->

    <owl:Class rdf:about="http://www.cubrc.org/ontologies/KDD/Mid/EventOntology#ActOfAttemptedSuicide">
        <rdfs:label>Act Of Attempted Suicide</rdfs:label>
        <rdfs:subClassOf rdf:resource="http://www.cubrc.org/ontologies/KDD/Mid/EventOntology#ActOfAttempt"/>
        <rdfs:comment>Definition: An Act Of Attempt of killing oneself intentionally. (derived from JC3IEDM-MIRD-DMWG-Edition_3.0.2_20090514)</rdfs:comment>
    </owl:Class>
    


    <!-- http://www.cubrc.org/ontologies/KDD/Mid/EventOntology#ActOfBattery -->

    <owl:Class rdf:about="http://www.cubrc.org/ontologies/KDD/Mid/EventOntology#ActOfBattery">
        <rdfs:label>Act Of Battery</rdfs:label>
        <rdfs:subClassOf rdf:resource="http://www.cubrc.org/ontologies/KDD/Mid/EventOntology#CriminalActAgainstThePerson"/>
        <rdfs:comment>Definition: A Criminal Act Against the Person involving the use of force against another, resulting in harmful or offensive contact, different from an Act of Assault in that the contact need not be violent (derived from http://en.wikipedia.org/wiki/Battery)</rdfs:comment>
    </owl:Class>
    


    <!-- http://www.cubrc.org/ontologies/KDD/Mid/EventOntology#ActOfBlackMarketTrafficking -->

    <owl:Class rdf:about="http://www.cubrc.org/ontologies/KDD/Mid/EventOntology#ActOfBlackMarketTrafficking">
        <rdfs:label>Act Of Black Market Trafficking</rdfs:label>
        <rdfs:subClassOf rdf:resource="http://www.cubrc.org/ontologies/KDD/Mid/EventOntology#CriminalAct"/>
        <rdfs:comment>Definition: A Criminal Act of trading of goods and services that is not part of the official economy of a country. This may be trade of legal goods and services where taxes are not paid or trade of illegal goods and services. (derived from http://en.wikipedia.org/wiki/Black_market)</rdfs:comment>
    </owl:Class>
    


    <!-- http://www.cubrc.org/ontologies/KDD/Mid/EventOntology#ActOfBlackmail -->

    <owl:Class rdf:about="http://www.cubrc.org/ontologies/KDD/Mid/EventOntology#ActOfBlackmail">
        <rdfs:label>Act Of Blackmail</rdfs:label>
        <rdfs:subClassOf rdf:resource="http://www.cubrc.org/ontologies/KDD/Mid/EventOntology#CriminalActAgainstProperty"/>
        <rdfs:comment>Definition: A Criminal Act Against Property of threatening to reveal substantially true information about a person to the public, a family member, or associates unless some demand is met. (derived from http://en.wikipedia.org/wiki/Blackmail)</rdfs:comment>
    </owl:Class>
    


    <!-- http://www.cubrc.org/ontologies/KDD/Mid/EventOntology#ActOfBooking -->

    <owl:Class rdf:about="http://www.cubrc.org/ontologies/KDD/Mid/EventOntology#ActOfBooking">
        <rdfs:label>Act Of Booking</rdfs:label>
        <rdfs:subClassOf rdf:resource="http://www.cubrc.org/ontologies/KDD/Mid/EventOntology#LegalSystemAct"/>
        <rdfs:comment>Definition: A Legal System Act of photographing, fingerprinting and recording identifying data of a suspect. (derived from http://www.id.uscourts.gov/glossary.htm)</rdfs:comment>
    </owl:Class>
    


    <!-- http://www.cubrc.org/ontologies/KDD/Mid/EventOntology#ActOfBreaching -->

    <owl:Class rdf:about="http://www.cubrc.org/ontologies/KDD/Mid/EventOntology#ActOfBreaching">
        <rdfs:label>Breaching Operation</rdfs:label>
        <rdfs:subClassOf rdf:resource="http://www.cubrc.org/ontologies/KDD/Mid/EventOntology#ActOfMobilityOperation"/>
        <rdfs:comment>Definition: An Act of Military Force conducted as a combined arms operation with the objective of projecting combat power to the far side of an obstacle and is accomplished by the creation of lanes through or over an obstacle to allow an attacking force to pass rapidly (derived from The Army Universal Task List FM 7-15 February 2009).</rdfs:comment>
    </owl:Class>
    


    <!-- http://www.cubrc.org/ontologies/KDD/Mid/EventOntology#ActOfBribery -->

    <owl:Class rdf:about="http://www.cubrc.org/ontologies/KDD/Mid/EventOntology#ActOfBribery">
        <rdfs:subClassOf rdf:resource="http://www.cubrc.org/ontologies/KDD/Mid/EventOntology#CriminalActAgainstJustice"/>
        <rdfs:comment rdf:datatype="&xsd;string">Definition: A Criminal Act Against Justice in which some item of value is offered, given, received, or solicited in order to influence the actions of an official or other person in charge of a public or legal duty. (Source: http://en.wikipedia.org/wiki/Bribery)</rdfs:comment>
    </owl:Class>
    


    <!-- http://www.cubrc.org/ontologies/KDD/Mid/EventOntology#ActOfBulkCashSmuggling -->

    <owl:Class rdf:about="http://www.cubrc.org/ontologies/KDD/Mid/EventOntology#ActOfBulkCashSmuggling">
        <rdfs:subClassOf rdf:resource="http://www.cubrc.org/ontologies/KDD/Mid/EventOntology#ActOfSmuggling"/>
        <rdfs:comment rdf:datatype="&xsd;string">Definition: An Act of Smuggling that is a reporting offense in which, with the intent to evade a currency reporting requirement, an agent knowingly conceals a significant amount of money in currency or other monetary instruments on the person of such individual or in any conveyance, article of luggage, merchandise, or other container, and transports or transfers or attempts to transport or transfer such currency or monetary instruments from one location to another (Source: http://www.ice.gov/bulk-cash-smuggling-center/faq/)</rdfs:comment>
    </owl:Class>
    


    <!-- http://www.cubrc.org/ontologies/KDD/Mid/EventOntology#ActOfBurglary -->

    <owl:Class rdf:about="http://www.cubrc.org/ontologies/KDD/Mid/EventOntology#ActOfBurglary">
        <rdfs:label>Act Of Burglary</rdfs:label>
        <rdfs:subClassOf rdf:resource="http://www.cubrc.org/ontologies/KDD/Mid/EventOntology#InchoateCriminalAct"/>
        <rdfs:comment>Definition: An Inchoate Criminal Act of entry into a building for the purposes of committing an offense. (derived from http://en.wikipedia.org/wiki/Burglary). Comment: Also known as Breaking and Entering.</rdfs:comment>
    </owl:Class>
    


    <!-- http://www.cubrc.org/ontologies/KDD/Mid/EventOntology#ActOfCargoTransportation -->

    <owl:Class rdf:about="http://www.cubrc.org/ontologies/KDD/Mid/EventOntology#ActOfCargoTransportation">
        <rdfs:label xml:lang="en">ActOfTransportation</rdfs:label>
        <rdfs:subClassOf rdf:resource="http://www.cubrc.org/ontologies/KDD/Mid/EventOntology#ActOfMovement"/>
    </owl:Class>
    


    <!-- http://www.cubrc.org/ontologies/KDD/Mid/EventOntology#ActOfCeremony -->

    <owl:Class rdf:about="http://www.cubrc.org/ontologies/KDD/Mid/EventOntology#ActOfCeremony">
        <rdfs:label>Act Of Ceremony</rdfs:label>
        <rdfs:subClassOf rdf:resource="http://www.cubrc.org/ontologies/KDD/Mid/EventOntology#SocialAct"/>
        <rdfs:comment>Definition: A Social Act of ritual significance, performed on a special occasion. (derived from http://en.wikipedia.org/wiki/Ceremony)</rdfs:comment>
    </owl:Class>
    


    <!-- http://www.cubrc.org/ontologies/KDD/Mid/EventOntology#ActOfChangeOfResidence -->

    <owl:Class rdf:about="http://www.cubrc.org/ontologies/KDD/Mid/EventOntology#ActOfChangeOfResidence">
        <rdfs:label rdf:datatype="&xsd;string">Act Of Change Of Residence</rdfs:label>
        <rdfs:subClassOf rdf:resource="http://www.cubrc.org/ontologies/KDD/Mid/EventOntology#ActOfMovement"/>
        <rdfs:comment rdf:datatype="&xsd;string">Definition: An Act of Movement involving Persons moving from one place of residence to another.</rdfs:comment>
    </owl:Class>
    


    <!-- http://www.cubrc.org/ontologies/KDD/Mid/EventOntology#ActOfChangeOfVenue -->

    <owl:Class rdf:about="http://www.cubrc.org/ontologies/KDD/Mid/EventOntology#ActOfChangeOfVenue">
        <rdfs:label>Act Of Change Of Venue</rdfs:label>
        <rdfs:subClassOf rdf:resource="http://www.cubrc.org/ontologies/KDD/Mid/EventOntology#LegalSystemAct"/>
        <rdfs:comment>Definition: A Legal System Act of moving a Criminal Trial or Lawsuit to another location. (derived from http://www.id.uscourts.gov/glossary.htm)</rdfs:comment>
    </owl:Class>
    


    <!-- http://www.cubrc.org/ontologies/KDD/Mid/EventOntology#ActOfCivilAffairs -->

    <owl:Class rdf:about="http://www.cubrc.org/ontologies/KDD/Mid/EventOntology#ActOfCivilAffairs">
        <rdfs:label>Civil Affairs Operation</rdfs:label>
        <rdfs:subClassOf rdf:resource="http://www.cubrc.org/ontologies/KDD/Mid/EventOntology#ActOfCivilMilitaryOperation"/>
        <rdfs:comment>Definition: An Act of Civil Military Operation that includes instances of any of the following types of action: public legal support, economic and commerce support, infrastructure support, government support, public health and welfare support, and public education and information support (derived from The Army Universal Task List FM 7-15 February 2009).</rdfs:comment>
    </owl:Class>
    


    <!-- http://www.cubrc.org/ontologies/KDD/Mid/EventOntology#ActOfCivilDisorder -->

    <owl:Class rdf:about="http://www.cubrc.org/ontologies/KDD/Mid/EventOntology#ActOfCivilDisorder">
        <rdfs:label rdf:datatype="&xsd;string">Act of civil disorder</rdfs:label>
        <rdfs:subClassOf rdf:resource="http://www.cubrc.org/ontologies/KDD/Mid/EventOntology#CriminalAct"/>
        <rdfs:comment rdf:datatype="&xsd;string">Definition: A Criminal Act consisting of a public disturbance involving acts of violence by assemblages of three or more persons, which causes an immediate danger of or results in damage or injury to the property or person of any other individual. </rdfs:comment>
    </owl:Class>
    


    <!-- http://www.cubrc.org/ontologies/KDD/Mid/EventOntology#ActOfCivilMilitaryOperation -->

    <owl:Class rdf:about="http://www.cubrc.org/ontologies/KDD/Mid/EventOntology#ActOfCivilMilitaryOperation">
        <rdfs:label>Conduct Civil Military Operations</rdfs:label>
        <rdfs:subClassOf rdf:resource="http://www.cubrc.org/ontologies/KDD/Mid/EventOntology#ActOfCommandAndControlWarfighting"/>
        <rdfs:comment>Definition: An Act of Command and Control Warfighting in which a commander establishes, maintains, influences, or exploits relations between military forces, governmental and nongovernmental civilian organizations and authorities, and the civilian populace in a friendly, neutral, or hostile operational area in order to facilitate military operations to consolidate and achieve U.S. objectives (derived from The Army Universal Task List FM 7-15 February 2009).</rdfs:comment>
    </owl:Class>
    


    <!-- http://www.cubrc.org/ontologies/KDD/Mid/EventOntology#ActOfCivilSupportOperation -->

    <owl:Class rdf:about="http://www.cubrc.org/ontologies/KDD/Mid/EventOntology#ActOfCivilSupportOperation">
        <rdfs:label>Conduct Civil Support Operation</rdfs:label>
        <rdfs:subClassOf rdf:resource="http://www.cubrc.org/ontologies/KDD/Mid/EventOntology#ActOfMilitaryForce"/>
        <rdfs:comment>Definition: An Act of Military Force in which Department of Defense support is provided to U.S. civil authorities for domestic emergencies, and for designated law enforcement and other activities. Civil support includes operations that address the consequences of natural or man-made disasters, accidents, and incidents within the United States and its territories (derived from The Army Universal Task List FM 7-15 February 2009).</rdfs:comment>
    </owl:Class>
    


    <!-- http://www.cubrc.org/ontologies/KDD/Mid/EventOntology#ActOfClearing -->

    <owl:Class rdf:about="http://www.cubrc.org/ontologies/KDD/Mid/EventOntology#ActOfClearing">
        <rdfs:label>Clearing Operation</rdfs:label>
        <rdfs:subClassOf rdf:resource="http://www.cubrc.org/ontologies/KDD/Mid/EventOntology#ActOfMobilityOperation"/>
        <rdfs:comment>Definition: An Act of Military Force conducted to enable the use of a designated area or route by the total elimination or neutralization of an obstacle (to include explosives hazard) or portions of an obstacle  (derived from The Army Universal Task List FM 7-15 February 2009).</rdfs:comment>
    </owl:Class>
    


    <!-- http://www.cubrc.org/ontologies/KDD/Mid/EventOntology#ActOfCombatPatrol -->

    <owl:Class rdf:about="http://www.cubrc.org/ontologies/KDD/Mid/EventOntology#ActOfCombatPatrol">
        <rdfs:label>Combat Patrol</rdfs:label>
        <rdfs:subClassOf rdf:resource="http://www.cubrc.org/ontologies/KDD/Mid/EventOntology#ActOfForceManeuver"/>
        <rdfs:comment>Definition: An Act of Force Maneuver in which ground and air detachments provide security and harass, destroy, or capture enemy troops, equipment, or installations (derived from The Army Universal Task List FM 7-15 February 2009).</rdfs:comment>
    </owl:Class>
    


    <!-- http://www.cubrc.org/ontologies/KDD/Mid/EventOntology#ActOfCommandAndControlWarfare -->

    <owl:Class rdf:about="http://www.cubrc.org/ontologies/KDD/Mid/EventOntology#ActOfCommandAndControlWarfare">
        <rdfs:label>Integrated Command and Control Warfare</rdfs:label>
        <rdfs:subClassOf rdf:resource="http://www.cubrc.org/ontologies/KDD/Mid/EventOntology#ActOfFiresWarfighting"/>
        <rdfs:comment>Definition: An Act of Fires Warfighting that is the integrated use of physical attack, electronic warfare, and computer network operations, supported by intelligence, to degrade, destroy, and exploit an enemy�s or adversary�s command and control system or to deny information to it (derived from The Army Universal Task List FM 7-15 February 2009).</rdfs:comment>
    </owl:Class>
    


    <!-- http://www.cubrc.org/ontologies/KDD/Mid/EventOntology#ActOfCommandAndControlWarfighting -->

    <owl:Class rdf:about="http://www.cubrc.org/ontologies/KDD/Mid/EventOntology#ActOfCommandAndControlWarfighting">
        <rdfs:label>Realize the Command and Control Warfighting Function</rdfs:label>
        <rdfs:subClassOf rdf:resource="http://www.cubrc.org/ontologies/KDD/Mid/EventOntology#ActOfMilitaryForce"/>
        <rdfs:comment>Definition: An Act of Military Force is a task that supports a commander in exercising authority and direction. It includes those tasks associated with acquiring friendly information, managing relevant information, and directing and leading subordinates (derived from The Army Universal Task List FM 7-15 February 2009).</rdfs:comment>
    </owl:Class>
    


    <!-- http://www.cubrc.org/ontologies/KDD/Mid/EventOntology#ActOfCommandPostOperation -->

    <owl:Class rdf:about="http://www.cubrc.org/ontologies/KDD/Mid/EventOntology#ActOfCommandPostOperation">
        <rdfs:label>Conduct Command Post Operation</rdfs:label>
        <rdfs:subClassOf rdf:resource="http://www.cubrc.org/ontologies/KDD/Mid/EventOntology#ActOfCommandAndControlWarfighting"/>
        <rdfs:comment>Definition: An Act of Command and Control Warfighting during which the principal facility used by the commander to exercise command and control of tactical operations is organized, created or erected, operated, and/or moved (derived from The Army Universal Task List FM 7-15 February 2009).</rdfs:comment>
    </owl:Class>
    


    <!-- http://www.cubrc.org/ontologies/KDD/Mid/EventOntology#ActOfCommandProgramExecution -->

    <owl:Class rdf:about="http://www.cubrc.org/ontologies/KDD/Mid/EventOntology#ActOfCommandProgramExecution">
        <rdfs:label>Execute Command Programs</rdfs:label>
        <rdfs:subClassOf rdf:resource="http://www.cubrc.org/ontologies/KDD/Mid/EventOntology#ActOfCommandAndControlWarfighting"/>
        <rdfs:comment>Definition: An Act of Command and Control Warfighting is a performance of a task required by U.S. Code and Army regulations including: support commander�s leadership responsibilities for morale, welfare, and discipline; preserve historical documentation and artifacts; train subordinates and units; and develop a command environmental program. (derived from The Army Universal Task List FM 7-15 February 2009).</rdfs:comment>
    </owl:Class>
    


    <!-- http://www.cubrc.org/ontologies/KDD/Mid/EventOntology#ActOfCommanding -->

    <owl:Class rdf:about="http://www.cubrc.org/ontologies/KDD/Mid/EventOntology#ActOfCommanding">
        <rdfs:label rdf:datatype="&xsd;string">Act of Commanding</rdfs:label>
        <rdfs:subClassOf rdf:resource="http://www.cubrc.org/ontologies/KDD/Mid/EventOntology#ActOfDirectiveCommunication"/>
    </owl:Class>
    


    <!-- http://www.cubrc.org/ontologies/KDD/Mid/EventOntology#ActOfCommissiveCommunication -->

    <owl:Class rdf:about="http://www.cubrc.org/ontologies/KDD/Mid/EventOntology#ActOfCommissiveCommunication">
        <rdfs:label rdf:datatype="&xsd;string">Act Of Commissive Communication</rdfs:label>
        <rdfs:subClassOf rdf:resource="http://www.cubrc.org/ontologies/KDD/Mid/EventOntology#ActOfPersonalCommunication"/>
        <rdfs:comment rdf:datatype="&xsd;string">Definition: An Act Of Personal Communication that commits a speaker to some future action. (loosely derived from John Searle&apos;s Speech Acts: An Essay in the Philosophy of Language)</rdfs:comment>
        <rdfs:comment rdf:datatype="&xsd;string">Examples: agreeing, betting, guaranteeing, inviting, offering, promising, swearing, volunteering</rdfs:comment>
    </owl:Class>
    


    <!-- http://www.cubrc.org/ontologies/KDD/Mid/EventOntology#ActOfCommunication -->

    <owl:Class rdf:about="http://www.cubrc.org/ontologies/KDD/Mid/EventOntology#ActOfCommunication">
        <rdfs:label>Act Of Communication</rdfs:label>
        <rdfs:subClassOf rdf:resource="http://www.cubrc.org/ontologies/KDD/Mid/EventOntology#IntentionalAct"/>
        <rdfs:comment>Definition: An Intentional Act in which some Information Content Entity is transferred from some Agent to Another (derived from http://en.wikipedia.org/wiki/Communication)</rdfs:comment>
    </owl:Class>
    


    <!-- http://www.cubrc.org/ontologies/KDD/Mid/EventOntology#ActOfCommunicationByMedia -->

    <owl:Class rdf:about="http://www.cubrc.org/ontologies/KDD/Mid/EventOntology#ActOfCommunicationByMedia">
        <rdfs:label rdf:datatype="&xsd;string">Act Of Communication by Media</rdfs:label>
        <rdfs:subClassOf rdf:resource="http://www.cubrc.org/ontologies/KDD/Mid/EventOntology#ActOfCommunication"/>
    </owl:Class>
    


    <!-- http://www.cubrc.org/ontologies/KDD/Mid/EventOntology#ActOfCommutation -->

    <owl:Class rdf:about="http://www.cubrc.org/ontologies/KDD/Mid/EventOntology#ActOfCommutation">
        <rdfs:label>Act Of Commutation</rdfs:label>
        <rdfs:subClassOf rdf:resource="http://www.cubrc.org/ontologies/KDD/Mid/EventOntology#LegalSystemAct"/>
        <rdfs:comment>Definition: A Legal System Act of reducing a sentence, as for example, from death to life imprisonment (derived from http://www.id.uscourts.gov/glossary.htm)</rdfs:comment>
    </owl:Class>
    


    <!-- http://www.cubrc.org/ontologies/KDD/Mid/EventOntology#ActOfCondoling -->

    <owl:Class rdf:about="http://www.cubrc.org/ontologies/KDD/Mid/EventOntology#ActOfCondoling">
        <rdfs:label rdf:datatype="&xsd;string">Act Of Condoling</rdfs:label>
        <rdfs:subClassOf rdf:resource="http://www.cubrc.org/ontologies/KDD/Mid/EventOntology#ActOfExpressiveCommunication"/>
    </owl:Class>
    


    <!-- http://www.cubrc.org/ontologies/KDD/Mid/EventOntology#ActOfConductingImprovisedExplosiveDefeatOperation -->

    <owl:Class rdf:about="http://www.cubrc.org/ontologies/KDD/Mid/EventOntology#ActOfConductingImprovisedExplosiveDefeatOperation">
        <rdfs:label>Conduct Improvised Explosive Defeat Operation</rdfs:label>
        <rdfs:subClassOf rdf:resource="http://www.cubrc.org/ontologies/KDD/Mid/EventOntology#ActOfSurvivabilityOperation"/>
        <rdfs:comment>Definition: An Act of Survivability Operation in which improvised explosive device (IED) defeat operations are performed to defeat asymmetric attacks against U.S. forces (derived from The Army Universal Task List FM 7-15 February 2009).</rdfs:comment>
    </owl:Class>
    


    <!-- http://www.cubrc.org/ontologies/KDD/Mid/EventOntology#ActOfConductingMassMediaInterview -->

    <owl:Class rdf:about="http://www.cubrc.org/ontologies/KDD/Mid/EventOntology#ActOfConductingMassMediaInterview">
        <rdfs:label>Act Of Conducting Mass Media Interview</rdfs:label>
        <rdfs:subClassOf rdf:resource="http://www.cubrc.org/ontologies/KDD/Mid/EventOntology#ActOfMassMediaCommunication"/>
        <rdfs:comment>Definition: An Act Of Mass Media Communication involving a conversation between a reporter and a person of public interest, used as a basis of a broadcast or publication. (derived from JC3IEDM-MIRD-DMWG-Edition_3.0.2_20090514)</rdfs:comment>
    </owl:Class>
    


    <!-- http://www.cubrc.org/ontologies/KDD/Mid/EventOntology#ActOfConfession -->

    <owl:Class rdf:about="http://www.cubrc.org/ontologies/KDD/Mid/EventOntology#ActOfConfession">
        <rdfs:label rdf:datatype="&xsd;string">Act of Confession</rdfs:label>
        <rdfs:subClassOf rdf:resource="http://www.cubrc.org/ontologies/KDD/Mid/EventOntology#ActOfRepresentativeCommunication"/>
        <rdfs:comment rdf:datatype="&xsd;string">Definition: An Act of Representative Communication in which a person makes an admission of misdeeds or faults.</rdfs:comment>
    </owl:Class>
    


    <!-- http://www.cubrc.org/ontologies/KDD/Mid/EventOntology#ActOfCongratulating -->

    <owl:Class rdf:about="http://www.cubrc.org/ontologies/KDD/Mid/EventOntology#ActOfCongratulating">
        <rdfs:label rdf:datatype="&xsd;string">Act of Congratulating</rdfs:label>
        <rdfs:subClassOf rdf:resource="http://www.cubrc.org/ontologies/KDD/Mid/EventOntology#ActOfExpressiveCommunication"/>
    </owl:Class>
    


    <!-- http://www.cubrc.org/ontologies/KDD/Mid/EventOntology#ActOfConspiracy -->

    <owl:Class rdf:about="http://www.cubrc.org/ontologies/KDD/Mid/EventOntology#ActOfConspiracy">
        <rdfs:label>Act Of Conspiracy</rdfs:label>
        <rdfs:subClassOf rdf:resource="http://www.cubrc.org/ontologies/KDD/Mid/EventOntology#InchoateCriminalAct"/>
        <rdfs:comment>Definition: An Inchoate Criminal Act of agreement between two or more persons to break the law at some time in the future, and, in some cases, with at least one overt act in furtherance of that agreement. (derived from http://en.wikipedia.org/wiki/Conspiracy_(crime))</rdfs:comment>
    </owl:Class>
    


    <!-- http://www.cubrc.org/ontologies/KDD/Mid/EventOntology#ActOfConspiracyToCommitActOfArmsSmuggling -->

    <owl:Class rdf:about="http://www.cubrc.org/ontologies/KDD/Mid/EventOntology#ActOfConspiracyToCommitActOfArmsSmuggling">
        <rdfs:label>Act of Conspiracy to Commit Act of Arms Smuggling</rdfs:label>
        <rdfs:subClassOf rdf:resource="http://www.cubrc.org/ontologies/KDD/Mid/EventOntology#ActOfConspiracy"/>
    </owl:Class>
    


    <!-- http://www.cubrc.org/ontologies/KDD/Mid/EventOntology#ActOfConspiracyToCommitActOfArmsTrafficking -->

    <owl:Class rdf:about="http://www.cubrc.org/ontologies/KDD/Mid/EventOntology#ActOfConspiracyToCommitActOfArmsTrafficking">
        <rdfs:label>Act of Conspiracy to Commit Act of Arms Trafficking</rdfs:label>
        <rdfs:subClassOf rdf:resource="http://www.cubrc.org/ontologies/KDD/Mid/EventOntology#ActOfConspiracy"/>
    </owl:Class>
    


    <!-- http://www.cubrc.org/ontologies/KDD/Mid/EventOntology#ActOfConspiracyToCommitActOfFraud -->

    <owl:Class rdf:about="http://www.cubrc.org/ontologies/KDD/Mid/EventOntology#ActOfConspiracyToCommitActOfFraud">
        <rdfs:label>Act of Conspiracy to Commit Act of Fraud</rdfs:label>
        <rdfs:subClassOf rdf:resource="http://www.cubrc.org/ontologies/KDD/Mid/EventOntology#ActOfConspiracy"/>
    </owl:Class>
    


    <!-- http://www.cubrc.org/ontologies/KDD/Mid/EventOntology#ActOfConspiracyToCommitActOfIllegalDrugManufacturing -->

    <owl:Class rdf:about="http://www.cubrc.org/ontologies/KDD/Mid/EventOntology#ActOfConspiracyToCommitActOfIllegalDrugManufacturing">
        <rdfs:label>Act of Conspiracy to Commit Act of Illegal Drug Manufacturing</rdfs:label>
        <rdfs:subClassOf rdf:resource="http://www.cubrc.org/ontologies/KDD/Mid/EventOntology#ActOfConspiracy"/>
    </owl:Class>
    


    <!-- http://www.cubrc.org/ontologies/KDD/Mid/EventOntology#ActOfConspiracyToCommitActOfIllegalDrugSmuggling -->

    <owl:Class rdf:about="http://www.cubrc.org/ontologies/KDD/Mid/EventOntology#ActOfConspiracyToCommitActOfIllegalDrugSmuggling">
        <rdfs:label>Act of Conspiracy to Commit Act of Illegal Drug Smuggling</rdfs:label>
        <rdfs:subClassOf rdf:resource="http://www.cubrc.org/ontologies/KDD/Mid/EventOntology#ActOfConspiracy"/>
    </owl:Class>
    


    <!-- http://www.cubrc.org/ontologies/KDD/Mid/EventOntology#ActOfConspiracyToCommitActOfIllegalDrugTrafficking -->

    <owl:Class rdf:about="http://www.cubrc.org/ontologies/KDD/Mid/EventOntology#ActOfConspiracyToCommitActOfIllegalDrugTrafficking">
        <rdfs:label>Act of Conspiracy to Commit Act of Illegal Drug Trafficking</rdfs:label>
        <rdfs:subClassOf rdf:resource="http://www.cubrc.org/ontologies/KDD/Mid/EventOntology#ActOfConspiracy"/>
    </owl:Class>
    


    <!-- http://www.cubrc.org/ontologies/KDD/Mid/EventOntology#ActOfConspiracyToCommitActOfMurder -->

    <owl:Class rdf:about="http://www.cubrc.org/ontologies/KDD/Mid/EventOntology#ActOfConspiracyToCommitActOfMurder">
        <rdfs:label>Act of Conspiracy to Commit Act of Murder</rdfs:label>
        <rdfs:subClassOf rdf:resource="http://www.cubrc.org/ontologies/KDD/Mid/EventOntology#ActOfConspiracy"/>
    </owl:Class>
    


    <!-- http://www.cubrc.org/ontologies/KDD/Mid/EventOntology#ActOfConstructiveManslaughter -->

    <owl:Class rdf:about="http://www.cubrc.org/ontologies/KDD/Mid/EventOntology#ActOfConstructiveManslaughter">
        <rdfs:label>Act Of Constructive Manslaughter</rdfs:label>
        <rdfs:subClassOf rdf:resource="http://www.cubrc.org/ontologies/KDD/Mid/EventOntology#ActOfInvoluntaryManslaughter"/>
        <rdfs:comment>Definition: An Act of Involuntary Manslaughter that  occurs when someone kills, without intent, in the course of committing an unlawful act (derived from http://en.wikipedia.org/wiki/Manslaughter).</rdfs:comment>
    </owl:Class>
    


    <!-- http://www.cubrc.org/ontologies/KDD/Mid/EventOntology#ActOfContinuance -->

    <owl:Class rdf:about="http://www.cubrc.org/ontologies/KDD/Mid/EventOntology#ActOfContinuance">
        <rdfs:label>Act Of Continuance</rdfs:label>
        <rdfs:subClassOf rdf:resource="http://www.cubrc.org/ontologies/KDD/Mid/EventOntology#LegalSystemAct"/>
        <rdfs:comment>Definition: A Legal System Act of postponing a Trial to a later date. (derived from http://www.id.uscourts.gov/glossary.htm)</rdfs:comment>
    </owl:Class>
    


    <!-- http://www.cubrc.org/ontologies/KDD/Mid/EventOntology#ActOfContractFormation -->

    <owl:Class rdf:about="http://www.cubrc.org/ontologies/KDD/Mid/EventOntology#ActOfContractFormation">
        <rdfs:label xml:lang="en">Act Of Contract Formation</rdfs:label>
        <rdfs:subClassOf rdf:resource="http://www.cubrc.org/ontologies/KDD/Mid/EventOntology#ActOfPromising"/>
        <rdfs:comment>Definition: An Act Of Promising having a lawful object entered into voluntarily by two or more agents with legal capacity, each of whom intends to create one or more legal obligations between them. (derived from http://en.wikipedia.org/wiki/Contract#Formation) </rdfs:comment>
    </owl:Class>
    


    <!-- http://www.cubrc.org/ontologies/KDD/Mid/EventOntology#ActOfConviction -->

    <owl:Class rdf:about="http://www.cubrc.org/ontologies/KDD/Mid/EventOntology#ActOfConviction">
        <rdfs:label>Act Of Conviction</rdfs:label>
        <rdfs:subClassOf rdf:resource="http://www.cubrc.org/ontologies/KDD/Mid/EventOntology#LegalSystemAct"/>
        <rdfs:comment>Definition: A Legal System Act of issuing a judgment of guilt against the defendant in a Criminal Trial (derived from http://www.id.uscourts.gov/glossary.htm)</rdfs:comment>
    </owl:Class>
    


    <!-- http://www.cubrc.org/ontologies/KDD/Mid/EventOntology#ActOfConvoySecurityOperation -->

    <owl:Class rdf:about="http://www.cubrc.org/ontologies/KDD/Mid/EventOntology#ActOfConvoySecurityOperation">
        <rdfs:label>Conduct Convoy Security Operation</rdfs:label>
        <rdfs:subClassOf rdf:resource="http://www.cubrc.org/ontologies/KDD/Mid/EventOntology#ActOfOperationalAreaSecurity"/>
        <rdfs:comment>Definition: An Action of Operational Area Security in which convoys are protected against the danger of enemy ground action. Convoy security operations are defensive in nature and orient on the protected force.  (derived from The Army Universal Task List FM 7-15 February 2009).</rdfs:comment>
    </owl:Class>
    


    <!-- http://www.cubrc.org/ontologies/KDD/Mid/EventOntology#ActOfCopyrightedMediaTrafficking -->

    <owl:Class rdf:about="http://www.cubrc.org/ontologies/KDD/Mid/EventOntology#ActOfCopyrightedMediaTrafficking">
        <rdfs:label>Act Of Copyrighted Media Trafficking</rdfs:label>
        <rdfs:subClassOf rdf:resource="http://www.cubrc.org/ontologies/KDD/Mid/EventOntology#ActOfBlackMarketTrafficking"/>
        <rdfs:comment>Definition: An Act of Black Market Trafficking involving the illegal manufacture, distribution, and sale of counterfeit copyrighted material.</rdfs:comment>
    </owl:Class>
    


    <!-- http://www.cubrc.org/ontologies/KDD/Mid/EventOntology#ActOfCounterambushManeuver -->

    <owl:Class rdf:about="http://www.cubrc.org/ontologies/KDD/Mid/EventOntology#ActOfCounterambushManeuver">
        <rdfs:label>Conduct Counterambush Action</rdfs:label>
        <rdfs:subClassOf rdf:resource="http://www.cubrc.org/ontologies/KDD/Mid/EventOntology#ActOfForceManeuver"/>
        <rdfs:comment>Definition: An Act of Force Maneuver which is an immediate action against near and far ambushes to minimize casualties, exit the enemy engagement area, inflict casualties on the enemy ambush force, and continue the mission (derived from The Army Universal Task List FM 7-15 February 2009).</rdfs:comment>
    </owl:Class>
    


    <!-- http://www.cubrc.org/ontologies/KDD/Mid/EventOntology#ActOfCounterfeitPrescriptionDrugTrafficking -->

    <owl:Class rdf:about="http://www.cubrc.org/ontologies/KDD/Mid/EventOntology#ActOfCounterfeitPrescriptionDrugTrafficking">
        <rdfs:label>Act Of Counterfeit Prescription Drug Trafficking</rdfs:label>
        <rdfs:subClassOf rdf:resource="http://www.cubrc.org/ontologies/KDD/Mid/EventOntology#ActOfDrugTrafficking"/>
        <rdfs:comment>Definition: An Act of Drug Trafficking involving the manufacture, distribution, and sale of Counterfeit Prescription Drugs.</rdfs:comment>
    </owl:Class>
    


    <!-- http://www.cubrc.org/ontologies/KDD/Mid/EventOntology#ActOfCounterfeiting -->

    <owl:Class rdf:about="http://www.cubrc.org/ontologies/KDD/Mid/EventOntology#ActOfCounterfeiting">
        <rdfs:label>Act of Counterfeiting</rdfs:label>
        <rdfs:subClassOf rdf:resource="http://www.cubrc.org/ontologies/KDD/Mid/EventOntology#ActOfFraud"/>
        <rdfs:comment rdf:datatype="&xsd;string">Definition: An act of fraud performed by altering, copying, or imitating something, without authority or right, with the intent to deceive or defraud by passing the copy or thing altered or imitated as that which is original or genuine; or the selling, buying, or possession of an altered, copied, or imitated thing with the intent to deceive or defraud. Attempts are included. (derived from definition of Forgery and Counterfeiting at: http://www2.fbi.gov/ucr/cius2009/about/offense_definitions.html)</rdfs:comment>
    </owl:Class>
    


    <!-- http://www.cubrc.org/ontologies/KDD/Mid/EventOntology#ActOfCountermobilityOperation -->

    <owl:Class rdf:about="http://www.cubrc.org/ontologies/KDD/Mid/EventOntology#ActOfCountermobilityOperation">
        <rdfs:label>Conduct a Countermobility Operation</rdfs:label>
        <rdfs:subClassOf rdf:resource="http://www.cubrc.org/ontologies/KDD/Mid/EventOntology#ActOfMovementAndManeuverWarfighting"/>
        <rdfs:comment>Definition: An Act of Military Force involving the construction of reinforcing obstacles integrated with fires to inhibit the maneuver of an enemy force, increase time for target acquisition, and increase weapon effectiveness.  (derived from The Army Universal Task List FM 7-15 February 2009).</rdfs:comment>
    </owl:Class>
    


    <!-- http://www.cubrc.org/ontologies/KDD/Mid/EventOntology#ActOfCriminalConversion -->

    <owl:Class rdf:about="http://www.cubrc.org/ontologies/KDD/Mid/EventOntology#ActOfCriminalConversion">
        <rdfs:label>Act Of Criminal Conversion</rdfs:label>
        <rdfs:subClassOf rdf:resource="http://www.cubrc.org/ontologies/KDD/Mid/EventOntology#CriminalActAgainstProperty"/>
        <rdfs:comment>Definition: A Criminal Act Against Property of exerting unauthorized use or control of another persons property. It differs from theft in that it does not include the element of intending to deprive the owner of the possession of that property. (derived from http://en.wikipedia.org/wiki/Criminal_conversion).</rdfs:comment>
    </owl:Class>
    


    <!-- http://www.cubrc.org/ontologies/KDD/Mid/EventOntology#ActOfCriminalHomicide -->

    <owl:Class rdf:about="http://www.cubrc.org/ontologies/KDD/Mid/EventOntology#ActOfCriminalHomicide">
        <rdfs:label>Act Of Criminal Homicide</rdfs:label>
        <rdfs:subClassOf rdf:resource="http://www.cubrc.org/ontologies/KDD/Mid/EventOntology#CriminalActAgainstThePerson"/>
        <rdfs:comment>Definition: A Criminal Act Against the Person of killing  one human by another and having circumstances that fall within outlawed behavior. (derived from http://en.wikipedia.org/wiki/Homicide)</rdfs:comment>
    </owl:Class>
    


    <!-- http://www.cubrc.org/ontologies/KDD/Mid/EventOntology#ActOfCriminallyNegligentManslaughter -->

    <owl:Class rdf:about="http://www.cubrc.org/ontologies/KDD/Mid/EventOntology#ActOfCriminallyNegligentManslaughter">
        <rdfs:label>Act Of Criminally Negligent Manslaughter</rdfs:label>
        <rdfs:subClassOf rdf:resource="http://www.cubrc.org/ontologies/KDD/Mid/EventOntology#ActOfInvoluntaryManslaughter"/>
        <rdfs:comment>Definition: An Act of Involuntary Manslaughter that  occurs when death results from serious negligence, or, in some jurisdictions, serious recklessness (derived from http://en.wikipedia.org/wiki/Manslaughter).</rdfs:comment>
    </owl:Class>
    


    <!-- http://www.cubrc.org/ontologies/KDD/Mid/EventOntology#ActOfCrossingADangerArea -->

    <owl:Class rdf:about="http://www.cubrc.org/ontologies/KDD/Mid/EventOntology#ActOfCrossingADangerArea">
        <rdfs:label>Cross a Danger Area</rdfs:label>
        <rdfs:subClassOf rdf:resource="http://www.cubrc.org/ontologies/KDD/Mid/EventOntology#ActOfForceManeuver"/>
        <rdfs:comment>Definition: An Act of Force Maneuver in which forces rapidly move across potential enemy engagement areas without detection by the enemy and without exposing the entire force (derived from The Army Universal Task List FM 7-15 February 2009).</rdfs:comment>
    </owl:Class>
    


    <!-- http://www.cubrc.org/ontologies/KDD/Mid/EventOntology#ActOfCustody -->

    <owl:Class rdf:about="http://www.cubrc.org/ontologies/KDD/Mid/EventOntology#ActOfCustody">
        <rdfs:label>Act Of Custody</rdfs:label>
        <rdfs:subClassOf rdf:resource="http://www.cubrc.org/ontologies/KDD/Mid/EventOntology#LegalSystemAct"/>
        <rdfs:comment>Definition: A Legal System Act of detaining a Person by lawful process or authority to assure his or her appearance to any Hearing or Trial. (derived from http://www.id.uscourts.gov/glossary.htm)</rdfs:comment>
    </owl:Class>
    


    <!-- http://www.cubrc.org/ontologies/KDD/Mid/EventOntology#ActOfDeceptiveCommunication -->

    <owl:Class rdf:about="http://www.cubrc.org/ontologies/KDD/Mid/EventOntology#ActOfDeceptiveCommunication">
        <rdfs:label>Act Of Deceptive Communication</rdfs:label>
        <rdfs:subClassOf rdf:resource="http://www.cubrc.org/ontologies/KDD/Mid/EventOntology#ActOfCommunication"/>
        <rdfs:comment>Definition: Ac Act Of Communication intended to mislead the audience by distortion or falsification of evidence and induce a reaction that is prejudicial to the interests of the audience. (derived from JC3IEDM-MIRD-DMWG-Edition_3.0.2_20090514)</rdfs:comment>
    </owl:Class>
    


    <!-- http://www.cubrc.org/ontologies/KDD/Mid/EventOntology#ActOfDecidingSurfaceFires -->

    <owl:Class rdf:about="http://www.cubrc.org/ontologies/KDD/Mid/EventOntology#ActOfDecidingSurfaceFires">
        <rdfs:label>Decide Surface Fires</rdfs:label>
        <rdfs:subClassOf rdf:resource="http://www.cubrc.org/ontologies/KDD/Mid/EventOntology#ActOfFiresWarfighting"/>
        <rdfs:comment>Definition: An Act of Fires Warfighting in which a force analyzes the situation relative to the mission, objectives, and capabilities and identifies and nominates specific vulnerabilities, high-value targets, and high-payoff targets that if influenced, degraded, delayed, disrupted, disabled, or destroyed will accomplish the commander�s intent (derived from The Army Universal Task List FM 7-15 February 2009).</rdfs:comment>
    </owl:Class>
    


    <!-- http://www.cubrc.org/ontologies/KDD/Mid/EventOntology#ActOfDeclarativeCommunication -->

    <owl:Class rdf:about="http://www.cubrc.org/ontologies/KDD/Mid/EventOntology#ActOfDeclarativeCommunication">
        <rdfs:label rdf:datatype="&xsd;string">Act Of Declarative Communication</rdfs:label>
        <rdfs:subClassOf rdf:resource="http://www.cubrc.org/ontologies/KDD/Mid/EventOntology#ActOfPersonalCommunication"/>
        <rdfs:comment rdf:datatype="&xsd;string">Definition: An Act Of Communication that changes the reality in accord with the proposition fo the declaration (loosely derived from John Searle&apos;s Speech Acts: An Essay in the Philosophy of Language).</rdfs:comment>
        <rdfs:comment rdf:datatype="&xsd;string">Examples: Baptism, Sentencing a person to imprisonment, Pronouncing a couple husband and wife, Declaring war</rdfs:comment>
    </owl:Class>
    


    <!-- http://www.cubrc.org/ontologies/KDD/Mid/EventOntology#ActOfDecoyUse -->

    <owl:Class rdf:about="http://www.cubrc.org/ontologies/KDD/Mid/EventOntology#ActOfDecoyUse">
        <rdfs:label rdf:datatype="&xsd;string">Act of decoy use</rdfs:label>
        <rdfs:subClassOf rdf:resource="http://www.cubrc.org/ontologies/KDD/Mid/EventOntology#ActOfInstrumentUse"/>
        <rdfs:comment rdf:datatype="&xsd;string">Definition: An Act Of Instrument Use in which some Agent uses some Decoy</rdfs:comment>
    </owl:Class>
    


    <!-- http://www.cubrc.org/ontologies/KDD/Mid/EventOntology#ActOfDefensiveOperation -->

    <owl:Class rdf:about="http://www.cubrc.org/ontologies/KDD/Mid/EventOntology#ActOfDefensiveOperation">
        <rdfs:label>Conduct Defensive Operation</rdfs:label>
        <rdfs:subClassOf rdf:resource="http://www.cubrc.org/ontologies/KDD/Mid/EventOntology#ActOfMilitaryForce"/>
        <rdfs:comment>Definition: An Act of Military Force conducted to defeat an enemy attack, gain time, economize forces, and develop conditions favorable for offensive or stability operations. (derived from The Army Universal Task List FM 7-15 February 2009).</rdfs:comment>
    </owl:Class>
    


    <!-- http://www.cubrc.org/ontologies/KDD/Mid/EventOntology#ActOfDenial -->

    <owl:Class rdf:about="http://www.cubrc.org/ontologies/KDD/Mid/EventOntology#ActOfDenial">
        <rdfs:label rdf:datatype="&xsd;string">Act Of Denial</rdfs:label>
        <rdfs:subClassOf rdf:resource="http://www.cubrc.org/ontologies/KDD/Mid/EventOntology#ActOfRepresentativeCommunication"/>
    </owl:Class>
    


    <!-- http://www.cubrc.org/ontologies/KDD/Mid/EventOntology#ActOfDetectingAndLocatingSurfaceTarget -->

    <owl:Class rdf:about="http://www.cubrc.org/ontologies/KDD/Mid/EventOntology#ActOfDetectingAndLocatingSurfaceTarget">
        <rdfs:label>Detect and Locate Surface Targets</rdfs:label>
        <rdfs:subClassOf rdf:resource="http://www.cubrc.org/ontologies/KDD/Mid/EventOntology#ActOfFiresWarfighting"/>
        <rdfs:comment>Definition: An Act of Fires Warfighting in which a force perceives an object of possible military interest without confirming it by recognition (detect) and determines the placement of a target on the battlefield (locate) (derived from The Army Universal Task List FM 7-15 February 2009).</rdfs:comment>
    </owl:Class>
    


    <!-- http://www.cubrc.org/ontologies/KDD/Mid/EventOntology#ActOfDirectFire -->

    <owl:Class rdf:about="http://www.cubrc.org/ontologies/KDD/Mid/EventOntology#ActOfDirectFire">
        <rdfs:label>Direct Fire</rdfs:label>
        <rdfs:subClassOf rdf:resource="http://www.cubrc.org/ontologies/KDD/Mid/EventOntology#ActOfMovementAndManeuverWarfighting"/>
        <rdfs:comment>Definition: An Act of Military Force in which some Force conducts lethal and nonlethal direct fires using weapon systems such as small arms, tanks, antitank weapons, automatic weapons, directed energy, optical, acoustic, and blunt trauma weapons (derived from The Army Universal Task List FM 7-15 February 2009).</rdfs:comment>
    </owl:Class>
    


    <!-- http://www.cubrc.org/ontologies/KDD/Mid/EventOntology#ActOfDirectiveCommunication -->

    <owl:Class rdf:about="http://www.cubrc.org/ontologies/KDD/Mid/EventOntology#ActOfDirectiveCommunication">
        <rdfs:label rdf:datatype="&xsd;string">Act Of Directive Communication</rdfs:label>
        <rdfs:subClassOf rdf:resource="http://www.cubrc.org/ontologies/KDD/Mid/EventOntology#ActOfPersonalCommunication"/>
        <rdfs:comment rdf:datatype="&xsd;string">Definition: An Act Of Personal Communication that are to cause the hearer to take a particular action (loosely derived from John Searle&apos;s Speech Acts: An Essay in the Philosophy of Language)</rdfs:comment>
        <rdfs:comment rdf:datatype="&xsd;string">Examples: advising, admonishing, asking, begging, dismissing, excusing, forbidding, instructing, ordering, permitting, requesting, requiring, suggesting, urging, warning</rdfs:comment>
    </owl:Class>
    


    <!-- http://www.cubrc.org/ontologies/KDD/Mid/EventOntology#ActOfDisabledEquipmentRecovery -->

    <owl:Class rdf:about="http://www.cubrc.org/ontologies/KDD/Mid/EventOntology#ActOfDisabledEquipmentRecovery">
        <rdfs:label>Recover Disabled Equipment</rdfs:label>
        <rdfs:subClassOf rdf:resource="http://www.cubrc.org/ontologies/KDD/Mid/EventOntology#ActOfMaintenanceSupport"/>
        <rdfs:comment>Definition: An Act of Maintenance Support in which damaged, discarded, condemned, or abandoned multinational or enemy materiel (ground, aircraft, and marine) are recovered and evacuated (derived from The Army Universal Task List FM 7-15 February 2009).</rdfs:comment>
    </owl:Class>
    


    <!-- http://www.cubrc.org/ontologies/KDD/Mid/EventOntology#ActOfDonating -->

    <owl:Class rdf:about="http://www.cubrc.org/ontologies/KDD/Mid/EventOntology#ActOfDonating">
        <rdfs:label rdf:datatype="&xsd;string">Act Of Donating</rdfs:label>
        <rdfs:subClassOf rdf:resource="http://www.cubrc.org/ontologies/KDD/Mid/EventOntology#ActOfFinancialInstrumentUse"/>
        <rdfs:comment rdf:datatype="&xsd;string">Definition: An Act of Financial Instrument Use wherein a Financial Instrument by Function or a Finanical Instrument by Role is tranfered by an agent (donor) to another Agent (Recipient) without return consideration (derived from http://en.wikipedia.org/wiki/Donation)</rdfs:comment>
    </owl:Class>
    


    <!-- http://www.cubrc.org/ontologies/KDD/Mid/EventOntology#ActOfDrugTrafficking -->

    <owl:Class rdf:about="http://www.cubrc.org/ontologies/KDD/Mid/EventOntology#ActOfDrugTrafficking">
        <rdfs:label>Act Of Drug Trafficking</rdfs:label>
        <rdfs:subClassOf rdf:resource="http://www.cubrc.org/ontologies/KDD/Mid/EventOntology#ActOfBlackMarketTrafficking"/>
        <rdfs:comment>Definition: An Act Of Black Market Trafficking involving the cultivation, manufacture, distribution and sale of substances which are subject to drug prohibition or drug regulation laws. (derived from http://en.wikipedia.org/wiki/Illegal_drug_trade).</rdfs:comment>
    </owl:Class>
    


    <!-- http://www.cubrc.org/ontologies/KDD/Mid/EventOntology#ActOfEconomicSupport -->

    <owl:Class rdf:about="http://www.cubrc.org/ontologies/KDD/Mid/EventOntology#ActOfEconomicSupport">
        <rdfs:label>Economic Support</rdfs:label>
        <rdfs:subClassOf rdf:resource="http://www.cubrc.org/ontologies/KDD/Mid/EventOntology#ActOfCivilAffairs"/>
        <rdfs:comment>Definition: An Act of Civil Affairs that includes instances of any of the following types of action: determining the availability of local resources for military and civilian use, determining the economic controls and the governmental structure related to economics and commerce, assisting in the development and execution of price control and rationing programs, direct support to keep key industries operating, developing and implementing plans to prevent black-market activities (derived from The Army Universal Task List FM 7-15 February 2009).</rdfs:comment>
    </owl:Class>
    


    <!-- http://www.cubrc.org/ontologies/KDD/Mid/EventOntology#ActOfEducationalTrainingAcquisition -->

    <owl:Class rdf:about="http://www.cubrc.org/ontologies/KDD/Mid/EventOntology#ActOfEducationalTrainingAcquisition">
        <rdfs:label rdf:datatype="&xsd;string">Act Of Educational Training Acquisition</rdfs:label>
        <rdfs:subClassOf rdf:resource="http://www.cubrc.org/ontologies/KDD/Mid/EventOntology#ActOfTrainingAcquisition"/>
        <rdfs:comment rdf:datatype="&xsd;string">Definition: An Act of Training performed by an Agent by acquiring knowledge of a curriculum from an Agent or communication medium affiliated with some Educational Organization.</rdfs:comment>
    </owl:Class>
    


    <!-- http://www.cubrc.org/ontologies/KDD/Mid/EventOntology#ActOfEducationalTrainingInstruction -->

    <owl:Class rdf:about="http://www.cubrc.org/ontologies/KDD/Mid/EventOntology#ActOfEducationalTrainingInstruction">
        <rdfs:label rdf:datatype="&xsd;string">Act Of Educational Training Instruction</rdfs:label>
        <rdfs:subClassOf rdf:resource="http://www.cubrc.org/ontologies/KDD/Mid/EventOntology#ActOfTrainingInstruction"/>
        <rdfs:comment rdf:datatype="&xsd;string">Definition: An Act of Training performed by an Agent affiliatied with some Educational Organization by imparting knowledge of a curriculum to an Agent either directly or indirectly through some communication medium.</rdfs:comment>
    </owl:Class>
    


    <!-- http://www.cubrc.org/ontologies/KDD/Mid/EventOntology#ActOfEmbezzlement -->

    <owl:Class rdf:about="http://www.cubrc.org/ontologies/KDD/Mid/EventOntology#ActOfEmbezzlement">
        <rdfs:label>Act Of Embezzlement</rdfs:label>
        <rdfs:subClassOf rdf:resource="http://www.cubrc.org/ontologies/KDD/Mid/EventOntology#CriminalActAgainstProperty"/>
        <rdfs:comment>Definition: A Criminal Act Against Property of dishonestly appropriating or secreting assets by one or more individuals to whom such assets have been entrusted. (derived from http://en.wikipedia.org/wiki/Embezzlement).</rdfs:comment>
    </owl:Class>
    


    <!-- http://www.cubrc.org/ontologies/KDD/Mid/EventOntology#ActOfEmployingAirAndMissleDefense -->

    <owl:Class rdf:about="http://www.cubrc.org/ontologies/KDD/Mid/EventOntology#ActOfEmployingAirAndMissleDefense">
        <rdfs:label>Employ Air and Missle Defense</rdfs:label>
        <rdfs:subClassOf rdf:resource="http://www.cubrc.org/ontologies/KDD/Mid/EventOntology#ActOfProtectionWarfighting"/>
        <rdfs:comment>Definition: An Act of Protection Warfighting in which the force is protected from missile attack, air attack, and aerial surveillance by any of the following: interceptor missiles, ballistic missiles, cruise missiles, conventional fixed- and rotarywing aircraft, and unmanned aircraft systems (derived from The Army Universal Task List FM 7-15 February 2009).</rdfs:comment>
    </owl:Class>
    


    <!-- http://www.cubrc.org/ontologies/KDD/Mid/EventOntology#ActOfEmployingObscurants -->

    <owl:Class rdf:about="http://www.cubrc.org/ontologies/KDD/Mid/EventOntology#ActOfEmployingObscurants">
        <rdfs:label>Employ Obscurants</rdfs:label>
        <rdfs:subClassOf rdf:resource="http://www.cubrc.org/ontologies/KDD/Mid/EventOntology#ActOfMovementAndManeuverWarfighting"/>
        <rdfs:comment>Definition: Act of Military Force in which a chemical agent that decreases the level of energy available for the functions of seekers, trackers, and vision enhancement devices is used to conceal friendly positions and screen maneuvering forces from enemy observation (derived from The Army Universal Task List FM 7-15 February 2009).</rdfs:comment>
    </owl:Class>
    


    <!-- http://www.cubrc.org/ontologies/KDD/Mid/EventOntology#ActOfEmployingProtectiveEquipment -->

    <owl:Class rdf:about="http://www.cubrc.org/ontologies/KDD/Mid/EventOntology#ActOfEmployingProtectiveEquipment">
        <rdfs:label>Employ Protective Equipment</rdfs:label>
        <rdfs:subClassOf rdf:resource="http://www.cubrc.org/ontologies/KDD/Mid/EventOntology#ActOfSurvivabilityOperation"/>
        <rdfs:comment>Definition: An Act of Employment Operation during which individual and collective equipment is employed to protect personnel, systems, and facilities against hazards caused by enemy action. Protective equipment includes individual and collective chemical, biological, radiological, and nuclear (CBRN) detection and protective systems. It also includes using other items such as bullet-resistant glazing, hydraulically or manually operated vehicle crash barriers, personnel gates that limit the number of personnel passing through at one time, intrusion detection systems, security lighting, and security fences (derived from The Army Universal Task List FM 7-15 February 2009).</rdfs:comment>
    </owl:Class>
    


    <!-- http://www.cubrc.org/ontologies/KDD/Mid/EventOntology#ActOfEmployingSafetyTechniques -->

    <owl:Class rdf:about="http://www.cubrc.org/ontologies/KDD/Mid/EventOntology#ActOfEmployingSafetyTechniques">
        <rdfs:label>Employ Safety Techniques</rdfs:label>
        <rdfs:subClassOf rdf:resource="http://www.cubrc.org/ontologies/KDD/Mid/EventOntology#ActOfProtectionWarfighting"/>
        <rdfs:comment>Definition: An Act of Protection Warfighting in which hazards to the force are identified and recommendations are made on ways to mitigate those hazards (derived from The Army Universal Task List FM 7-15 February 2009).</rdfs:comment>
    </owl:Class>
    


    <!-- http://www.cubrc.org/ontologies/KDD/Mid/EventOntology#ActOfEmployment -->

    <owl:Class rdf:about="http://www.cubrc.org/ontologies/KDD/Mid/EventOntology#ActOfEmployment">
        <rdfs:label rdf:datatype="&xsd;string">Act Of Employment</rdfs:label>
        <rdfs:subClassOf rdf:resource="http://www.cubrc.org/ontologies/KDD/Mid/EventOntology#ActOfAssociation"/>
        <rdfs:comment rdf:datatype="&xsd;string">Definition: An Act of Association wherein an Organization assigns a set of activities to some Person to be performed in exchange for financial compensation.</rdfs:comment>
    </owl:Class>
    


    <!-- http://www.cubrc.org/ontologies/KDD/Mid/EventOntology#ActOfEncounter -->

    <owl:Class rdf:about="http://www.cubrc.org/ontologies/KDD/Mid/EventOntology#ActOfEncounter">
        <rdfs:label rdf:datatype="&xsd;string">Act of Encounter</rdfs:label>
        <rdfs:subClassOf rdf:resource="http://www.cubrc.org/ontologies/KDD/Mid/EventOntology#ActOfAssociation"/>
        <rdfs:comment rdf:datatype="&xsd;string">Definition: An Act Of Association wherein two or more Persons meet in a casual, unplanned manner (derived from http://wordnetweb.princeton.edu/perl/webwn?s=encounter) (Sense Key: Encounter%2:38:00)</rdfs:comment>
    </owl:Class>
    


    <!-- http://www.cubrc.org/ontologies/KDD/Mid/EventOntology#ActOfEngineeringSupport -->

    <owl:Class rdf:about="http://www.cubrc.org/ontologies/KDD/Mid/EventOntology#ActOfEngineeringSupport">
        <rdfs:label>Engineering Support</rdfs:label>
        <rdfs:subClassOf rdf:resource="http://www.cubrc.org/ontologies/KDD/Mid/EventOntology#ActOfLogisticSupport"/>
        <rdfs:comment>Definition: An Act of Logistic Support involving either the construction, repair or acquisition of facilities and transportation routes (derived from The Army Universal Task List FM 7-15 February 2009).</rdfs:comment>
    </owl:Class>
    


    <!-- http://www.cubrc.org/ontologies/KDD/Mid/EventOntology#ActOfEntertainment -->

    <owl:Class rdf:about="http://www.cubrc.org/ontologies/KDD/Mid/EventOntology#ActOfEntertainment">
        <rdfs:label rdf:datatype="&xsd;string">Act Of Entertainment</rdfs:label>
        <rdfs:subClassOf rdf:resource="http://www.cubrc.org/ontologies/KDD/Mid/EventOntology#IntentionalAct"/>
        <rdfs:comment rdf:datatype="&xsd;string">An Intentional Act consisting of any activity which provides a diversion or permits people to amuse themselves in their leisure time. (derived from http://en.wikipedia.org/wiki/Entertainment)</rdfs:comment>
    </owl:Class>
    


    <!-- http://www.cubrc.org/ontologies/KDD/Mid/EventOntology#ActOfEnvelopmentManeuver -->

    <owl:Class rdf:about="http://www.cubrc.org/ontologies/KDD/Mid/EventOntology#ActOfEnvelopmentManeuver">
        <rdfs:label>Conduct an Evelopment</rdfs:label>
        <rdfs:subClassOf rdf:resource="http://www.cubrc.org/ontologies/KDD/Mid/EventOntology#ActOfForceManeuver"/>
        <rdfs:comment>Definition: An Act of Force Maneuver in which an attacking force seeks to avoid the principal enemy defenses by seizing objectives to the enemy rear to destroy the enemy in his current positions. At the tactical level, envelopments focus on seizing terrain, destroying specific enemy forces, and interdicting enemy withdrawal routes.  (derived from The Army Universal Task List FM 7-15 February 2009).</rdfs:comment>
    </owl:Class>
    


    <!-- http://www.cubrc.org/ontologies/KDD/Mid/EventOntology#ActOfEquipmentRepair -->

    <owl:Class rdf:about="http://www.cubrc.org/ontologies/KDD/Mid/EventOntology#ActOfEquipmentRepair">
        <rdfs:label>Repair Equipment</rdfs:label>
        <rdfs:subClassOf rdf:resource="http://www.cubrc.org/ontologies/KDD/Mid/EventOntology#ActOfMaintenanceSupport"/>
        <rdfs:comment>Definition: An Act of Maintenance Support in which an artifact is restored to serviceable condition by correcting a specific failure or unserviceable condition (derived from The Army Universal Task List FM 7-15 February 2009).</rdfs:comment>
    </owl:Class>
    


    <!-- http://www.cubrc.org/ontologies/KDD/Mid/EventOntology#ActOfEscapeFromDetentionFacility -->

    <owl:Class rdf:about="http://www.cubrc.org/ontologies/KDD/Mid/EventOntology#ActOfEscapeFromDetentionFacility">
        <rdfs:label>Act Of Escape From Detention Facility</rdfs:label>
        <rdfs:subClassOf rdf:resource="http://www.cubrc.org/ontologies/KDD/Mid/EventOntology#CriminalActAgainstJustice"/>
        <rdfs:comment>Definition: A CriminalAct Against Justice in which an inmate leaves prison through unofficial or illegal ways (derived from http://en.wikipedia.org/wiki/Prison_escape)</rdfs:comment>
    </owl:Class>
    


    <!-- http://www.cubrc.org/ontologies/KDD/Mid/EventOntology#ActOfEspionage -->

    <owl:Class rdf:about="http://www.cubrc.org/ontologies/KDD/Mid/EventOntology#ActOfEspionage">
        <rdfs:label rdf:datatype="&xsd;string">Act Of Espionage</rdfs:label>
        <rdfs:subClassOf rdf:resource="http://www.cubrc.org/ontologies/KDD/Mid/EventOntology#ActOfIntelligenceGathering"/>
        <rdfs:comment rdf:datatype="&xsd;string">Definition: An Act of Intelligence Gathering involving the obtaining of information that is considered secret or confidential without the permission of the holder of the information. (derived from http://en.wikipedia.org/wiki/Espionage)</rdfs:comment>
    </owl:Class>
    


    <!-- http://www.cubrc.org/ontologies/KDD/Mid/EventOntology#ActOfEstablishingCheckpoint -->

    <owl:Class rdf:about="http://www.cubrc.org/ontologies/KDD/Mid/EventOntology#ActOfEstablishingCheckpoint">
        <rdfs:label>Establish Checkpoint</rdfs:label>
        <rdfs:subClassOf rdf:resource="http://www.cubrc.org/ontologies/KDD/Mid/EventOntology#ActOfOperationalAreaSecurity"/>
        <rdfs:comment>Definition: An Act of Operational Area Secuirty in which checkpoints are established that will be used to monitor and control movement, inspect cargo, enforce rules and regulations, and provide information (derived from The Army Universal Task List FM 7-15 February 2009).</rdfs:comment>
    </owl:Class>
    


    <!-- http://www.cubrc.org/ontologies/KDD/Mid/EventOntology#ActOfEstablishingGuardPost -->

    <owl:Class rdf:about="http://www.cubrc.org/ontologies/KDD/Mid/EventOntology#ActOfEstablishingGuardPost">
        <rdfs:label>Establish Guard Post</rdfs:label>
        <rdfs:subClassOf rdf:resource="http://www.cubrc.org/ontologies/KDD/Mid/EventOntology#ActOfOperationalAreaSecurity"/>
        <rdfs:comment>Definition: An Act of Operational Area Security including delineation of the organization and functions of interior and exterior guards to include orders, countersigns, parole words, and responsibility of the main guard; the duties of personnel; and methods of mounting the guard (derived from The Army Universal Task List FM 7-15 February 2009).</rdfs:comment>
    </owl:Class>
    


    <!-- http://www.cubrc.org/ontologies/KDD/Mid/EventOntology#ActOfExplosiveDeviceUse -->

    <owl:Class rdf:about="http://www.cubrc.org/ontologies/KDD/Mid/EventOntology#ActOfExplosiveDeviceUse">
        <rdfs:label rdf:datatype="&xsd;string">Act Of Explosive Device Use</rdfs:label>
        <rdfs:subClassOf rdf:resource="http://www.cubrc.org/ontologies/KDD/Mid/EventOntology#ActOfWeaponUse"/>
        <rdfs:comment rdf:datatype="&xsd;string">An Act Of Weapon Use in which some Agent uses some Explosive Device</rdfs:comment>
    </owl:Class>
    


    <!-- http://www.cubrc.org/ontologies/KDD/Mid/EventOntology#ActOfExplosiveOrdnanceDisposalSupport -->

    <owl:Class rdf:about="http://www.cubrc.org/ontologies/KDD/Mid/EventOntology#ActOfExplosiveOrdnanceDisposalSupport">
        <rdfs:label>Explosive Ordnance Disposal Support</rdfs:label>
        <rdfs:subClassOf rdf:resource="http://www.cubrc.org/ontologies/KDD/Mid/EventOntology#ActOfProtectionWarfighting"/>
        <rdfs:comment>Definition: An Act of Military Force in which some Force (usually an Explosive Ordnance Disposal (EOD) team) seeks to eliminate or reduce the effects of unexploded explosive ordnance (UXO), improvised explosive devices (IEDs), and chemical, biological, radiological, and nuclear (CBRN) hazards to protect the commander�s combat power or which present a threat to civilian facilities, materiel and personnel, regardless of location (derived from The Army Universal Task List FM 7-15 February 2009).</rdfs:comment>
    </owl:Class>
    


    <!-- http://www.cubrc.org/ontologies/KDD/Mid/EventOntology#ActOfExpressiveCommunication -->

    <owl:Class rdf:about="http://www.cubrc.org/ontologies/KDD/Mid/EventOntology#ActOfExpressiveCommunication">
        <rdfs:label rdf:datatype="&xsd;string">Act Of Expressive Communication</rdfs:label>
        <rdfs:subClassOf rdf:resource="http://www.cubrc.org/ontologies/KDD/Mid/EventOntology#ActOfPersonalCommunication"/>
        <rdfs:comment rdf:datatype="&xsd;string">Definition: An Act Of Personal Communication that expresses the Speaker&apos;s attitudes and emotions towards some proposition (loosely derived from John Searle&apos;s Speech Acts: An Essay in the Philosophy of Language)</rdfs:comment>
        <rdfs:comment rdf:datatype="&xsd;string">Examples: apologizing, condoling, congratulating, greeting, thanking, accepting (acknowledging an acknowledgment)</rdfs:comment>
    </owl:Class>
    


    <!-- http://www.cubrc.org/ontologies/KDD/Mid/EventOntology#ActOfExpungement -->

    <owl:Class rdf:about="http://www.cubrc.org/ontologies/KDD/Mid/EventOntology#ActOfExpungement">
        <rdfs:label>Act Of Expungement</rdfs:label>
        <rdfs:subClassOf rdf:resource="http://www.cubrc.org/ontologies/KDD/Mid/EventOntology#LegalSystemAct"/>
        <rdfs:comment>Definition: A Legal System Act by which the record of a Person convicted of a crime is destroyed or sealed. (derived from http://www.id.uscourts.gov/glossary.htm)</rdfs:comment>
    </owl:Class>
    


    <!-- http://www.cubrc.org/ontologies/KDD/Mid/EventOntology#ActOfExtortion -->

    <owl:Class rdf:about="http://www.cubrc.org/ontologies/KDD/Mid/EventOntology#ActOfExtortion">
        <rdfs:label>Act Of Extortion</rdfs:label>
        <rdfs:subClassOf rdf:resource="http://www.cubrc.org/ontologies/KDD/Mid/EventOntology#CriminalActAgainstProperty"/>
        <rdfs:comment>Definition: A Criminal Act Against Property which occurs when a person unlawfully obtains either money, property or services from a person(s), entity, or institution, through coercion. (derived from http:/en.wikipedia.org/wiki/Extortion)</rdfs:comment>
    </owl:Class>
    


    <!-- http://www.cubrc.org/ontologies/KDD/Mid/EventOntology#ActOfExtradition -->

    <owl:Class rdf:about="http://www.cubrc.org/ontologies/KDD/Mid/EventOntology#ActOfExtradition">
        <rdfs:label>Act Of Extradition</rdfs:label>
        <rdfs:subClassOf rdf:resource="http://www.cubrc.org/ontologies/KDD/Mid/EventOntology#LegalSystemAct"/>
        <rdfs:comment>Definition: A Legal System Act in which a person accused of a Criminal Act is surrendered from one jurisdiction to another. (derived from http://www.id.uscourts.gov/glossary.htm)</rdfs:comment>
    </owl:Class>
    


    <!-- http://www.cubrc.org/ontologies/KDD/Mid/EventOntology#ActOfFacilityUse -->

    <owl:Class rdf:about="http://www.cubrc.org/ontologies/KDD/Mid/EventOntology#ActOfFacilityUse">
        <rdfs:label rdf:datatype="&xsd;string">Act Of Facility Use</rdfs:label>
        <rdfs:subClassOf rdf:resource="http://www.cubrc.org/ontologies/KDD/Mid/EventOntology#ActOfArtifactEmployment"/>
        <rdfs:comment rdf:datatype="&xsd;string">An Act Of Artifact Employment in which an Agent makes use of some Facility</rdfs:comment>
    </owl:Class>
    


    <!-- http://www.cubrc.org/ontologies/KDD/Mid/EventOntology#ActOfFalseImprisonment -->

    <owl:Class rdf:about="http://www.cubrc.org/ontologies/KDD/Mid/EventOntology#ActOfFalseImprisonment">
        <rdfs:label>Act Of False Imprisonment</rdfs:label>
        <rdfs:subClassOf rdf:resource="http://www.cubrc.org/ontologies/KDD/Mid/EventOntology#CriminalActAgainstThePerson"/>
        <rdfs:comment>Definition: A Criminal Act Against the Person False involving a restraint of a person in a bounded area without justification or consent (derived from http://en.wikipedia.org/wiki/False_imprisonment).</rdfs:comment>
    </owl:Class>
    


    <!-- http://www.cubrc.org/ontologies/KDD/Mid/EventOntology#ActOfFalsePretence -->

    <owl:Class rdf:about="http://www.cubrc.org/ontologies/KDD/Mid/EventOntology#ActOfFalsePretence">
        <rdfs:label>Act Of False Pretence</rdfs:label>
        <rdfs:subClassOf rdf:resource="http://www.cubrc.org/ontologies/KDD/Mid/EventOntology#CriminalActAgainstProperty"/>
        <rdfs:comment>Definition: A Criminal Act Against Property  which occurs when a person obtains money, property, or services from a person(s), entity, or institution by intentionally misrepresenting a past or existing fact. (derived from http:/en.wikipedia.org/wiki/False_pretenses)</rdfs:comment>
    </owl:Class>
    


    <!-- http://www.cubrc.org/ontologies/KDD/Mid/EventOntology#ActOfFelonyHomicide -->

    <owl:Class rdf:about="http://www.cubrc.org/ontologies/KDD/Mid/EventOntology#ActOfFelonyHomicide">
        <rdfs:label>Act Of Felony Homicide</rdfs:label>
        <rdfs:subClassOf rdf:resource="http://www.cubrc.org/ontologies/KDD/Mid/EventOntology#ActOfCriminalHomicide"/>
        <rdfs:comment>Definition: An Act of Criminal Homicide that occurs when an offender kills accidentally or without specific intent to kill in the course of an applicable felony, or when a death occurs during or in furtherance of that felony (derived from http://en.wikipedia.org/wiki/Felony_murder_rule).</rdfs:comment>
    </owl:Class>
    


    <!-- http://www.cubrc.org/ontologies/KDD/Mid/EventOntology#ActOfFinancialDeposit -->

    <owl:Class rdf:about="http://www.cubrc.org/ontologies/KDD/Mid/EventOntology#ActOfFinancialDeposit">
        <rdfs:label rdf:datatype="&xsd;string">Act Of Financial Deposit</rdfs:label>
        <rdfs:subClassOf rdf:resource="http://www.cubrc.org/ontologies/KDD/Mid/EventOntology#ActOfFinancialInstrumentUse"/>
        <rdfs:comment rdf:datatype="&xsd;string">Definition: An Act of Financial Instrument Use wherein a Financial Instrument by Function or a Finanical Instrument by Role is transferred by an agent (Depositor) to another Agent to create a liability to be repaid to the Depositor through an Act of Financial Withdrawal (derived from http://en.wikipedia.org/wiki/Deposit_(bank))</rdfs:comment>
    </owl:Class>
    


    <!-- http://www.cubrc.org/ontologies/KDD/Mid/EventOntology#ActOfFinancialInstrumentUse -->

    <owl:Class rdf:about="http://www.cubrc.org/ontologies/KDD/Mid/EventOntology#ActOfFinancialInstrumentUse">
        <rdfs:label rdf:datatype="&xsd;string">Act Of Financial Instrument Use</rdfs:label>
        <rdfs:subClassOf rdf:resource="http://www.cubrc.org/ontologies/KDD/Mid/EventOntology#ActOfInstrumentUse"/>
        <rdfs:comment rdf:datatype="&xsd;string">An Act Of Instrument Use in which some Agent uses some Financial Instrument</rdfs:comment>
    </owl:Class>
    


    <!-- http://www.cubrc.org/ontologies/KDD/Mid/EventOntology#ActOfFinancialWithdrawal -->

    <owl:Class rdf:about="http://www.cubrc.org/ontologies/KDD/Mid/EventOntology#ActOfFinancialWithdrawal">
        <rdfs:label rdf:datatype="&xsd;string">Act Of Financial Withdrawal</rdfs:label>
        <rdfs:subClassOf rdf:resource="http://www.cubrc.org/ontologies/KDD/Mid/EventOntology#ActOfFinancialInstrumentUse"/>
        <rdfs:comment rdf:datatype="&xsd;string">Definition: An Act of Financial Instrument Use wherein a Financial Instrument by Function or a Finanical Instrument by Role is transferred by an agent to another Agent (Depositor) from an account created by an earlier Act of Financial Deposit performed by the Depositor (derived from http://en.wikipedia.org/wiki/Deposit_(bank))</rdfs:comment>
    </owl:Class>
    


    <!-- http://www.cubrc.org/ontologies/KDD/Mid/EventOntology#ActOfFiresWarfighting -->

    <owl:Class rdf:about="http://www.cubrc.org/ontologies/KDD/Mid/EventOntology#ActOfFiresWarfighting">
        <rdfs:label>Realize the Fires Warfighting Function</rdfs:label>
        <rdfs:subClassOf rdf:resource="http://www.cubrc.org/ontologies/KDD/Mid/EventOntology#ActOfMilitaryForce"/>
        <rdfs:comment>Definition: An Act of Military Force from any of the related tasks and systems that provide collective and coordinated indirect fires, joint fires, and command and control warfare, including nonlethal fires, through the targeting process (derived from The Army Universal Task List FM 7-15 February 2009).</rdfs:comment>
    </owl:Class>
    


    <!-- http://www.cubrc.org/ontologies/KDD/Mid/EventOntology#ActOfForceDeployment -->

    <owl:Class rdf:about="http://www.cubrc.org/ontologies/KDD/Mid/EventOntology#ActOfForceDeployment">
        <rdfs:label>Force Deployment</rdfs:label>
        <rdfs:subClassOf rdf:resource="http://www.cubrc.org/ontologies/KDD/Mid/EventOntology#ActOfMovementAndManeuverWarfighting"/>
        <rdfs:comment>Definition: An Act of Military Force composed of Acts required to: prepare and move forces, move sustainment equipment, and move supplies within a theater of operations. This act involves the force as it task organizes, echelons and tailors itself for movement based on the mission, concept of operations, available lift, and other resources. This Act also includes instances of Redeployment wherein forces and materiel are transferred to support another joint force commander�s operational requirements, or to return personnel, equipment, and materiel to the home and/or demobilization stations for reintegration and/or out-processing. (derived from The Army Universal Task List FM 7-15 February 2009).</rdfs:comment>
    </owl:Class>
    


    <!-- http://www.cubrc.org/ontologies/KDD/Mid/EventOntology#ActOfForceManeuver -->

    <owl:Class rdf:about="http://www.cubrc.org/ontologies/KDD/Mid/EventOntology#ActOfForceManeuver">
        <rdfs:label>Force Maneuver</rdfs:label>
        <rdfs:subClassOf rdf:resource="http://www.cubrc.org/ontologies/KDD/Mid/EventOntology#ActOfMovementAndManeuverWarfighting"/>
        <rdfs:comment>Definition: An Act of Military Force in which some Force in an Area of Operation moves in combination with fires to achieve a position of advantage in respect to the enemy in order to accomplish the mission (derived from The Army Universal Task List FM 7-15 February 2009).</rdfs:comment>
    </owl:Class>
    


    <!-- http://www.cubrc.org/ontologies/KDD/Mid/EventOntology#ActOfForceMovement -->

    <owl:Class rdf:about="http://www.cubrc.org/ontologies/KDD/Mid/EventOntology#ActOfForceMovement">
        <rdfs:label>Force Movement</rdfs:label>
        <rdfs:subClassOf rdf:resource="http://www.cubrc.org/ontologies/KDD/Mid/EventOntology#ActOfMovementAndManeuverWarfighting"/>
        <rdfs:comment>Definition: An Act of Military Force in which some Force relocates or moves by any means or mode of transportation preparatory to deploying into combat formations to support tactical commander and joint force commander plans, including acts of generating and dispersing tactical forces (derived from The Army Universal Task List FM 7-15 February 2009).</rdfs:comment>
    </owl:Class>
    


    <!-- http://www.cubrc.org/ontologies/KDD/Mid/EventOntology#ActOfFoundingAnOrganization -->

    <owl:Class rdf:about="http://www.cubrc.org/ontologies/KDD/Mid/EventOntology#ActOfFoundingAnOrganization">
        <rdfs:label>Act of Founding an Organization</rdfs:label>
        <rdfs:subClassOf rdf:resource="http://www.cubrc.org/ontologies/KDD/Mid/EventOntology#ActOfDeclarativeCommunication"/>
        <rdfs:comment>Definition: An Act of Declarative Communication in which a Person or Group of Persons declares the start of an organization</rdfs:comment>
    </owl:Class>
    


    <!-- http://www.cubrc.org/ontologies/KDD/Mid/EventOntology#ActOfFratricideAvoidance -->

    <owl:Class rdf:about="http://www.cubrc.org/ontologies/KDD/Mid/EventOntology#ActOfFratricideAvoidance">
        <rdfs:label>Perform Fratricide Avoidance</rdfs:label>
        <rdfs:subClassOf rdf:resource="http://www.cubrc.org/ontologies/KDD/Mid/EventOntology#ActOfProtectionWarfighting"/>
        <rdfs:comment>Definition: An Act of Protection Warfighting which tends to lead to the prevention of the unintentional killing of friendly personnel by friendly firepower (derived from The Army Universal Task List FM 7-15 February 2009).</rdfs:comment>
    </owl:Class>
    


    <!-- http://www.cubrc.org/ontologies/KDD/Mid/EventOntology#ActOfFraud -->

    <owl:Class rdf:about="http://www.cubrc.org/ontologies/KDD/Mid/EventOntology#ActOfFraud">
        <rdfs:label>Act of Fraud</rdfs:label>
        <rdfs:subClassOf rdf:resource="http://www.cubrc.org/ontologies/KDD/Mid/EventOntology#CriminalActAgainstProperty"/>
        <rdfs:comment rdf:datatype="&xsd;string">Definition: A Criminal Act Against Property in which an intentional deception or misrepresentation made by a person with the knowledge that the deception could result in some unauthorized benefit to himself or some other person. It includes any act that constitutes fraud under applicable Federal or State law. (Source: http://www.gpo.gov/fdsys/pkg/CFR-2003-title42-vol3/xml/CFR-2003-title42-vol3-sec455-2.xml)</rdfs:comment>
    </owl:Class>
    


    <!-- http://www.cubrc.org/ontologies/KDD/Mid/EventOntology#ActOfFreightHandling -->

    <owl:Class rdf:about="http://www.cubrc.org/ontologies/KDD/Mid/EventOntology#ActOfFreightHandling">
        <rdfs:label xml:lang="en">ActOfFreightHandling</rdfs:label>
        <rdfs:subClassOf rdf:resource="http://www.cubrc.org/ontologies/KDD/Mid/EventOntology#ActOfFacilityUse"/>
    </owl:Class>
    


    <!-- http://www.cubrc.org/ontologies/KDD/Mid/EventOntology#ActOfFrontalAttack -->

    <owl:Class rdf:about="http://www.cubrc.org/ontologies/KDD/Mid/EventOntology#ActOfFrontalAttack">
        <rdfs:label>Conduct a Frontal Attack</rdfs:label>
        <rdfs:subClassOf rdf:resource="http://www.cubrc.org/ontologies/KDD/Mid/EventOntology#ActOfForceManeuver"/>
        <rdfs:comment>Definition: An Act of Force Maneuver in which the attacking force seeks to destroy a weaker enemy force or fix a larger enemy force in place over a broad front. At the tactical level, an attacking force can use a frontal attack to overrun a weaker enemy force rapidly. A frontal attack strikes the enemy across a wide front and over the most direct approaches.  (derived from The Army Universal Task List FM 7-15 February 2009).</rdfs:comment>
    </owl:Class>
    


    <!-- http://www.cubrc.org/ontologies/KDD/Mid/EventOntology#ActOfFunding -->

    <owl:Class rdf:about="http://www.cubrc.org/ontologies/KDD/Mid/EventOntology#ActOfFunding">
        <rdfs:label rdf:datatype="&xsd;string">Act of funding</rdfs:label>
        <rdfs:subClassOf rdf:resource="http://www.cubrc.org/ontologies/KDD/Mid/EventOntology#ActOfFinancialInstrumentUse"/>
        <rdfs:comment rdf:datatype="&xsd;string">Definition: An Act Of Financial Instrument Use in which an agent provides a sum of money to another agent for a particular purpose.</rdfs:comment>
    </owl:Class>
    


    <!-- http://www.cubrc.org/ontologies/KDD/Mid/EventOntology#ActOfGovernment -->

    <owl:Class rdf:about="http://www.cubrc.org/ontologies/KDD/Mid/EventOntology#ActOfGovernment">
        <rdfs:label xml:lang="en">ActOfGovernment</rdfs:label>
        <rdfs:subClassOf rdf:resource="http://www.cubrc.org/ontologies/KDD/Mid/EventOntology#IntentionalAct"/>
    </owl:Class>
    


    <!-- http://www.cubrc.org/ontologies/KDD/Mid/EventOntology#ActOfGovernmentSupport -->

    <owl:Class rdf:about="http://www.cubrc.org/ontologies/KDD/Mid/EventOntology#ActOfGovernmentSupport">
        <rdfs:label>Government Support</rdfs:label>
        <rdfs:subClassOf rdf:resource="http://www.cubrc.org/ontologies/KDD/Mid/EventOntology#ActOfCivilAffairs"/>
        <rdfs:comment>Definition: An Act of Civil Affairs that is an instance of either providing public safety support or public administration support (derived from The Army Universal Task List FM 7-15 February 2009).</rdfs:comment>
    </owl:Class>
    


    <!-- http://www.cubrc.org/ontologies/KDD/Mid/EventOntology#ActOfHealthServiceSupport -->

    <owl:Class rdf:about="http://www.cubrc.org/ontologies/KDD/Mid/EventOntology#ActOfHealthServiceSupport">
        <rdfs:label>Health Service Support</rdfs:label>
        <rdfs:subClassOf rdf:resource="http://www.cubrc.org/ontologies/KDD/Mid/EventOntology#ActOfSustainmentWarfighting"/>
        <rdfs:comment>Definition: An Act of Military Force that is an instance of any of the types of support and services performed, provided, and arranged by Medical Personnel to promote, improve, conserve, or restore the mental and physical wellbeing of Soldiers and, as directed, other personnel (derived from The Army Universal Task List FM 7-15 February 2009).</rdfs:comment>
    </owl:Class>
    


    <!-- http://www.cubrc.org/ontologies/KDD/Mid/EventOntology#ActOfHealthcareFraud -->

    <owl:Class rdf:about="http://www.cubrc.org/ontologies/KDD/Mid/EventOntology#ActOfHealthcareFraud">
        <rdfs:label>Act of Healthcare Fraud</rdfs:label>
        <rdfs:subClassOf rdf:resource="http://www.cubrc.org/ontologies/KDD/Mid/EventOntology#ActOfFraud"/>
    </owl:Class>
    


    <!-- http://www.cubrc.org/ontologies/KDD/Mid/EventOntology#ActOfHomicide -->

    <owl:Class rdf:about="http://www.cubrc.org/ontologies/KDD/Mid/EventOntology#ActOfHomicide">
        <rdfs:label rdf:datatype="&xsd;string">Act Of Homicide</rdfs:label>
        <rdfs:subClassOf rdf:resource="http://www.cubrc.org/ontologies/KDD/Mid/EventOntology#ActOfViolence"/>
        <rdfs:comment rdf:datatype="&xsd;string">An Act Of Violence which causes the unlawful killing of another person</rdfs:comment>
    </owl:Class>
    


    <!-- http://www.cubrc.org/ontologies/KDD/Mid/EventOntology#ActOfHumanLaborTrafficking -->

    <owl:Class rdf:about="http://www.cubrc.org/ontologies/KDD/Mid/EventOntology#ActOfHumanLaborTrafficking">
        <rdfs:subClassOf rdf:resource="http://www.cubrc.org/ontologies/KDD/Mid/EventOntology#ActOfHumanTrafficking"/>
        <rdfs:comment rdf:datatype="&xsd;string">Definition: An Act of Human Trafficking in which a person is recruited, harbored, transported, provisioned, or obtaininedfor labor or services, through the use of force, fraud or coercion for the purpose of subjection to involuntary servitude, peonage, debt bondage or slavery (Source: http://www.acf.hhs.gov/programs/orr/resource/fact-sheet-labor-trafficking-english)</rdfs:comment>
    </owl:Class>
    


    <!-- http://www.cubrc.org/ontologies/KDD/Mid/EventOntology#ActOfHumanSmuggling -->

    <owl:Class rdf:about="http://www.cubrc.org/ontologies/KDD/Mid/EventOntology#ActOfHumanSmuggling">
        <rdfs:subClassOf rdf:resource="http://www.cubrc.org/ontologies/KDD/Mid/EventOntology#ActOfSmuggling"/>
        <rdfs:comment rdf:datatype="&xsd;string">Definition: An Act of Smuggling in which people are imported into a country via the deliberate evasion of immigration laws. This includes bringing illegal aliens into a country, as well as the unlawful transportation and harboring of aliens already in a country illegally. (Source: http://www.ice.gov/human-smuggling/)</rdfs:comment>
    </owl:Class>
    


    <!-- http://www.cubrc.org/ontologies/KDD/Mid/EventOntology#ActOfHumanTrafficking -->

    <owl:Class rdf:about="http://www.cubrc.org/ontologies/KDD/Mid/EventOntology#ActOfHumanTrafficking">
        <rdfs:label rdf:datatype="&xsd;string">Act of Human Trafficking</rdfs:label>
        <rdfs:subClassOf rdf:resource="http://www.cubrc.org/ontologies/KDD/Mid/EventOntology#ActOfBlackMarketTrafficking"/>
        <rdfs:comment rdf:datatype="&xsd;string">Definition: An Act of Black Market Trafficking involving the illegal trade in Persons for the purposes of Prostitution or forced labor (derived from http:/en.wikipedia.org/wiki/Human_trafficking).</rdfs:comment>
    </owl:Class>
    


    <!-- http://www.cubrc.org/ontologies/KDD/Mid/EventOntology#ActOfIEDAndUXOProtectionOperation -->

    <owl:Class rdf:about="http://www.cubrc.org/ontologies/KDD/Mid/EventOntology#ActOfIEDAndUXOProtectionOperation">
        <rdfs:label>Conduct Improvised Explosive Device and Unexploded Ordnance Protection Operation</rdfs:label>
        <rdfs:subClassOf rdf:resource="http://www.cubrc.org/ontologies/KDD/Mid/EventOntology#ActOfProtectionWarfighting"/>
        <rdfs:comment>Definition: An Act of Protection Warfighting that includes reviewing base defense plans and bomb threat or search procedures, assisting in facility explosive hazard site surveys, and developing and implementing explosive ordnance disposal (EOD) emergency response plans and the antiterrorism or force protection plan. Provide training to emergency preparedness personnel on bomb threat search, improvised explosive device (IED) defeat techniques, unexploded explosive ordnance (UXO) identification, and marking procedures. Provide chemical, biological, radiological, nuclear, and high-yield explosives emergency response plans and facility site surveys to commanders. Provide EOD support to weapon storage site inspections. Provide EOD support to amnesty and weapon buyback programs (derived from The Army Universal Task List FM 7-15 February 2009).</rdfs:comment>
    </owl:Class>
    


    <!-- http://www.cubrc.org/ontologies/KDD/Mid/EventOntology#ActOfIdentification -->

    <owl:Class rdf:about="http://www.cubrc.org/ontologies/KDD/Mid/EventOntology#ActOfIdentification">
        <rdfs:label rdf:datatype="&xsd;string">Act Of Identification</rdfs:label>
        <rdfs:subClassOf rdf:resource="http://www.cubrc.org/ontologies/KDD/Mid/EventOntology#ActOfRepresentativeCommunication"/>
    </owl:Class>
    


    <!-- http://www.cubrc.org/ontologies/KDD/Mid/EventOntology#ActOfIllegalDrugTrafficking -->

    <owl:Class rdf:about="http://www.cubrc.org/ontologies/KDD/Mid/EventOntology#ActOfIllegalDrugTrafficking">
        <rdfs:label>Act Of Illegal Drug Trafficking</rdfs:label>
        <rdfs:subClassOf rdf:resource="http://www.cubrc.org/ontologies/KDD/Mid/EventOntology#ActOfDrugTrafficking"/>
        <rdfs:comment>Definition: An Act Of Drug Trafficking involving the cultivation, manufacture, distribution and sale of substances which are subject to drug prohibition laws. (derived from http://en.wikipedia.org/wiki/Illegal_drug_trade)</rdfs:comment>
    </owl:Class>
    


    <!-- http://www.cubrc.org/ontologies/KDD/Mid/EventOntology#ActOfIllegalEntry -->

    <owl:Class rdf:about="http://www.cubrc.org/ontologies/KDD/Mid/EventOntology#ActOfIllegalEntry">
        <rdfs:subClassOf rdf:resource="http://www.cubrc.org/ontologies/KDD/Mid/EventOntology#ActOfIllegalImmigration"/>
        <rdfs:comment rdf:datatype="&xsd;string">Definition: An Act of Illegal Imigration in which foreign nationals arrive in or cross the borders into a country in violation of its immigration law. (Source: http://en.wikipedia.org/wiki/Illegal_entry)</rdfs:comment>
    </owl:Class>
    


    <!-- http://www.cubrc.org/ontologies/KDD/Mid/EventOntology#ActOfIllegalImmigration -->

    <owl:Class rdf:about="http://www.cubrc.org/ontologies/KDD/Mid/EventOntology#ActOfIllegalImmigration">
        <rdfs:subClassOf rdf:resource="http://www.cubrc.org/ontologies/KDD/Mid/EventOntology#CriminalAct"/>
        <rdfs:comment rdf:datatype="&xsd;string">Definition: A Criminal Act in which persons migrate into a country in violation of the immigration laws of that country. United Nations signatories have agreed to exempt refugees from criminal charges upon such entry, which is in accordance with the Universal Declaration of Human Rights wherein is stated that &quot;Everyone has the right to seek and to enjoy in other countries asylum from persecution&quot;. (Source: http://en.wikipedia.org/wiki/Illegal_immigration)</rdfs:comment>
    </owl:Class>
    


    <!-- http://www.cubrc.org/ontologies/KDD/Mid/EventOntology#ActOfIlluminationFire -->

    <owl:Class rdf:about="http://www.cubrc.org/ontologies/KDD/Mid/EventOntology#ActOfIlluminationFire">
        <rdfs:label>Provide Illumination</rdfs:label>
        <rdfs:subClassOf rdf:resource="http://www.cubrc.org/ontologies/KDD/Mid/EventOntology#ActOfIndirectFire"/>
        <rdfs:comment>Definition: An Act of Indirect Fire in which illumination rounds are fired in order to support night operations or harass the enemy (derived from The Army Universal Task List FM 7-15 February 2009).</rdfs:comment>
    </owl:Class>
    


    <!-- http://www.cubrc.org/ontologies/KDD/Mid/EventOntology#ActOfImpeachment -->

    <owl:Class rdf:about="http://www.cubrc.org/ontologies/KDD/Mid/EventOntology#ActOfImpeachment">
        <rdfs:label>Act Of Impeachment</rdfs:label>
        <rdfs:subClassOf rdf:resource="http://www.cubrc.org/ontologies/KDD/Mid/EventOntology#CriminalTrial"/>
        <rdfs:comment>Definition: A Criminal Trial in which some public official is the defendant. (derived from http://www.id.uscourts.gov/glossary.htm)</rdfs:comment>
    </owl:Class>
    


    <!-- http://www.cubrc.org/ontologies/KDD/Mid/EventOntology#ActOfImprovisedExplosiveDeviceCache -->

    <owl:Class rdf:about="http://www.cubrc.org/ontologies/KDD/Mid/EventOntology#ActOfImprovisedExplosiveDeviceCache">
        <rdfs:label>Improvised Explosive Device Cache</rdfs:label>
        <rdfs:subClassOf rdf:resource="http://www.cubrc.org/ontologies/KDD/Mid/EventOntology#ActOfConductingImprovisedExplosiveDefeatOperation"/>
        <rdfs:comment>Definition: An Act of Conducting Improvised Explosive Defeat Operation in which the discovery and/or recovery of unarmed Improvised Explosive Devices, Improvised Explosive Device Components, or Explosive Ordnance in a permanent, fixed location occurs (derived from the Weapons Technical Intelligence (WTI) Improvised Explosive Device (IED) Lexicon 3rd Edition May 2010).</rdfs:comment>
    </owl:Class>
    


    <!-- http://www.cubrc.org/ontologies/KDD/Mid/EventOntology#ActOfImprovisedExplosiveDeviceFind -->

    <owl:Class rdf:about="http://www.cubrc.org/ontologies/KDD/Mid/EventOntology#ActOfImprovisedExplosiveDeviceFind">
        <rdfs:label>Improvised Explosive Device Find</rdfs:label>
        <rdfs:subClassOf rdf:resource="http://www.cubrc.org/ontologies/KDD/Mid/EventOntology#ActOfConductingImprovisedExplosiveDefeatOperation"/>
        <rdfs:comment>Definition: An Act of Conducting Improvised Explosive Defeat Operation in which the discovery or turn in of Improvised Explosive Device or Improvised Explosive Device Components in a temporary and/or transitory location occurs (derived from the Weapons Technical Intelligence (WTI) Improvised Explosive Device (IED) Lexicon 3rd Edition May 2010).</rdfs:comment>
    </owl:Class>
    


    <!-- http://www.cubrc.org/ontologies/KDD/Mid/EventOntology#ActOfIncarceration -->

    <owl:Class rdf:about="http://www.cubrc.org/ontologies/KDD/Mid/EventOntology#ActOfIncarceration">
        <rdfs:label>Act Of Incarceration</rdfs:label>
        <rdfs:subClassOf rdf:resource="http://www.cubrc.org/ontologies/KDD/Mid/EventOntology#LegalSystemAct"/>
        <rdfs:comment>Definition: A Legal System Act in which a person convicted of having committed a Criminal Act is imprisoned in a jail or penitentiary. (derived from http://www.id.uscourts.gov/glossary.htm)</rdfs:comment>
    </owl:Class>
    


    <!-- http://www.cubrc.org/ontologies/KDD/Mid/EventOntology#ActOfIndictment -->

    <owl:Class rdf:about="http://www.cubrc.org/ontologies/KDD/Mid/EventOntology#ActOfIndictment">
        <rdfs:label>Act Of Indictment</rdfs:label>
        <rdfs:subClassOf rdf:resource="http://www.cubrc.org/ontologies/KDD/Mid/EventOntology#ActOfRepresentativeCommunication"/>
        <rdfs:comment>Definition: An Act of Representative Communication that is a formal accusation that a person has committed a crime (derived from http://en.wikipedia.org/wiki/Indictment)</rdfs:comment>
    </owl:Class>
    


    <!-- http://www.cubrc.org/ontologies/KDD/Mid/EventOntology#ActOfIndirectFire -->

    <owl:Class rdf:about="http://www.cubrc.org/ontologies/KDD/Mid/EventOntology#ActOfIndirectFire">
        <rdfs:label>Indirect Fire</rdfs:label>
        <rdfs:subClassOf rdf:resource="http://www.cubrc.org/ontologies/KDD/Mid/EventOntology#ActOfFiresWarfighting"/>
        <rdfs:comment>Definition: An Act of Military Force in which weapon systems are aimed and fired towards targets without reliance upon a direct line of sight between the weapon system and the target (derived from The Army Universal Task List FM 7-15 February 2009).</rdfs:comment>
    </owl:Class>
    


    <!-- http://www.cubrc.org/ontologies/KDD/Mid/EventOntology#ActOfInfiltrationManeuver -->

    <owl:Class rdf:about="http://www.cubrc.org/ontologies/KDD/Mid/EventOntology#ActOfInfiltrationManeuver">
        <rdfs:label>Conduct an Infiltration</rdfs:label>
        <rdfs:subClassOf rdf:resource="http://www.cubrc.org/ontologies/KDD/Mid/EventOntology#ActOfForceManeuver"/>
        <rdfs:comment>Definition: An Act of Force Maneuver in which an attacking force conducts undetected movement through or into an area occupied by enemy forces to occupy a position of advantage while exposing only small elements to enemy defensive fires (derived from The Army Universal Task List FM 7-15 February 2009).</rdfs:comment>
    </owl:Class>
    


    <!-- http://www.cubrc.org/ontologies/KDD/Mid/EventOntology#ActOfInformationProtection -->

    <owl:Class rdf:about="http://www.cubrc.org/ontologies/KDD/Mid/EventOntology#ActOfInformationProtection">
        <rdfs:label>Conduct Information Protection</rdfs:label>
        <rdfs:subClassOf rdf:resource="http://www.cubrc.org/ontologies/KDD/Mid/EventOntology#ActOfProtectionWarfighting"/>
        <rdfs:comment>Definition: An Act of Protection Warfighting that includes either active or passive measures that protect and defend friendly information and information systems to ensure timely, accurate, and relevant friendly information. It denies enemies, adversaries, and others the opportunity to exploit friendly information and information systems for their own purposes (derived from The Army Universal Task List FM 7-15 February 2009).</rdfs:comment>
    </owl:Class>
    


    <!-- http://www.cubrc.org/ontologies/KDD/Mid/EventOntology#ActOfInformationSuperiorityTaskIntegration -->

    <owl:Class rdf:about="http://www.cubrc.org/ontologies/KDD/Mid/EventOntology#ActOfInformationSuperiorityTaskIntegration">
        <rdfs:label>Integrate Information Superiority Contributors</rdfs:label>
        <rdfs:subClassOf rdf:resource="http://www.cubrc.org/ontologies/KDD/Mid/EventOntology#ActOfCommandAndControlWarfighting"/>
        <rdfs:comment>Definition: An Act of Command and Control Warfighting in which commanders integrate information tasks; intelligence, surveillance, and reconnaissance (ISR); knowledge management; and information management in order to achieve information superiority over the enemy  (derived from The Army Universal Task List FM 7-15 February 2009).</rdfs:comment>
    </owl:Class>
    


    <!-- http://www.cubrc.org/ontologies/KDD/Mid/EventOntology#ActOfInfrastructureSupport -->

    <owl:Class rdf:about="http://www.cubrc.org/ontologies/KDD/Mid/EventOntology#ActOfInfrastructureSupport">
        <rdfs:label>Infrastructure Support</rdfs:label>
        <rdfs:subClassOf rdf:resource="http://www.cubrc.org/ontologies/KDD/Mid/EventOntology#ActOfCivilAffairs"/>
        <rdfs:comment>Definition: An Act of Civil Affairs that includes instances of any of the following types of action: providing public communications support, public transportation support and public works and facilities support (derived from The Army Universal Task List FM 7-15 February 2009).</rdfs:comment>
    </owl:Class>
    


    <!-- http://www.cubrc.org/ontologies/KDD/Mid/EventOntology#ActOfInhabitancy -->

    <owl:Class rdf:about="http://www.cubrc.org/ontologies/KDD/Mid/EventOntology#ActOfInhabitancy">
        <rdfs:label rdf:datatype="&xsd;string">Act of Inhabitancy</rdfs:label>
        <rdfs:subClassOf rdf:resource="http://www.cubrc.org/ontologies/KDD/Mid/EventOntology#IntentionalAct"/>
        <rdfs:comment rdf:datatype="&xsd;string">An Intentional Act of dwelling in a location.</rdfs:comment>
    </owl:Class>
    


    <!-- http://www.cubrc.org/ontologies/KDD/Mid/EventOntology#ActOfInstrumentUse -->

    <owl:Class rdf:about="http://www.cubrc.org/ontologies/KDD/Mid/EventOntology#ActOfInstrumentUse">
        <rdfs:label rdf:datatype="&xsd;string">Act Of Instrument Use</rdfs:label>
        <rdfs:subClassOf rdf:resource="http://www.cubrc.org/ontologies/KDD/Mid/EventOntology#ActOfArtifactEmployment"/>
        <rdfs:comment rdf:datatype="&xsd;string">An Act Of Artifact Employment in which some Agent uses some Instrument.</rdfs:comment>
    </owl:Class>
    


    <!-- http://www.cubrc.org/ontologies/KDD/Mid/EventOntology#ActOfIntellectualPropertyRightsTheft -->

    <owl:Class rdf:about="http://www.cubrc.org/ontologies/KDD/Mid/EventOntology#ActOfIntellectualPropertyRightsTheft">
        <rdfs:subClassOf rdf:resource="http://www.cubrc.org/ontologies/KDD/Mid/EventOntology#ActOfLarceny"/>
        <rdfs:comment rdf:datatype="&xsd;string">Definition: An Act of Larceny that violates criminal laws that protect copyrights, patents, trademarks, other forms of intellectual property, and trade secrets, both in the United States and abroad. (Source: https://www.bja.gov/ProgramDetails.aspx?Program_ID=64)</rdfs:comment>
    </owl:Class>
    


    <!-- http://www.cubrc.org/ontologies/KDD/Mid/EventOntology#ActOfIntelligenceGathering -->

    <owl:Class rdf:about="http://www.cubrc.org/ontologies/KDD/Mid/EventOntology#ActOfIntelligenceGathering">
        <rdfs:label rdf:datatype="&xsd;string">Act Of Intelligence Gathering</rdfs:label>
        <rdfs:subClassOf rdf:resource="http://www.cubrc.org/ontologies/KDD/Mid/EventOntology#IntentionalAct"/>
        <rdfs:comment rdf:datatype="&xsd;string">Definition: An Intentional Act of producing and/or gathering information by a government or other Organization to guide decisions and actions by answering questions or obtaining advance warning of events and movements deemed to be important or otherwise relevant. (derived from http://en.wikipedia.org/wiki/Intelligence_(information_gathering)</rdfs:comment>
    </owl:Class>
    


    <!-- http://www.cubrc.org/ontologies/KDD/Mid/EventOntology#ActOfIntelligencePreparationOfTheBattlefield -->

    <owl:Class rdf:about="http://www.cubrc.org/ontologies/KDD/Mid/EventOntology#ActOfIntelligencePreparationOfTheBattlefield">
        <rdfs:label>Intelligence Preparation of the Battlefield</rdfs:label>
        <rdfs:subClassOf rdf:resource="http://www.cubrc.org/ontologies/KDD/Mid/EventOntology#ActOfIntelligenceSupportToSituationalUnderstanding"/>
        <rdfs:comment>Definition: An Act of Intelligence Support in which information and intelligence about the operational environment and the options it presents to friendly and threat forces is generated. Intelligence preparation of the battlefield (IPB) is a systematic process of analyzing and visualizing the portions of the mission variables of enemy, terrain, weather, and civil considerations in a specific geographic area and for each additional mission  (derived from The Army Universal Task List FM 7-15 February 2009).</rdfs:comment>
    </owl:Class>
    


    <!-- http://www.cubrc.org/ontologies/KDD/Mid/EventOntology#ActOfIntelligenceSupportToForceGeneration -->

    <owl:Class rdf:about="http://www.cubrc.org/ontologies/KDD/Mid/EventOntology#ActOfIntelligenceSupportToForceGeneration">
        <rdfs:label>Intelligence Support to Force Generation</rdfs:label>
        <rdfs:subClassOf rdf:resource="http://www.cubrc.org/ontologies/KDD/Mid/EventOntology#ActOfMilitaryIntelligence"/>
        <rdfs:comment>Definition: An Act of Military Intelligence in which knowledge concerning an area of interest is generated, facilitating future intelligence operations, and tailoring the force. It includes establishing intelligence communication architecture and knowledge management  (derived from The Army Universal Task List FM 7-15 February 2009).</rdfs:comment>
    </owl:Class>
    


    <!-- http://www.cubrc.org/ontologies/KDD/Mid/EventOntology#ActOfIntelligenceSupportToSituationalUnderstanding -->

    <owl:Class rdf:about="http://www.cubrc.org/ontologies/KDD/Mid/EventOntology#ActOfIntelligenceSupportToSituationalUnderstanding">
        <rdfs:label>Intelligence Support to Situational Understanding</rdfs:label>
        <rdfs:subClassOf rdf:resource="http://www.cubrc.org/ontologies/KDD/Mid/EventOntology#ActOfMilitaryIntelligence"/>
        <rdfs:comment>Definition: An Act of Military Intelligence in which information and intelligence is provided to commanders to assist them in achieving a clear understanding of the force�s current state with relation to the enemy and the environment (derived from The Army Universal Task List FM 7-15 February 2009).</rdfs:comment>
    </owl:Class>
    


    <!-- http://www.cubrc.org/ontologies/KDD/Mid/EventOntology#ActOfIntelligenceSupportToTargeting -->

    <owl:Class rdf:about="http://www.cubrc.org/ontologies/KDD/Mid/EventOntology#ActOfIntelligenceSupportToTargeting">
        <rdfs:label>Targeting Intelligence Support</rdfs:label>
        <rdfs:subClassOf rdf:resource="http://www.cubrc.org/ontologies/KDD/Mid/EventOntology#ActOfMilitaryIntelligence"/>
        <rdfs:comment>Definition: An Act of Military Intelligence in which the commander is provided information and intelligence support for targeting through lethal and nonlethal actions, including intelligence support to the planning and execution of direct and indirect fires, command and control warfare  information engagement, and individual capabilities of information and knowledge management as well as assessing the effects of those operations (derived from The Army Universal Task List FM 7-15 February 2009).</rdfs:comment>
    </owl:Class>
    


    <!-- http://www.cubrc.org/ontologies/KDD/Mid/EventOntology#ActOfIntelligenceSurveillanceAndReconnaisance -->

    <owl:Class rdf:about="http://www.cubrc.org/ontologies/KDD/Mid/EventOntology#ActOfIntelligenceSurveillanceAndReconnaisance">
        <rdfs:label>Perform Intelligence Surveillance and Reconnaisance</rdfs:label>
        <rdfs:subClassOf rdf:resource="http://www.cubrc.org/ontologies/KDD/Mid/EventOntology#ActOfMilitaryIntelligence"/>
        <rdfs:comment>Definition: An Act of Military Intelligence that synchronizes and integrates the planning and operation of sensors, assets, and processing, exploitation, and dissemination systems in direct support of current and future operations  (derived from The Army Universal Task List FM 7-15 February 2009).</rdfs:comment>
    </owl:Class>
    


    <!-- http://www.cubrc.org/ontologies/KDD/Mid/EventOntology#ActOfInternment -->

    <owl:Class rdf:about="http://www.cubrc.org/ontologies/KDD/Mid/EventOntology#ActOfInternment">
        <rdfs:label>Conduct Internment Resettlement Operations</rdfs:label>
        <rdfs:subClassOf rdf:resource="http://www.cubrc.org/ontologies/KDD/Mid/EventOntology#ActOfSustainmentWarfighting"/>
        <rdfs:comment>Definition: An Act of Military Force  in which a Person in the custody of U.S. forces who has not been classified according to the Geneva Convention as an enemy prisoner of war (EPW), a retained personnel, or a civilian internee is treated as an EPW until a legal status is ascertained by competent authority. This includes activities performed by units when they are responsible for interning enemy combatants, retained persons and civilian detainees or other support to displaced civilians. It ensures the safety and humane treatment of the incarcerated individuals, the maintenance of law and order in the facilities, as well as the safety of guards and the surrounding civilian and military facilities and installations (derived from The Army Universal Task List FM 7-15 February 2009).</rdfs:comment>
    </owl:Class>
    


    <!-- http://www.cubrc.org/ontologies/KDD/Mid/EventOntology#ActOfInterpersonalRelationship -->

    <owl:Class rdf:about="http://www.cubrc.org/ontologies/KDD/Mid/EventOntology#ActOfInterpersonalRelationship">
        <rdfs:label rdf:datatype="&xsd;string">Act of Interpersonal Relationship</rdfs:label>
        <rdfs:subClassOf rdf:resource="http://www.cubrc.org/ontologies/KDD/Mid/EventOntology#ActOfAssociation"/>
        <rdfs:comment rdf:datatype="&xsd;string">Definition: An Act of Association between two or more Persons that may range from fleeting to enduring. (derived from http://en.wikipedia.org/wiki/Interpersonal_relationship)</rdfs:comment>
    </owl:Class>
    


    <!-- http://www.cubrc.org/ontologies/KDD/Mid/EventOntology#ActOfInviting -->

    <owl:Class rdf:about="http://www.cubrc.org/ontologies/KDD/Mid/EventOntology#ActOfInviting">
        <rdfs:label rdf:datatype="&xsd;string">Act Of Inviting</rdfs:label>
        <rdfs:subClassOf rdf:resource="http://www.cubrc.org/ontologies/KDD/Mid/EventOntology#ActOfCommissiveCommunication"/>
    </owl:Class>
    


    <!-- http://www.cubrc.org/ontologies/KDD/Mid/EventOntology#ActOfInvoluntaryManslaughter -->

    <owl:Class rdf:about="http://www.cubrc.org/ontologies/KDD/Mid/EventOntology#ActOfInvoluntaryManslaughter">
        <rdfs:label>Act Of Involuntary Manslaughter</rdfs:label>
        <rdfs:subClassOf rdf:resource="http://www.cubrc.org/ontologies/KDD/Mid/EventOntology#ActOfManslaughter"/>
        <rdfs:comment>Definition: An Act of Manslaughter that occurs without malice aforethought. (derived from http://en.wikipedia.org/wiki/Manslaughter)</rdfs:comment>
    </owl:Class>
    


    <!-- http://www.cubrc.org/ontologies/KDD/Mid/EventOntology#ActOfIssuingMassMediaArticle -->

    <owl:Class rdf:about="http://www.cubrc.org/ontologies/KDD/Mid/EventOntology#ActOfIssuingMassMediaArticle">
        <rdfs:label>Act Of Issuing Mass Media Article</rdfs:label>
        <rdfs:subClassOf rdf:resource="http://www.cubrc.org/ontologies/KDD/Mid/EventOntology#ActOfMassMediaCommunication"/>
        <rdfs:comment>Definition: An Act Of Mass Media Communication involving the sending forth or putting into circulation a non-fictional essay, especially one included with others in a newspaper, magazine, or journal. (derived from JC3IEDM-MIRD-DMWG-Edition_3.0.2_20090514).</rdfs:comment>
    </owl:Class>
    


    <!-- http://www.cubrc.org/ontologies/KDD/Mid/EventOntology#ActOfIssuingMassMediaDocumentary -->

    <owl:Class rdf:about="http://www.cubrc.org/ontologies/KDD/Mid/EventOntology#ActOfIssuingMassMediaDocumentary">
        <rdfs:label>Act Of Issuing Mass Media Documentary</rdfs:label>
        <rdfs:subClassOf rdf:resource="http://www.cubrc.org/ontologies/KDD/Mid/EventOntology#ActOfMassMediaCommunication"/>
        <rdfs:comment>Definition: An Act Of Mass Media Communication involiving the the sending forth or putting into circulation information that provides a factual record or report. (derived from JC3IEDM-MIRD-DMWG-Edition_3.0.2_20090514)</rdfs:comment>
    </owl:Class>
    


    <!-- http://www.cubrc.org/ontologies/KDD/Mid/EventOntology#ActOfIssuingMassMediaPressRelease -->

    <owl:Class rdf:about="http://www.cubrc.org/ontologies/KDD/Mid/EventOntology#ActOfIssuingMassMediaPressRelease">
        <rdfs:label>Act Of Issuing Mass Media Press Release</rdfs:label>
        <rdfs:subClassOf rdf:resource="http://www.cubrc.org/ontologies/KDD/Mid/EventOntology#ActOfMassMediaCommunication"/>
        <rdfs:comment>Definition: An Act Of Mass Media Communication involving the sending forth or putting into circulation an official statement issued to media for information. (derived from JC3IEDM-MIRD-DMWG-Edition_3.0.2_20090514)</rdfs:comment>
    </owl:Class>
    


    <!-- http://www.cubrc.org/ontologies/KDD/Mid/EventOntology#ActOfKidnapping -->

    <owl:Class rdf:about="http://www.cubrc.org/ontologies/KDD/Mid/EventOntology#ActOfKidnapping">
        <rdfs:label rdf:datatype="&xsd;string">Act Of Kidnapping</rdfs:label>
        <rdfs:subClassOf rdf:resource="http://www.cubrc.org/ontologies/KDD/Mid/EventOntology#ActOfViolence"/>
        <rdfs:subClassOf rdf:resource="http://www.cubrc.org/ontologies/KDD/Mid/EventOntology#CriminalActAgainstThePerson"/>
        <rdfs:comment rdf:datatype="&xsd;string">An Act Of Violence in which a person is taken away or transported against the person&apos;s will, usually to hold the person in false imprisonment, a confinement without legal authority (derived from http://en.wikipeidia.org/wiki/Kidnapping).</rdfs:comment>
    </owl:Class>
    


    <!-- http://www.cubrc.org/ontologies/KDD/Mid/EventOntology#ActOfLading -->

    <owl:Class rdf:about="http://www.cubrc.org/ontologies/KDD/Mid/EventOntology#ActOfLading">
        <rdfs:label xml:lang="en">ActOfLading</rdfs:label>
        <rdfs:subClassOf rdf:resource="http://www.cubrc.org/ontologies/KDD/Mid/EventOntology#ActOfFreightHandling"/>
    </owl:Class>
    


    <!-- http://www.cubrc.org/ontologies/KDD/Mid/EventOntology#ActOfLarceny -->

    <owl:Class rdf:about="http://www.cubrc.org/ontologies/KDD/Mid/EventOntology#ActOfLarceny">
        <rdfs:label>Act Of Larceny</rdfs:label>
        <rdfs:subClassOf rdf:resource="http://www.cubrc.org/ontologies/KDD/Mid/EventOntology#CriminalActAgainstProperty"/>
        <rdfs:comment>Definition: A Criminal Act Against Property involving the wrongful acquisition of the personal property of another person. (derived from http://en.wikipedia.org/wiki/Larceny). Comment: Also known as Theft.</rdfs:comment>
    </owl:Class>
    


    <!-- http://www.cubrc.org/ontologies/KDD/Mid/EventOntology#ActOfLegalInstrumentUse -->

    <owl:Class rdf:about="http://www.cubrc.org/ontologies/KDD/Mid/EventOntology#ActOfLegalInstrumentUse">
        <rdfs:label rdf:datatype="&xsd;string">Act Of Legal Instrument Use</rdfs:label>
        <rdfs:subClassOf rdf:resource="http://www.cubrc.org/ontologies/KDD/Mid/EventOntology#ActOfInstrumentUse"/>
        <rdfs:comment rdf:datatype="&xsd;string">An Act Of Instrument Use in which some Agent uses some Legal Instrument</rdfs:comment>
    </owl:Class>
    


    <!-- http://www.cubrc.org/ontologies/KDD/Mid/EventOntology#ActOfLethalDirectFire -->

    <owl:Class rdf:about="http://www.cubrc.org/ontologies/KDD/Mid/EventOntology#ActOfLethalDirectFire">
        <rdfs:label>Lethal Direct Fire</rdfs:label>
        <rdfs:subClassOf rdf:resource="http://www.cubrc.org/ontologies/KDD/Mid/EventOntology#ActOfDirectFire"/>
        <rdfs:comment>Definition: An Act of Direct Fire in which some Force engages enemy equipment and materiel, personnel, fortifications, and facilities with direct fire designed to destroy the target; the direct fires may be from fixed- or rotary-wing systems (derived from The Army Universal Task List FM 7-15 February 2009).</rdfs:comment>
    </owl:Class>
    


    <!-- http://www.cubrc.org/ontologies/KDD/Mid/EventOntology#ActOfLinkUpWithTacticalForce -->

    <owl:Class rdf:about="http://www.cubrc.org/ontologies/KDD/Mid/EventOntology#ActOfLinkUpWithTacticalForce">
        <rdfs:label>Link Up with Other Tactical Forces</rdfs:label>
        <rdfs:subClassOf rdf:resource="http://www.cubrc.org/ontologies/KDD/Mid/EventOntology#ActOfForceManeuver"/>
        <rdfs:comment>Definition: An Act of Force Maneuver that occurs when friendly forces meet in an Area of Operations including circumstances such as: an advancing force reaches an objective area previously seized by an airborne or air assault force; when an encircled element breaks out to rejoin friendly forces or a force comes to the relief of an encircled force; and when converging maneuver forces meet. Forces may be moving toward each other, or one may be stationary (derived from The Army Universal Task List FM 7-15 February 2009).</rdfs:comment>
    </owl:Class>
    


    <!-- http://www.cubrc.org/ontologies/KDD/Mid/EventOntology#ActOfLoaning -->

    <owl:Class rdf:about="http://www.cubrc.org/ontologies/KDD/Mid/EventOntology#ActOfLoaning">
        <rdfs:label rdf:datatype="&xsd;string">Act Of Loaning</rdfs:label>
        <rdfs:subClassOf rdf:resource="http://www.cubrc.org/ontologies/KDD/Mid/EventOntology#ActOfFinancialInstrumentUse"/>
        <rdfs:comment rdf:datatype="&xsd;string">Definition: An Act of Financial Instrument Use wherein a Financial Instrument by Function or a Finanical Instrument by Role is given by an agent (Creditor) to another Agent (Debtor) in order to receive Repayments from the Debtor which are of greater Financial Value (derived from http://en.wikipedia.org/wiki/Loan).</rdfs:comment>
    </owl:Class>
    


    <!-- http://www.cubrc.org/ontologies/KDD/Mid/EventOntology#ActOfLogisticSupport -->

    <owl:Class rdf:about="http://www.cubrc.org/ontologies/KDD/Mid/EventOntology#ActOfLogisticSupport">
        <rdfs:label>Logistics</rdfs:label>
        <rdfs:subClassOf rdf:resource="http://www.cubrc.org/ontologies/KDD/Mid/EventOntology#ActOfSustainmentWarfighting"/>
        <rdfs:comment>Definition: An Act of Military Force which including either the design, development, acquisition, fielding, and maintenance of equipment and systems (derived from The Army Universal Task List FM 7-15 February 2009).</rdfs:comment>
    </owl:Class>
    


    <!-- http://www.cubrc.org/ontologies/KDD/Mid/EventOntology#ActOfMaintainingCommunityRelations -->

    <owl:Class rdf:about="http://www.cubrc.org/ontologies/KDD/Mid/EventOntology#ActOfMaintainingCommunityRelations">
        <rdfs:label>Maintain Community Relations</rdfs:label>
        <rdfs:subClassOf rdf:resource="http://www.cubrc.org/ontologies/KDD/Mid/EventOntology#ActOfPublicAffairsOperation"/>
        <rdfs:comment>Definition: An Act of Public Affairs which assists in conducting (planning, preparing, executing, and assessing) community relations programs as resources permit. It includes the conduct of programs to establish and sustain mutually beneficial relationships with the public, focusing on communities neighboring, or directly affected by Army activities (derived from The Army Universal Task List FM 7-15 February 2009).</rdfs:comment>
    </owl:Class>
    


    <!-- http://www.cubrc.org/ontologies/KDD/Mid/EventOntology#ActOfMaintenanceSupport -->

    <owl:Class rdf:about="http://www.cubrc.org/ontologies/KDD/Mid/EventOntology#ActOfMaintenanceSupport">
        <rdfs:label>Maintenance Support</rdfs:label>
        <rdfs:subClassOf rdf:resource="http://www.cubrc.org/ontologies/KDD/Mid/EventOntology#ActOfLogisticSupport"/>
        <rdfs:comment>Definition: An Act of Logistic Support in which weapon systems and equipment are kept available for use through repair and/or scheduled maintainenace  (derived from The Army Universal Task List FM 7-15 February 2009).</rdfs:comment>
    </owl:Class>
    


    <!-- http://www.cubrc.org/ontologies/KDD/Mid/EventOntology#ActOfMalfeasanceInOffice -->

    <owl:Class rdf:about="http://www.cubrc.org/ontologies/KDD/Mid/EventOntology#ActOfMalfeasanceInOffice">
        <rdfs:label>Act Of Malfeasance In Office</rdfs:label>
        <rdfs:subClassOf rdf:resource="http://www.cubrc.org/ontologies/KDD/Mid/EventOntology#CriminalActAgainstJustice"/>
        <rdfs:comment>Definition: A Criminal Act Against Justice commission of an unlawful act, done in an official capacity, which affects the performance of official duties (derived from http://en.wikipedia.org/wiki/Malfeasance_in_office).</rdfs:comment>
    </owl:Class>
    


    <!-- http://www.cubrc.org/ontologies/KDD/Mid/EventOntology#ActOfManslaughter -->

    <owl:Class rdf:about="http://www.cubrc.org/ontologies/KDD/Mid/EventOntology#ActOfManslaughter">
        <rdfs:label>Act Of Manslaughter</rdfs:label>
        <rdfs:subClassOf rdf:resource="http://www.cubrc.org/ontologies/KDD/Mid/EventOntology#ActOfCriminalHomicide"/>
        <rdfs:comment>Definition: An Act of Criminal Homicide that involves the killing of a human being, in a manner considered by law as less culpable than murder (derived from http://en.wikipedia.org/wiki/Manslaughter)</rdfs:comment>
    </owl:Class>
    


    <!-- http://www.cubrc.org/ontologies/KDD/Mid/EventOntology#ActOfMarrying -->

    <owl:Class rdf:about="http://www.cubrc.org/ontologies/KDD/Mid/EventOntology#ActOfMarrying">
        <rdfs:label rdf:datatype="&xsd;string">Act of Marrying</rdfs:label>
        <rdfs:subClassOf rdf:resource="http://www.cubrc.org/ontologies/KDD/Mid/EventOntology#LegalSystemAct"/>
        <rdfs:subClassOf>
            <owl:Restriction>
                <owl:onProperty rdf:resource="http://www.obofoundry.org/ro/ro.owl#precedes"/>
                <owl:someValuesFrom rdf:resource="http://www.cubrc.org/ontologies/KDD/Mid/EventOntology#Marriage"/>
            </owl:Restriction>
        </rdfs:subClassOf>
        <rdfs:comment rdf:datatype="&xsd;string">Definition: A Legal System Act that establishes a Marriage between two people (derived from http://en.wikipedia.org/wiki/Marriage)</rdfs:comment>
    </owl:Class>
    


    <!-- http://www.cubrc.org/ontologies/KDD/Mid/EventOntology#ActOfMassMediaCommunication -->

    <owl:Class rdf:about="http://www.cubrc.org/ontologies/KDD/Mid/EventOntology#ActOfMassMediaCommunication">
        <rdfs:label>Act Of Mass Media Communication</rdfs:label>
        <rdfs:subClassOf rdf:resource="http://www.cubrc.org/ontologies/KDD/Mid/EventOntology#ActOfCommunication"/>
        <rdfs:comment>Definition: An Act of Communication intended to reach a large audience using a medium such as the internet, television, radio, newspaper, and magazine. (derived from http://en.wikipedia.org/wiki/The_media</rdfs:comment>
    </owl:Class>
    


    <!-- http://www.cubrc.org/ontologies/KDD/Mid/EventOntology#ActOfMediaOperation -->

    <owl:Class rdf:about="http://www.cubrc.org/ontologies/KDD/Mid/EventOntology#ActOfMediaOperation">
        <rdfs:label>Media Operation</rdfs:label>
        <rdfs:subClassOf rdf:resource="http://www.cubrc.org/ontologies/KDD/Mid/EventOntology#ActOfPublicAffairsOperation"/>
        <rdfs:comment>Definition: An Act of Public Affairs which provides assistance to media that is covering operations; including assisting media on coverage ground rules; arranging interviews and briefings; coordinating unit visits and escorts; and providing assistance in arranging transportation, messing, billeting, communications support, protective equipment, and medical care (derived from The Army Universal Task List FM 7-15 February 2009).</rdfs:comment>
    </owl:Class>
    


    <!-- http://www.cubrc.org/ontologies/KDD/Mid/EventOntology#ActOfMedicalEvacuation -->

    <owl:Class rdf:about="http://www.cubrc.org/ontologies/KDD/Mid/EventOntology#ActOfMedicalEvacuation">
        <rdfs:label>Medical Evacuation</rdfs:label>
        <rdfs:subClassOf rdf:resource="http://www.cubrc.org/ontologies/KDD/Mid/EventOntology#ActOfHealthServiceSupport"/>
        <rdfs:comment>Definition: An Act of Health Service Support in which direct and area air and ground medical evacuation (MEDEVAC) is provided to; evacuate sick, injured, or wounded personnel (U.S. joint, interagency, and multinational forces; enemy prisoners of war; detained or retained personnel; and when authorized civilian personnel) from the point of injury or wounding, casualty collection points, battalion aid stations, ambulance exchange points, or any other designated points where casualties have been located to be evacuated to a higher level medical treatment facility (MTF) in the area of operations (AO)  (derived from The Army Universal Task List FM 7-15 February 2009).</rdfs:comment>
    </owl:Class>
    


    <!-- http://www.cubrc.org/ontologies/KDD/Mid/EventOntology#ActOfMedicalTreatmentInAreaOfOperations -->

    <owl:Class rdf:about="http://www.cubrc.org/ontologies/KDD/Mid/EventOntology#ActOfMedicalTreatmentInAreaOfOperations">
        <rdfs:label>Medical Treatment</rdfs:label>
        <rdfs:subClassOf rdf:resource="http://www.cubrc.org/ontologies/KDD/Mid/EventOntology#ActOfHealthServiceSupport"/>
        <rdfs:comment>Definition: An Act of Health Service Support in which medical treatment (organic and area support) is provided for all units in the area of operations (AO), such an act may include the examination and stabilization of patients,  evaluation of wounds, disease and nonbattle injuries, and the determination of treatment and medical evacuation precedence (derived from The Army Universal Task List FM 7-15 February 2009).</rdfs:comment>
    </owl:Class>
    


    <!-- http://www.cubrc.org/ontologies/KDD/Mid/EventOntology#ActOfMeeting -->

    <owl:Class rdf:about="http://www.cubrc.org/ontologies/KDD/Mid/EventOntology#ActOfMeeting">
        <rdfs:label rdf:datatype="&xsd;string">Act of Meeting</rdfs:label>
        <rdfs:subClassOf rdf:resource="http://www.cubrc.org/ontologies/KDD/Mid/EventOntology#ActOfAssociation"/>
        <rdfs:comment rdf:datatype="&xsd;string">Definition: An Act of Association wherein two or more Persons assemble for some common purpose. (http://wordnetweb.princeton.edu/perl/webwn?s=meet) (Sense Key: meet%2:41:00, get together%2:41:00)</rdfs:comment>
    </owl:Class>
    


    <!-- http://www.cubrc.org/ontologies/KDD/Mid/EventOntology#ActOfMilitaryForce -->

    <owl:Class rdf:about="http://www.cubrc.org/ontologies/KDD/Mid/EventOntology#ActOfMilitaryForce">
        <rdfs:label rdf:datatype="&xsd;string">ActOfMilitaryForce</rdfs:label>
        <rdfs:subClassOf rdf:resource="http://www.cubrc.org/ontologies/KDD/Mid/EventOntology#IntentionalAct"/>
    </owl:Class>
    


    <!-- http://www.cubrc.org/ontologies/KDD/Mid/EventOntology#ActOfMilitaryIntelligence -->

    <owl:Class rdf:about="http://www.cubrc.org/ontologies/KDD/Mid/EventOntology#ActOfMilitaryIntelligence">
        <rdfs:label>Military Intelligence</rdfs:label>
        <rdfs:subClassOf rdf:resource="http://www.cubrc.org/ontologies/KDD/Mid/EventOntology#ActOfMilitaryForce"/>
        <rdfs:comment>Definition: An Act of Military Force which facilitates understanding of the operational environment, enemy, terrain, and civil considerations. It is not limited to collection of information but involves analysis as well, it includes tasks associated with intelligence, surveillance, and reconnaissance operations, and is driven by the commander. (derived from The Army Universal Task List FM 7-15 February 2009).</rdfs:comment>
    </owl:Class>
    


    <!-- http://www.cubrc.org/ontologies/KDD/Mid/EventOntology#ActOfMilitaryTrainingAcquisition -->

    <owl:Class rdf:about="http://www.cubrc.org/ontologies/KDD/Mid/EventOntology#ActOfMilitaryTrainingAcquisition">
        <rdfs:label rdf:datatype="&xsd;string">Act Of Military Training Acquisition</rdfs:label>
        <rdfs:subClassOf rdf:resource="http://www.cubrc.org/ontologies/KDD/Mid/EventOntology#ActOfTrainingAcquisition"/>
        <rdfs:comment rdf:datatype="&xsd;string">Definition: An Act of Training performed by an Agent by acquiring knowledge of the tactics, techniques, and/or strategies of Military Operations from an Agent or communication medium affiliated with a Military Organization.</rdfs:comment>
    </owl:Class>
    


    <!-- http://www.cubrc.org/ontologies/KDD/Mid/EventOntology#ActOfMilitaryTrainingInstruction -->

    <owl:Class rdf:about="http://www.cubrc.org/ontologies/KDD/Mid/EventOntology#ActOfMilitaryTrainingInstruction">
        <rdfs:label rdf:datatype="&xsd;string">Act Of Military Training Instruction</rdfs:label>
        <rdfs:subClassOf rdf:resource="http://www.cubrc.org/ontologies/KDD/Mid/EventOntology#ActOfTrainingInstruction"/>
        <rdfs:comment rdf:datatype="&xsd;string">Definition: An Act of Training performed by an Agent affiliated with some Military Organization by imparting knowledge of the tactics, techniques, and/or strategies of Military Operations to an Agent either directly or indirectly through some communication medium.</rdfs:comment>
    </owl:Class>
    


    <!-- http://www.cubrc.org/ontologies/KDD/Mid/EventOntology#ActOfMobilityOperation -->

    <owl:Class rdf:about="http://www.cubrc.org/ontologies/KDD/Mid/EventOntology#ActOfMobilityOperation">
        <rdfs:label>Conduct a Mobility Operation</rdfs:label>
        <rdfs:subClassOf rdf:resource="http://www.cubrc.org/ontologies/KDD/Mid/EventOntology#ActOfMovementAndManeuverWarfighting"/>
        <rdfs:comment>Definition: An Act of Military Force that realizes the objective of maintaining freedom of movement for personnel and equipment in an area of operations without delays due to terrain or barriers, obstacles, and mines. Mobility tasks include breaching, clearing, or crossing obstacles; increasing battlefield circulation; improving or building roads; providing bridge and raft support; and identifying routes around contaminated areas.  (derived from The Army Universal Task List FM 7-15 February 2009).</rdfs:comment>
    </owl:Class>
    


    <!-- http://www.cubrc.org/ontologies/KDD/Mid/EventOntology#ActOfMoneyLaundering -->

    <owl:Class rdf:about="http://www.cubrc.org/ontologies/KDD/Mid/EventOntology#ActOfMoneyLaundering">
        <rdfs:label rdf:datatype="&xsd;string">Act of Money Laundering</rdfs:label>
        <rdfs:subClassOf rdf:resource="http://www.cubrc.org/ontologies/KDD/Mid/EventOntology#CriminalActAgainstJustice"/>
        <rdfs:comment rdf:datatype="&xsd;string">Definition: A Criminal Act Against Justice involving financial transactions performed with the intent to conceal the identity, source, and/or destination of illegally gained money by which the proceeds of some Criminal Act are converted into assets which appear to have a legitimate origin. (derived from http:/en.wikipedia.org/wiki/Money_laundering).</rdfs:comment>
    </owl:Class>
    


    <!-- http://www.cubrc.org/ontologies/KDD/Mid/EventOntology#ActOfMotion -->

    <owl:Class rdf:about="http://www.cubrc.org/ontologies/KDD/Mid/EventOntology#ActOfMotion">
        <rdfs:label rdf:datatype="&xsd;string">Act of motion</rdfs:label>
        <rdfs:subClassOf rdf:resource="http://www.cubrc.org/ontologies/KDD/Mid/EventOntology#IntentionalAct"/>
    </owl:Class>
    


    <!-- http://www.cubrc.org/ontologies/KDD/Mid/EventOntology#ActOfMovement -->

    <owl:Class rdf:about="http://www.cubrc.org/ontologies/KDD/Mid/EventOntology#ActOfMovement">
        <rdfs:label rdf:datatype="&xsd;string">Act Of Movement</rdfs:label>
        <rdfs:subClassOf rdf:resource="http://www.cubrc.org/ontologies/KDD/Mid/EventOntology#ActOfMotion"/>
        <rdfs:comment rdf:datatype="&xsd;string">Definition: An Act of Motion in which a change of location occurs.</rdfs:comment>
    </owl:Class>
    


    <!-- http://www.cubrc.org/ontologies/KDD/Mid/EventOntology#ActOfMovementAndManeuverWarfighting -->

    <owl:Class rdf:about="http://www.cubrc.org/ontologies/KDD/Mid/EventOntology#ActOfMovementAndManeuverWarfighting">
        <rdfs:label>Realize the Movement and Maneuver Warfighting Function</rdfs:label>
        <rdfs:subClassOf rdf:resource="http://www.cubrc.org/ontologies/KDD/Mid/EventOntology#ActOfMilitaryForce"/>
        <rdfs:comment>Definition: An Act of Military Force having instances which are tasks that move forces to achieve a position of advantage in relation to the enemy (derived from The Army Universal Task List FM 7-15 February 2009).</rdfs:comment>
    </owl:Class>
    


    <!-- http://www.cubrc.org/ontologies/KDD/Mid/EventOntology#ActOfMovementToContact -->

    <owl:Class rdf:about="http://www.cubrc.org/ontologies/KDD/Mid/EventOntology#ActOfMovementToContact">
        <rdfs:label>Conduct a Movement to Contact</rdfs:label>
        <rdfs:subClassOf rdf:resource="http://www.cubrc.org/ontologies/KDD/Mid/EventOntology#ActOfOffensiveOperation"/>
        <rdfs:comment>Definition: An Act of Offensive Operation designed to develop the situation and establish or regain contact. Forces conducting a movement to contact seek to make contact with the smallest forces feasible (derived from The Army Universal Task List FM 7-15 February 2009).</rdfs:comment>
    </owl:Class>
    


    <!-- http://www.cubrc.org/ontologies/KDD/Mid/EventOntology#ActOfMurder -->

    <owl:Class rdf:about="http://www.cubrc.org/ontologies/KDD/Mid/EventOntology#ActOfMurder">
        <rdfs:label rdf:datatype="&xsd;string">Act Of Murder</rdfs:label>
        <rdfs:subClassOf rdf:resource="http://www.cubrc.org/ontologies/KDD/Mid/EventOntology#ActOfHomicide"/>
        <rdfs:comment rdf:datatype="&xsd;string">An Act Of Homicide with malice aforethought.</rdfs:comment>
    </owl:Class>
    


    <!-- http://www.cubrc.org/ontologies/KDD/Mid/EventOntology#ActOfNonLethalDirectFire -->

    <owl:Class rdf:about="http://www.cubrc.org/ontologies/KDD/Mid/EventOntology#ActOfNonLethalDirectFire">
        <rdfs:label>Non-Lethal Direct Fire</rdfs:label>
        <rdfs:subClassOf rdf:resource="http://www.cubrc.org/ontologies/KDD/Mid/EventOntology#ActOfDirectFire"/>
        <rdfs:comment>Definition: An Act of Direct Fire in which some Force employs nonlethal direct fires to incapacitate threat personnel and materiel without causing permanent injury or destruction; the fires include using nonlethal weapons such as directed energy, blunt trauma, riot control agents, vehicle and vessel arresting devices, and water cannons (derived from The Army Universal Task List FM 7-15 February 2009).</rdfs:comment>
    </owl:Class>
    


    <!-- http://www.cubrc.org/ontologies/KDD/Mid/EventOntology#ActOfOathTaking -->

    <owl:Class rdf:about="http://www.cubrc.org/ontologies/KDD/Mid/EventOntology#ActOfOathTaking">
        <rdfs:label rdf:datatype="&xsd;string">Act Of Oath Taking</rdfs:label>
        <rdfs:subClassOf rdf:resource="http://www.cubrc.org/ontologies/KDD/Mid/EventOntology#ActOfCommissiveCommunication"/>
    </owl:Class>
    


    <!-- http://www.cubrc.org/ontologies/KDD/Mid/EventOntology#ActOfObstruction -->

    <owl:Class rdf:about="http://www.cubrc.org/ontologies/KDD/Mid/EventOntology#ActOfObstruction">
        <rdfs:label>Act Of Obstruction</rdfs:label>
        <rdfs:subClassOf rdf:resource="http://www.cubrc.org/ontologies/KDD/Mid/EventOntology#CriminalActAgainstJustice"/>
        <rdfs:comment>Definition: A Criminal Act Against Justice that involves interfering with the work of police, investigators, regulatory agencies, prosecutors, or other (usually government) officials. Examples include providing an offender with a false alibi and the destruction of evidence. (derived from http://en.wikipedia.org/wiki/Obstruction_of_justice)</rdfs:comment>
    </owl:Class>
    


    <!-- http://www.cubrc.org/ontologies/KDD/Mid/EventOntology#ActOfOffensiveOperation -->

    <owl:Class rdf:about="http://www.cubrc.org/ontologies/KDD/Mid/EventOntology#ActOfOffensiveOperation">
        <rdfs:label>Conduct Offensive Operation</rdfs:label>
        <rdfs:subClassOf rdf:resource="http://www.cubrc.org/ontologies/KDD/Mid/EventOntology#ActOfMilitaryForce"/>
        <rdfs:comment>Definition: An Act of Military Force conducted to defeat and destroy enemy forces and seize terrain, resources, and population centers (derived from The Army Universal Task List FM 7-15 February 2009).</rdfs:comment>
    </owl:Class>
    


    <!-- http://www.cubrc.org/ontologies/KDD/Mid/EventOntology#ActOfOperationSecurity -->

    <owl:Class rdf:about="http://www.cubrc.org/ontologies/KDD/Mid/EventOntology#ActOfOperationSecurity">
        <rdfs:label>Conduct Operations Security</rdfs:label>
        <rdfs:subClassOf rdf:resource="http://www.cubrc.org/ontologies/KDD/Mid/EventOntology#ActOfProtectionWarfighting"/>
        <rdfs:comment>Definition: An Act of Protection Warfighting in which involves selecting and executing measures that eliminate or reduce to an acceptable level the vulnerabilities of friendly actions to adversary exploitation (derived from The Army Universal Task List FM 7-15 February 2009).</rdfs:comment>
    </owl:Class>
    


    <!-- http://www.cubrc.org/ontologies/KDD/Mid/EventOntology#ActOfOperationalAreaSecurity -->

    <owl:Class rdf:about="http://www.cubrc.org/ontologies/KDD/Mid/EventOntology#ActOfOperationalAreaSecurity">
        <rdfs:label>Conduct Operational Area Security</rdfs:label>
        <rdfs:subClassOf rdf:resource="http://www.cubrc.org/ontologies/KDD/Mid/EventOntology#ActOfProtectionWarfighting"/>
        <rdfs:comment>Definition: An Act of Protection Warfighting friendly forces, installations, routes, and actions within an area of operations are protected (derived from The Army Universal Task List FM 7-15 February 2009).</rdfs:comment>
    </owl:Class>
    


    <!-- http://www.cubrc.org/ontologies/KDD/Mid/EventOntology#ActOfOperationsProcessExecution -->

    <owl:Class rdf:about="http://www.cubrc.org/ontologies/KDD/Mid/EventOntology#ActOfOperationsProcessExecution">
        <rdfs:label>Execute the Operations Process</rdfs:label>
        <rdfs:subClassOf rdf:resource="http://www.cubrc.org/ontologies/KDD/Mid/EventOntology#ActOfCommandAndControlWarfighting"/>
        <rdfs:comment>Definition: An Act of Command and Control Warfighting during which one or more of the major command and control activities performed during operations: planning, preparing, executing, or continuously assessing the operation is performed. These acts may be sequential or simultaneous and they are usually not discrete; they overlap and recur as circumstances demand  (derived from The Army Universal Task List FM 7-15 February 2009).</rdfs:comment>
    </owl:Class>
    


    <!-- http://www.cubrc.org/ontologies/KDD/Mid/EventOntology#ActOfOrganizedRetailTheft -->

    <owl:Class rdf:about="http://www.cubrc.org/ontologies/KDD/Mid/EventOntology#ActOfOrganizedRetailTheft">
        <rdfs:subClassOf rdf:resource="http://www.cubrc.org/ontologies/KDD/Mid/EventOntology#ActOfLarceny"/>
        <rdfs:comment rdf:datatype="&xsd;string">Definition: An Act of Larceny in which professional burglars, boosters, cons, thieves, fences and resellers conspire to steal and sell retail merchandise obtained from retail establishments by theft or deception. (Source: http://www.fbi.gov/news/testimony/combating-organized-retail-crime-the-role-of-federal-law-enforcement)</rdfs:comment>
    </owl:Class>
    


    <!-- http://www.cubrc.org/ontologies/KDD/Mid/EventOntology#ActOfOwnership -->

    <owl:Class rdf:about="http://www.cubrc.org/ontologies/KDD/Mid/EventOntology#ActOfOwnership">
        <rdfs:label rdf:datatype="&xsd;string">Act of ownership</rdfs:label>
        <rdfs:subClassOf rdf:resource="http://www.cubrc.org/ontologies/KDD/Mid/EventOntology#ActOfPossession"/>
    </owl:Class>
    


    <!-- http://www.cubrc.org/ontologies/KDD/Mid/EventOntology#ActOfParole -->

    <owl:Class rdf:about="http://www.cubrc.org/ontologies/KDD/Mid/EventOntology#ActOfParole">
        <rdfs:label>Act Of Parole</rdfs:label>
        <rdfs:subClassOf rdf:resource="http://www.cubrc.org/ontologies/KDD/Mid/EventOntology#LegalSystemAct"/>
        <rdfs:comment>Definition: A Legal System Act involving the supervised release of a criminal from Incarceration on certain prescribed conditions which entitle him to a termination of his Sentence. (derived from http://www.id.uscourts.gov/glossary.htm)</rdfs:comment>
    </owl:Class>
    


    <!-- http://www.cubrc.org/ontologies/KDD/Mid/EventOntology#ActOfPassageOfLines -->

    <owl:Class rdf:about="http://www.cubrc.org/ontologies/KDD/Mid/EventOntology#ActOfPassageOfLines">
        <rdfs:label>Conduct Passage of Lines</rdfs:label>
        <rdfs:subClassOf rdf:resource="http://www.cubrc.org/ontologies/KDD/Mid/EventOntology#ActOfForceManeuver"/>
        <rdfs:comment>Definition: An Act of Force Maneuver in which one unit moves through another unit�s positions with the intent of moving into or out of enemy contact (derived from The Army Universal Task List FM 7-15 February 2009).</rdfs:comment>
    </owl:Class>
    


    <!-- http://www.cubrc.org/ontologies/KDD/Mid/EventOntology#ActOfPenetrationManeuver -->

    <owl:Class rdf:about="http://www.cubrc.org/ontologies/KDD/Mid/EventOntology#ActOfPenetrationManeuver">
        <rdfs:label>Conduct a Penetration</rdfs:label>
        <rdfs:subClassOf rdf:resource="http://www.cubrc.org/ontologies/KDD/Mid/EventOntology#ActOfForceManeuver"/>
        <rdfs:comment>Definition: An Act of Force Maneuver in which an attacking force seeks to rupture enemy defenses on a narrow front to disrupt the defensive system. Commanders direct penetrations when enemy flanks are not assailable or time does not permit another form of maneuver. Successful penetrations create assailable flanks and provide access to enemy sustainment areas.  (derived from The Army Universal Task List FM 7-15 February 2009).</rdfs:comment>
    </owl:Class>
    


    <!-- http://www.cubrc.org/ontologies/KDD/Mid/EventOntology#ActOfPerformingCBRNEOperation -->

    <owl:Class rdf:about="http://www.cubrc.org/ontologies/KDD/Mid/EventOntology#ActOfPerformingCBRNEOperation">
        <rdfs:label>Conduct CBRNE</rdfs:label>
        <rdfs:subClassOf rdf:resource="http://www.cubrc.org/ontologies/KDD/Mid/EventOntology#ActOfProtectionWarfighting"/>
        <rdfs:comment>Definition: An Act of Protection Wartfighting in which forces defend against chemical, biological, radiological, nuclear, and high-yield explosives (CBRNE) weapons using the principles of avoidance, protection, and decontamination (derived from The Army Universal Task List FM 7-15 February 2009).</rdfs:comment>
    </owl:Class>
    


    <!-- http://www.cubrc.org/ontologies/KDD/Mid/EventOntology#ActOfPerjury -->

    <owl:Class rdf:about="http://www.cubrc.org/ontologies/KDD/Mid/EventOntology#ActOfPerjury">
        <rdfs:label>Act Of Perjury</rdfs:label>
        <rdfs:subClassOf rdf:resource="http://www.cubrc.org/ontologies/KDD/Mid/EventOntology#CriminalActAgainstJustice"/>
        <rdfs:comment>Definition: A Criminal Act Against Justice that is the willful act of swearing a false oath or affirmation to tell the truth, whether spoken or in writing, concerning matters material to a judicial proceeding. (derived from http://en.wikipedia.org/wiki/Perjury)</rdfs:comment>
    </owl:Class>
    


    <!-- http://www.cubrc.org/ontologies/KDD/Mid/EventOntology#ActOfPersonalCommunication -->

    <owl:Class rdf:about="http://www.cubrc.org/ontologies/KDD/Mid/EventOntology#ActOfPersonalCommunication">
        <rdfs:label>Act Of Personal Communication</rdfs:label>
        <rdfs:subClassOf rdf:resource="http://www.cubrc.org/ontologies/KDD/Mid/EventOntology#ActOfCommunication"/>
        <rdfs:comment>Definition: An Act of Communication having a small audience</rdfs:comment>
    </owl:Class>
    


    <!-- http://www.cubrc.org/ontologies/KDD/Mid/EventOntology#ActOfPersonnelRecoveryOperation -->

    <owl:Class rdf:about="http://www.cubrc.org/ontologies/KDD/Mid/EventOntology#ActOfPersonnelRecoveryOperation">
        <rdfs:label>Conduct Personnel Recovery Operations</rdfs:label>
        <rdfs:subClassOf rdf:resource="http://www.cubrc.org/ontologies/KDD/Mid/EventOntology#ActOfProtectionWarfighting"/>
        <rdfs:comment>Definition: An Act of Protection Warfighting to recover and return own personnel, whether Soldier, Army civilian, selected Department of Defense (DOD) contractors, or other personnel as determined by the Secretary of Defense who are isolated, missing, detained, or captured (IMDC) in an operational environment. IMDC personnel consist of U.S. forces, Army civilians, and DOD contractors who deploy with the force, or other personnel as designated by the President who are beyond the Army positive or procedural control of their unit, in an operational environment requiring them to survive, evade, resist, or escape.  (derived from The Army Universal Task List FM 7-15 February 2009).</rdfs:comment>
    </owl:Class>
    


    <!-- http://www.cubrc.org/ontologies/KDD/Mid/EventOntology#ActOfPersonnelServicesSupport -->

    <owl:Class rdf:about="http://www.cubrc.org/ontologies/KDD/Mid/EventOntology#ActOfPersonnelServicesSupport">
        <rdfs:label>Provide Personnel Services Support</rdfs:label>
        <rdfs:subClassOf rdf:resource="http://www.cubrc.org/ontologies/KDD/Mid/EventOntology#ActOfSustainmentWarfighting"/>
        <rdfs:comment>Definition: An Act of Military Force in which personnel services are provided for those sustainment functions related to Soldiers� welfare, readiness, and quality of life (derived from The Army Universal Task List FM 7-15 February 2009).</rdfs:comment>
    </owl:Class>
    


    <!-- http://www.cubrc.org/ontologies/KDD/Mid/EventOntology#ActOfPilgrimage -->

    <owl:Class rdf:about="http://www.cubrc.org/ontologies/KDD/Mid/EventOntology#ActOfPilgrimage">
        <rdfs:label rdf:datatype="&xsd;string">Act Of Pilgrimage</rdfs:label>
        <rdfs:subClassOf rdf:resource="http://www.cubrc.org/ontologies/KDD/Mid/EventOntology#ActOfTravel"/>
        <rdfs:comment rdf:datatype="&xsd;string">Definition: An Act Of Travel to a Location of importance to a person&apos;s beliefs and faith. (derived from http://en.wikipedia.org/wiki/Pilgrimage)</rdfs:comment>
    </owl:Class>
    


    <!-- http://www.cubrc.org/ontologies/KDD/Mid/EventOntology#ActOfPlanningForImprovisedExplosiveDeviceThreat -->

    <owl:Class rdf:about="http://www.cubrc.org/ontologies/KDD/Mid/EventOntology#ActOfPlanningForImprovisedExplosiveDeviceThreat">
        <rdfs:label>Plan for Possible Improvised Explosive Device Threat</rdfs:label>
        <rdfs:subClassOf rdf:resource="http://www.cubrc.org/ontologies/KDD/Mid/EventOntology#ActOfConductingImprovisedExplosiveDefeatOperation"/>
        <rdfs:comment>Definition: An Act of Conducting Improvised Explosive Defeat Operation that is a proactive action taken by friendly forces to predict, detect, prevent, avoid, neutralize, and protect against improvised explosive device events (derived from The Army Universal Task List FM 7-15 February 2009).</rdfs:comment>
    </owl:Class>
    


    <!-- http://www.cubrc.org/ontologies/KDD/Mid/EventOntology#ActOfPositionChange -->

    <owl:Class rdf:about="http://www.cubrc.org/ontologies/KDD/Mid/EventOntology#ActOfPositionChange">
        <rdfs:label rdf:datatype="&xsd;string">Act of position change</rdfs:label>
        <rdfs:subClassOf rdf:resource="http://www.cubrc.org/ontologies/KDD/Mid/EventOntology#ActOfMotion"/>
        <rdfs:comment rdf:datatype="&xsd;string">Definition: An Act Of Motion that does not entail an change of location, often a movement of a part of an object.</rdfs:comment>
    </owl:Class>
    


    <!-- http://www.cubrc.org/ontologies/KDD/Mid/EventOntology#ActOfPossession -->

    <owl:Class rdf:about="http://www.cubrc.org/ontologies/KDD/Mid/EventOntology#ActOfPossession">
        <rdfs:label rdf:datatype="&xsd;string">Act of possession</rdfs:label>
        <rdfs:subClassOf rdf:resource="http://www.cubrc.org/ontologies/KDD/Mid/EventOntology#IntentionalAct"/>
        <rdfs:comment rdf:datatype="&xsd;string">Definition: An Intentional Act in which an agent intentionally exercises control towards a thing. In all cases, to possess something, an agent must have an intention to possess it.  (Derived from http://en.wikipedia.org/wiki/Possession_(law)</rdfs:comment>
    </owl:Class>
    


    <!-- http://www.cubrc.org/ontologies/KDD/Mid/EventOntology#ActOfPostblastAnalysis -->

    <owl:Class rdf:about="http://www.cubrc.org/ontologies/KDD/Mid/EventOntology#ActOfPostblastAnalysis">
        <rdfs:label>Conduct Crater Fragmentation and Post-Blast Analysis</rdfs:label>
        <rdfs:subClassOf rdf:resource="http://www.cubrc.org/ontologies/KDD/Mid/EventOntology#ActOfMilitaryIntelligence"/>
        <rdfs:comment>Definition: An Act of Military Intelligence in which some Explosive ordnance disposal (EOD) unit conducts postblast analysis for forensic evidence and, if the need exists, EOD personnel can collect chemical and biological samples for analysis (derived from The Army Universal Task List FM 7-15 February 2009).</rdfs:comment>
    </owl:Class>
    


    <!-- http://www.cubrc.org/ontologies/KDD/Mid/EventOntology#ActOfPreparationForImprovisedExplosiveDefeatOperation -->

    <owl:Class rdf:about="http://www.cubrc.org/ontologies/KDD/Mid/EventOntology#ActOfPreparationForImprovisedExplosiveDefeatOperation">
        <rdfs:label>Prepare for Improvised Explosive Device (IED) Defeat</rdfs:label>
        <rdfs:subClassOf rdf:resource="http://www.cubrc.org/ontologies/KDD/Mid/EventOntology#ActOfConductingImprovisedExplosiveDefeatOperation"/>
        <rdfs:comment>Definition: An Act of Conducting Improvised Explosive Defeat Operation in which Units prepare for IED defeat operations prior to movement using the tenets of IED defeat (predict, detect, prevent, neutralize, and mitigate) (derived from The Army Universal Task List FM 7-15 February 2009).</rdfs:comment>
    </owl:Class>
    


    <!-- http://www.cubrc.org/ontologies/KDD/Mid/EventOntology#ActOfPreparationForSuspectedImprovisedExplosiveAttack -->

    <owl:Class rdf:about="http://www.cubrc.org/ontologies/KDD/Mid/EventOntology#ActOfPreparationForSuspectedImprovisedExplosiveAttack">
        <rdfs:label>Prepare for a Suspected Improvised Explosive Device Attack</rdfs:label>
        <rdfs:subClassOf rdf:resource="http://www.cubrc.org/ontologies/KDD/Mid/EventOntology#ActOfConductingImprovisedExplosiveDefeatOperation"/>
        <rdfs:comment>Definition: An Act of Conducting Improvised Explosive Defeat Operation in which units prepart for Enemy forces presenting the U.S. or coalition forces with conditions for which they are unprepared. Enemy organizations will adjust their improvised explosive device (IED) tactics, techniques, and procedures to the strengths and weaknesses of U.S. or coalition forces. The enemy is prepared to disperse its forces in areas of sanctuary and employ them in ways that make it difficult for U.S. or coalition forces to analyze and predict (derived from The Army Universal Task List FM 7-15 February 2009).</rdfs:comment>
    </owl:Class>
    


    <!-- http://www.cubrc.org/ontologies/KDD/Mid/EventOntology#ActOfPreparingFightingPositions -->

    <owl:Class rdf:about="http://www.cubrc.org/ontologies/KDD/Mid/EventOntology#ActOfPreparingFightingPositions">
        <rdfs:label>Prepare Fighting Positions</rdfs:label>
        <rdfs:subClassOf rdf:resource="http://www.cubrc.org/ontologies/KDD/Mid/EventOntology#ActOfSurvivabilityOperation"/>
        <rdfs:comment>Definition: An Act of Survivability Operation in which primary, alternate, and supplementary fighting positions that provide cover, concealment, and protection from the effects of enemy fires for occupants and systems, and allow for fields of fire and maneuver space for combat systems and units engaging the enemy are prepared (derived from The Army Universal Task List FM 7-15 February 2009).</rdfs:comment>
    </owl:Class>
    


    <!-- http://www.cubrc.org/ontologies/KDD/Mid/EventOntology#ActOfPreparingProtectivePositions -->

    <owl:Class rdf:about="http://www.cubrc.org/ontologies/KDD/Mid/EventOntology#ActOfPreparingProtectivePositions">
        <rdfs:label>Prepare Protective Positions</rdfs:label>
        <rdfs:subClassOf rdf:resource="http://www.cubrc.org/ontologies/KDD/Mid/EventOntology#ActOfSurvivabilityOperation"/>
        <rdfs:comment>Definition: An Act of Survivability Operation in which cover and concealment for personnel, systems, equipment, supplies, and other materiel not directly involved in fighting are provided (derived from The Army Universal Task List FM 7-15 February 2009).</rdfs:comment>
    </owl:Class>
    


    <!-- http://www.cubrc.org/ontologies/KDD/Mid/EventOntology#ActOfPrescriptionDrugTrafficking -->

    <owl:Class rdf:about="http://www.cubrc.org/ontologies/KDD/Mid/EventOntology#ActOfPrescriptionDrugTrafficking">
        <rdfs:label>Act Of Prescription Drug Trafficking</rdfs:label>
        <rdfs:subClassOf rdf:resource="http://www.cubrc.org/ontologies/KDD/Mid/EventOntology#ActOfDrugTrafficking"/>
        <rdfs:comment>Definition: An Act of Drug Trafficking involving the illegal distribution and sale of Prescription Drugs.</rdfs:comment>
    </owl:Class>
    


    <!-- http://www.cubrc.org/ontologies/KDD/Mid/EventOntology#ActOfProbation -->

    <owl:Class rdf:about="http://www.cubrc.org/ontologies/KDD/Mid/EventOntology#ActOfProbation">
        <rdfs:label>Act Of Probation</rdfs:label>
        <rdfs:subClassOf rdf:resource="http://www.cubrc.org/ontologies/KDD/Mid/EventOntology#ActOfSentencing"/>
        <rdfs:comment>Definition: A Sentence that involves allowing a Person that has been found guilty of a Criminal Act to stay in the community, usually under the supervision of a Parole Officer (derived from http://www.id.uscourts.gov/glossary.htm)</rdfs:comment>
    </owl:Class>
    


    <!-- http://www.cubrc.org/ontologies/KDD/Mid/EventOntology#ActOfProcurementFraud -->

    <owl:Class rdf:about="http://www.cubrc.org/ontologies/KDD/Mid/EventOntology#ActOfProcurementFraud">
        <rdfs:label>Act of Procurement Fraud</rdfs:label>
        <rdfs:subClassOf rdf:resource="http://www.cubrc.org/ontologies/KDD/Mid/EventOntology#ActOfFraud"/>
        <rdfs:comment>Definition: An Act of Fraud in which an Agent dishonestly obtains an advantage, avoids an obligation or causes a loss to public property or various means during the procurement process by public servants, contractors or any other person involved in the procurement. (derived from http://en.wikipedia.org/wiki/Procurement)</rdfs:comment>
    </owl:Class>
    


    <!-- http://www.cubrc.org/ontologies/KDD/Mid/EventOntology#ActOfPromising -->

    <owl:Class rdf:about="http://www.cubrc.org/ontologies/KDD/Mid/EventOntology#ActOfPromising">
        <rdfs:label rdf:datatype="&xsd;string">Act Of Promising</rdfs:label>
        <rdfs:subClassOf rdf:resource="http://www.cubrc.org/ontologies/KDD/Mid/EventOntology#ActOfCommissiveCommunication"/>
    </owl:Class>
    


    <!-- http://www.cubrc.org/ontologies/KDD/Mid/EventOntology#ActOfPropaganda -->

    <owl:Class rdf:about="http://www.cubrc.org/ontologies/KDD/Mid/EventOntology#ActOfPropaganda">
        <rdfs:label>Act Of Propaganda</rdfs:label>
        <rdfs:subClassOf rdf:resource="http://www.cubrc.org/ontologies/KDD/Mid/EventOntology#ActOfDeceptiveCommunication"/>
        <rdfs:comment>Definition: An Act Of Deceptive Communication Propaganda intended to influence the attitude of a mass audience toward some cause or position by presenting facts selectively (thus possibly lying by omission)  or by using loaded messages to produce an emotional rather than rational response to the information presented. (derived from http://en.wikipedia.org/wiki/Propaganda)</rdfs:comment>
    </owl:Class>
    


    <!-- http://www.cubrc.org/ontologies/KDD/Mid/EventOntology#ActOfProstitution -->

    <owl:Class rdf:about="http://www.cubrc.org/ontologies/KDD/Mid/EventOntology#ActOfProstitution">
        <rdfs:label>Act Of Prostitution</rdfs:label>
        <rdfs:subClassOf rdf:resource="http://www.cubrc.org/ontologies/KDD/Mid/EventOntology#ActOfBlackMarketTrafficking"/>
        <rdfs:comment>Definition: An Act of Black Market Trafficking involving the illegal provision of sexual services to another person in return for payment (derived from http://en.wikipedia.org/wiki/Prostitution).</rdfs:comment>
    </owl:Class>
    


    <!-- http://www.cubrc.org/ontologies/KDD/Mid/EventOntology#ActOfProtectingIndividualsAndSystems -->

    <owl:Class rdf:about="http://www.cubrc.org/ontologies/KDD/Mid/EventOntology#ActOfProtectingIndividualsAndSystems">
        <rdfs:label>Protect Individuals and Systems</rdfs:label>
        <rdfs:subClassOf rdf:resource="http://www.cubrc.org/ontologies/KDD/Mid/EventOntology#ActOfSurvivabilityOperation"/>
        <rdfs:comment>Definition: An Act of Survivability Operation in which protective positions (natural or artificial), measures, or equipment such as armor, detection equipment, mission-oriented protective posture gear (MOPP), and collective protective equipment are used to reduce effects of enemy weapon systems (derived from The Army Universal Task List FM 7-15 February 2009).</rdfs:comment>
    </owl:Class>
    


    <!-- http://www.cubrc.org/ontologies/KDD/Mid/EventOntology#ActOfProtectionWarfighting -->

    <owl:Class rdf:about="http://www.cubrc.org/ontologies/KDD/Mid/EventOntology#ActOfProtectionWarfighting">
        <rdfs:label>Realize the Protection Warfighting Function</rdfs:label>
        <rdfs:subClassOf rdf:resource="http://www.cubrc.org/ontologies/KDD/Mid/EventOntology#ActOfMilitaryForce"/>
        <rdfs:comment>Definition: An Act of Military Force that preserves the force so the commander can apply maximum combat power. Examples of such acts include: protecting personnel (combatants and noncombatants), physical assets, and information of the United States and multinational military and civilian partners (derived from The Army Universal Task List FM 7-15 February 2009).</rdfs:comment>
    </owl:Class>
    


    <!-- http://www.cubrc.org/ontologies/KDD/Mid/EventOntology#ActOfProvidingForceHealthProtection -->

    <owl:Class rdf:about="http://www.cubrc.org/ontologies/KDD/Mid/EventOntology#ActOfProvidingForceHealthProtection">
        <rdfs:label>Provide Force Health Protection</rdfs:label>
        <rdfs:subClassOf rdf:resource="http://www.cubrc.org/ontologies/KDD/Mid/EventOntology#ActOfProtectionWarfighting"/>
        <rdfs:comment>Definition: An Act of Protection Warfighting that encompasses measures to promote, improve, or conserve the mental and physical well-being of Soldiers (derived from The Army Universal Task List FM 7-15 February 2009).</rdfs:comment>
    </owl:Class>
    


    <!-- http://www.cubrc.org/ontologies/KDD/Mid/EventOntology#ActOfPublicAffairsOperation -->

    <owl:Class rdf:about="http://www.cubrc.org/ontologies/KDD/Mid/EventOntology#ActOfPublicAffairsOperation">
        <rdfs:label>Public Affairs Operation</rdfs:label>
        <rdfs:subClassOf rdf:resource="http://www.cubrc.org/ontologies/KDD/Mid/EventOntology#ActOfCommandAndControlWarfighting"/>
        <rdfs:comment>Definition: An Act of Military Force which informs and educates internal and external publics through public information, command information, and direct community engagement (derived from The Army Universal Task List FM 7-15 February 2009).</rdfs:comment>
    </owl:Class>
    


    <!-- http://www.cubrc.org/ontologies/KDD/Mid/EventOntology#ActOfPublicEducationAndInformationSupport -->

    <owl:Class rdf:about="http://www.cubrc.org/ontologies/KDD/Mid/EventOntology#ActOfPublicEducationAndInformationSupport">
        <rdfs:label>Public Education and Information Support</rdfs:label>
        <rdfs:subClassOf rdf:resource="http://www.cubrc.org/ontologies/KDD/Mid/EventOntology#ActOfCivilAffairs"/>
        <rdfs:comment>Definition: An Act of Civil Affairs that includes instances of providing public education and information support (derived from The Army Universal Task List FM 7-15 February 2009).</rdfs:comment>
    </owl:Class>
    


    <!-- http://www.cubrc.org/ontologies/KDD/Mid/EventOntology#ActOfPublicHealthAndWelfareSupport -->

    <owl:Class rdf:about="http://www.cubrc.org/ontologies/KDD/Mid/EventOntology#ActOfPublicHealthAndWelfareSupport">
        <rdfs:label>Public Health and Welfare Support</rdfs:label>
        <rdfs:subClassOf rdf:resource="http://www.cubrc.org/ontologies/KDD/Mid/EventOntology#ActOfCivilAffairs"/>
        <rdfs:comment>Definition: An Act of Civil Affairs that is an instance of any of the following types of action: determining the type and amount of welfare supplies needed for emergency relief, plan and coordination of the use of welfare supplies from all sources, advise and assist the host-nation government, and establishing and supervising emergency centers for distributing supplies and for housing and feeding civilians (derived from The Army Universal Task List FM 7-15 February 2009).</rdfs:comment>
    </owl:Class>
    


    <!-- http://www.cubrc.org/ontologies/KDD/Mid/EventOntology#ActOfPublicLegalSupport -->

    <owl:Class rdf:about="http://www.cubrc.org/ontologies/KDD/Mid/EventOntology#ActOfPublicLegalSupport">
        <rdfs:label>Public Legal Support</rdfs:label>
        <rdfs:subClassOf rdf:resource="http://www.cubrc.org/ontologies/KDD/Mid/EventOntology#ActOfCivilAffairs"/>
        <rdfs:comment>Definition: An Act of Civil Affairs that establishes the fair, competent, and efficient application and fair and effective enforcement of the civil and criminal laws of a society through impartial legal institutions and competent police and corrections systems (derived from The Army Universal Task List FM 7-15 February 2009).</rdfs:comment>
    </owl:Class>
    


    <!-- http://www.cubrc.org/ontologies/KDD/Mid/EventOntology#ActOfPublishingMassMediaArticle -->

    <owl:Class rdf:about="http://www.cubrc.org/ontologies/KDD/Mid/EventOntology#ActOfPublishingMassMediaArticle">
        <rdfs:label>Act Of Publishing Mass Media Article</rdfs:label>
        <rdfs:subClassOf rdf:resource="http://www.cubrc.org/ontologies/KDD/Mid/EventOntology#ActOfMassMediaCommunication"/>
        <rdfs:comment>Definition: An Act Of Mass Media Communication involving the making generally known a non-fictional essay, especially one included with others in a newspaper, magazine, journal, etc. (derived from JC3IEDM-MIRD-DMWG-Edition_3.0.2_20090514)</rdfs:comment>
    </owl:Class>
    


    <!-- http://www.cubrc.org/ontologies/KDD/Mid/EventOntology#ActOfPublishingMassMediaDocumentary -->

    <owl:Class rdf:about="http://www.cubrc.org/ontologies/KDD/Mid/EventOntology#ActOfPublishingMassMediaDocumentary">
        <rdfs:label>Act Of Publishing Mass Media Documentary</rdfs:label>
        <rdfs:subClassOf rdf:resource="http://www.cubrc.org/ontologies/KDD/Mid/EventOntology#ActOfMassMediaCommunication"/>
        <rdfs:comment>Definition: An Act Of Mass Media Communication involiving the generally making known information that provides a factual record or report. (derived from JC3IEDM-MIRD-DMWG-Edition_3.0.2_20090514)</rdfs:comment>
    </owl:Class>
    


    <!-- http://www.cubrc.org/ontologies/KDD/Mid/EventOntology#ActOfPublishingMassMediaPressRelease -->

    <owl:Class rdf:about="http://www.cubrc.org/ontologies/KDD/Mid/EventOntology#ActOfPublishingMassMediaPressRelease">
        <rdfs:label>Act Of Publishing Mass Media Press Release</rdfs:label>
        <rdfs:subClassOf rdf:resource="http://www.cubrc.org/ontologies/KDD/Mid/EventOntology#ActOfMassMediaCommunication"/>
        <rdfs:comment>Definition: An Act Of Mass Media Communication involving the generally making known an official statement issued to media for information. (derived from JC3IEDM-MIRD-DMWG-Edition_3.0.2_20090514)</rdfs:comment>
    </owl:Class>
    


    <!-- http://www.cubrc.org/ontologies/KDD/Mid/EventOntology#ActOfPurchasing -->

    <owl:Class rdf:about="http://www.cubrc.org/ontologies/KDD/Mid/EventOntology#ActOfPurchasing">
        <rdfs:label rdf:datatype="&xsd;string">Act Of Purchasing</rdfs:label>
        <rdfs:subClassOf rdf:resource="http://www.cubrc.org/ontologies/KDD/Mid/EventOntology#ActOfFinancialInstrumentUse"/>
        <rdfs:comment rdf:datatype="&xsd;string">Definition: An Act of Financial Instrument Use wherein a Financial Instrument by Function or a Finanical Instrument by Role is used by an Agent (buyer) to acquire a good or service from another agent (seller) (derived from http://en.wikipedia.org/wiki/Purchase)</rdfs:comment>
    </owl:Class>
    


    <!-- http://www.cubrc.org/ontologies/KDD/Mid/EventOntology#ActOfRacketeering -->

    <owl:Class rdf:about="http://www.cubrc.org/ontologies/KDD/Mid/EventOntology#ActOfRacketeering">
        <rdfs:subClassOf rdf:resource="http://www.cubrc.org/ontologies/KDD/Mid/EventOntology#CriminalAct"/>
        <rdfs:comment rdf:datatype="&xsd;string">Definition: A Criminal Act composed of those predicate criminal acts that are chargeable under the Racketeer Influenced and Corrupt Organizations statute. These are found in Title 18 of the United States Code, Section 1961 (1) and include the following federal crimes: (Bribery, Sports Bribery, Counterfeiting, Embezzlement of Union Funds, Mail Fraud, Wire Fraud, Money Laundering, Obstruction of Justice, Murder for Hire, Drug Trafficking, Prostitution, Sexual Exploitation of Children, Alien Smuggling, Trafficking in Counterfeit Goods, Theft from Interstate Shipment, Interstate Transportation of Stolen Property) and the following state crimes: ( Murder, Kidnapping, Gambling, Arson, Robbery, Bribery, Extortion, Drugs) (Source: http://www.fbi.gov/about-us/investigate/organizedcrime/glossary)</rdfs:comment>
    </owl:Class>
    


    <!-- http://www.cubrc.org/ontologies/KDD/Mid/EventOntology#ActOfReactingToEnemyDirectFires -->

    <owl:Class rdf:about="http://www.cubrc.org/ontologies/KDD/Mid/EventOntology#ActOfReactingToEnemyDirectFires">
        <rdfs:label>React to Enemy Direct Fires</rdfs:label>
        <rdfs:subClassOf rdf:resource="http://www.cubrc.org/ontologies/KDD/Mid/EventOntology#ActOfSurvivabilityOperation"/>
        <rdfs:comment>Definition: An Act of Survivability in which fire is returned at known or suspected enemy positions and take evasive action upon detecting enemy direct fires.  (derived from The Army Universal Task List FM 7-15 February 2009).</rdfs:comment>
    </owl:Class>
    


    <!-- http://www.cubrc.org/ontologies/KDD/Mid/EventOntology#ActOfReactingToEnemyIndirectFires -->

    <owl:Class rdf:about="http://www.cubrc.org/ontologies/KDD/Mid/EventOntology#ActOfReactingToEnemyIndirectFires">
        <rdfs:label>React to Enemy Indirect Fires</rdfs:label>
        <rdfs:subClassOf rdf:resource="http://www.cubrc.org/ontologies/KDD/Mid/EventOntology#ActOfSurvivabilityOperation"/>
        <rdfs:comment>Definition: An Act of Survivability in which Forces seek protection under the overhead cover of fighting or protective positions or move rapidly out of the impact area in the direction the unit commander orders. If armored vehicles are available, personnel mount, and the vehicles move out of the impact area in the direction and designated distance ordered by the unit commander (derived from The Army Universal Task List FM 7-15 February 2009).</rdfs:comment>
    </owl:Class>
    


    <!-- http://www.cubrc.org/ontologies/KDD/Mid/EventOntology#ActOfReactingToImprovisedExplosiveDevice -->

    <owl:Class rdf:about="http://www.cubrc.org/ontologies/KDD/Mid/EventOntology#ActOfReactingToImprovisedExplosiveDevice">
        <rdfs:label>React to Improvised Explosive Device</rdfs:label>
        <rdfs:subClassOf rdf:resource="http://www.cubrc.org/ontologies/KDD/Mid/EventOntology#ActOfConductingImprovisedExplosiveDefeatOperation"/>
        <rdfs:comment>Definition: An Act of Conducting Improvised Explosive Defeat Operation in which units plan, develop, and execute training to prevent or mitigate the potential effects that an IED may have on personnel and equipment (derived from The Army Universal Task List FM 7-15 February 2009).</rdfs:comment>
    </owl:Class>
    


    <!-- http://www.cubrc.org/ontologies/KDD/Mid/EventOntology#ActOfReceiptOfStolenProperty -->

    <owl:Class rdf:about="http://www.cubrc.org/ontologies/KDD/Mid/EventOntology#ActOfReceiptOfStolenProperty">
        <rdfs:label>Act Of Receipt Of Stolen Property</rdfs:label>
        <rdfs:subClassOf rdf:resource="http://www.cubrc.org/ontologies/KDD/Mid/EventOntology#CriminalActAgainstProperty"/>
        <rdfs:comment>Definition: A Criminal Act Against Property of knowingly receiving, concealing, or disposing of stolen property. (derived from http://en.wikipedia.org/wiki/Receipt_of_stolen_property)</rdfs:comment>
    </owl:Class>
    


    <!-- http://www.cubrc.org/ontologies/KDD/Mid/EventOntology#ActOfReconnaissance -->

    <owl:Class rdf:about="http://www.cubrc.org/ontologies/KDD/Mid/EventOntology#ActOfReconnaissance">
        <rdfs:label rdf:datatype="&xsd;string">Act Of Reconnaissance</rdfs:label>
        <rdfs:label>Reconnaissance</rdfs:label>
        <rdfs:subClassOf rdf:resource="http://www.cubrc.org/ontologies/KDD/Mid/EventOntology#ActOfIntelligenceGathering"/>
        <rdfs:subClassOf rdf:resource="http://www.cubrc.org/ontologies/KDD/Mid/EventOntology#ActOfIntelligenceSurveillanceAndReconnaisance"/>
        <rdfs:comment rdf:datatype="&xsd;string">Definition: An Act of Intelligence Gathering used to determine an Agent&apos;s disposition and intention; the composition and capabilities of Equipment and Facilities, and the surrounding landforms and weather conditions. (derived from http://en.wikipedia.org/wiki/Reconnaissance)</rdfs:comment>
        <rdfs:comment>Definition: An Act of Military Intelligence undertaken to obtain, by visual observation or other detection methods, information about activities and resources of an enemy or potential enemy and about the meteorological, hydrographic, or geographic characteristics of an area of operations (derived from The Army Universal Task List FM 7-15 February 2009).</rdfs:comment>
    </owl:Class>
    


    <!-- http://www.cubrc.org/ontologies/KDD/Mid/EventOntology#ActOfReconnaissanceInForce -->

    <owl:Class rdf:about="http://www.cubrc.org/ontologies/KDD/Mid/EventOntology#ActOfReconnaissanceInForce">
        <rdfs:label>Conduct a Reconnaissance in Force</rdfs:label>
        <rdfs:subClassOf rdf:resource="http://www.cubrc.org/ontologies/KDD/Mid/EventOntology#ActOfReconnaissance"/>
        <rdfs:comment>Definition: An Act of Reconnaissance that is a deliberate combat operation designed to discover or test the enemy�s strength, dispositions, and reactions or to obtain other information (derived from The Army Universal Task List FM 7-15 February 2009).</rdfs:comment>
    </owl:Class>
    


    <!-- http://www.cubrc.org/ontologies/KDD/Mid/EventOntology#ActOfReconnaissancePatrol -->

    <owl:Class rdf:about="http://www.cubrc.org/ontologies/KDD/Mid/EventOntology#ActOfReconnaissancePatrol">
        <rdfs:label>Reconnaissance Patrol</rdfs:label>
        <rdfs:subClassOf rdf:resource="http://www.cubrc.org/ontologies/KDD/Mid/EventOntology#ActOfReconnaissance"/>
        <rdfs:comment>Definition: An Act of Reconnaissance in which a detachment of ground, sea, or air forces gathers information about the enemy, terrain, or civil environment (derived from The Army Universal Task List FM 7-15 February 2009).</rdfs:comment>
    </owl:Class>
    


    <!-- http://www.cubrc.org/ontologies/KDD/Mid/EventOntology#ActOfReliefInPlace -->

    <owl:Class rdf:about="http://www.cubrc.org/ontologies/KDD/Mid/EventOntology#ActOfReliefInPlace">
        <rdfs:label>Conduct a Relief in Place</rdfs:label>
        <rdfs:subClassOf rdf:resource="http://www.cubrc.org/ontologies/KDD/Mid/EventOntology#ActOfForceManeuver"/>
        <rdfs:comment>Definition: An Act of Force Maneuver in which all or part of a unit is replaced in an area by an incoming unit (derived from The Army Universal Task List FM 7-15 February 2009).</rdfs:comment>
    </owl:Class>
    


    <!-- http://www.cubrc.org/ontologies/KDD/Mid/EventOntology#ActOfReligiousGroupAffiliation -->

    <owl:Class rdf:about="http://www.cubrc.org/ontologies/KDD/Mid/EventOntology#ActOfReligiousGroupAffiliation">
        <rdfs:label rdf:datatype="&xsd;string">Act Of Religious Group Affiliation</rdfs:label>
        <rdfs:subClassOf rdf:resource="http://www.cubrc.org/ontologies/KDD/Mid/EventOntology#ActOfAssociation"/>
        <rdfs:comment rdf:datatype="&xsd;string">Definition: An Act of Association wherein some Person belongs to some Religious Demonination or sub-Denomination.</rdfs:comment>
    </owl:Class>
    


    <!-- http://www.cubrc.org/ontologies/KDD/Mid/EventOntology#ActOfReligiousTrainingAcquisition -->

    <owl:Class rdf:about="http://www.cubrc.org/ontologies/KDD/Mid/EventOntology#ActOfReligiousTrainingAcquisition">
        <rdfs:label rdf:datatype="&xsd;string">Act Of Religious Training Acquisition</rdfs:label>
        <rdfs:subClassOf rdf:resource="http://www.cubrc.org/ontologies/KDD/Mid/EventOntology#ActOfTrainingAcquisition"/>
        <rdfs:comment rdf:datatype="&xsd;string">Definition: An Act of Training performed by an Agent by acquiring knowledge of the tenets and/or practices of a religion from an Agent or communication medium affiliated with a Religious Organization.</rdfs:comment>
    </owl:Class>
    


    <!-- http://www.cubrc.org/ontologies/KDD/Mid/EventOntology#ActOfReligiousTrainingInstruction -->

    <owl:Class rdf:about="http://www.cubrc.org/ontologies/KDD/Mid/EventOntology#ActOfReligiousTrainingInstruction">
        <rdfs:label rdf:datatype="&xsd;string">Act Of Religious Training Instruction</rdfs:label>
        <rdfs:subClassOf rdf:resource="http://www.cubrc.org/ontologies/KDD/Mid/EventOntology#ActOfTrainingInstruction"/>
        <rdfs:comment rdf:datatype="&xsd;string">Definition: An Act of Training performed by an Agent affiliated with some Religious Organization by imparting knowledge of the tenets and/or practices of a religion to an Agent either directly or indirectly through some communication medium.</rdfs:comment>
    </owl:Class>
    


    <!-- http://www.cubrc.org/ontologies/KDD/Mid/EventOntology#ActOfReligiousWorship -->

    <owl:Class rdf:about="http://www.cubrc.org/ontologies/KDD/Mid/EventOntology#ActOfReligiousWorship">
        <rdfs:label rdf:datatype="&xsd;string">Act of religious worship</rdfs:label>
        <rdfs:subClassOf rdf:resource="http://www.cubrc.org/ontologies/KDD/Mid/EventOntology#ActOfCeremony"/>
        <rdfs:comment rdf:datatype="&xsd;string">Definition: An Act of Ceremony wherein occurs acts of religious devotion usually directed towards a deity. (derived from http://en.wikipedia.org/wiki/Worship) (Sense Key: Worship%2:42:00 or Worship%1:04:00::)</rdfs:comment>
    </owl:Class>
    


    <!-- http://www.cubrc.org/ontologies/KDD/Mid/EventOntology#ActOfRemuneration -->

    <owl:Class rdf:about="http://www.cubrc.org/ontologies/KDD/Mid/EventOntology#ActOfRemuneration">
        <rdfs:label rdf:datatype="&xsd;string">Act Of Remuneration</rdfs:label>
        <rdfs:subClassOf rdf:resource="http://www.cubrc.org/ontologies/KDD/Mid/EventOntology#ActOfPurchasing"/>
        <rdfs:comment rdf:datatype="&xsd;string">Comment: Normally salary, but also commission, stock options, fringe benefits, etc.</rdfs:comment>
        <rdfs:comment rdf:datatype="&xsd;string">Definition: An Act of Purchasing wherein a Financial Instrument by Function or a Finanical Instrument by Role is used by an Agent (Employer) to compensate another Agent (Employee) for the services they perform for the Employer (derived from http://en.wikipedia.org/wiki/Remuneration)</rdfs:comment>
    </owl:Class>
    


    <!-- http://www.cubrc.org/ontologies/KDD/Mid/EventOntology#ActOfRenting -->

    <owl:Class rdf:about="http://www.cubrc.org/ontologies/KDD/Mid/EventOntology#ActOfRenting">
        <rdfs:subClassOf rdf:resource="http://www.cubrc.org/ontologies/KDD/Mid/EventOntology#ActOfPurchasing"/>
        <rdfs:comment rdf:datatype="&xsd;string">Definition: Renting is an agreement where a payment is made for the temporary use of a good, service or property owned by another (Source: http://en.wikipedia.org/wiki/Renting)</rdfs:comment>
    </owl:Class>
    


    <!-- http://www.cubrc.org/ontologies/KDD/Mid/EventOntology#ActOfRepayment -->

    <owl:Class rdf:about="http://www.cubrc.org/ontologies/KDD/Mid/EventOntology#ActOfRepayment">
        <rdfs:label rdf:datatype="&xsd;string">Act Of Repayment</rdfs:label>
        <rdfs:subClassOf rdf:resource="http://www.cubrc.org/ontologies/KDD/Mid/EventOntology#ActOfPurchasing"/>
        <rdfs:comment rdf:datatype="&xsd;string">Definition: An Act of Purchasing wherein a Financial Instrument by Function or a Finanical Instrument by Role is returned by an agent (Debtor) to another Agent (Creditor) to decrease the amount owed to the Creditor from an earlier ActOfLoaning (derived from http://en.wikipedia.org/wiki/Loan)</rdfs:comment>
    </owl:Class>
    


    <!-- http://www.cubrc.org/ontologies/KDD/Mid/EventOntology#ActOfReporting -->

    <owl:Class rdf:about="http://www.cubrc.org/ontologies/KDD/Mid/EventOntology#ActOfReporting">
        <rdfs:label rdf:datatype="&xsd;string">Act Of Reporting</rdfs:label>
        <rdfs:subClassOf rdf:resource="http://www.cubrc.org/ontologies/KDD/Mid/EventOntology#ActOfRepresentativeCommunication"/>
    </owl:Class>
    


    <!-- http://www.cubrc.org/ontologies/KDD/Mid/EventOntology#ActOfRepresentativeCommunication -->

    <owl:Class rdf:about="http://www.cubrc.org/ontologies/KDD/Mid/EventOntology#ActOfRepresentativeCommunication">
        <rdfs:label rdf:datatype="&xsd;string">Act Of Representative Communication</rdfs:label>
        <rdfs:subClassOf rdf:resource="http://www.cubrc.org/ontologies/KDD/Mid/EventOntology#ActOfPersonalCommunication"/>
        <rdfs:comment rdf:datatype="&xsd;string">Definition: An Act Of Personal Communication that commits a speaker to the truth of the expressed proposition. (loosely derived from John Searle&apos;s Speech Acts: An Essay in the Philosophy of Language)</rdfs:comment>
        <rdfs:comment rdf:datatype="&xsd;string">Examples: affirming, alleging, announcing, answering, attributing, claiming, classifying, concurring, confirming, conjecturing, denying, disagreeing, disclosing, disputing, identifying, informing, insisting, predicting, ranking, reporting, stating, stipulating</rdfs:comment>
    </owl:Class>
    


    <!-- http://www.cubrc.org/ontologies/KDD/Mid/EventOntology#ActOfRequesting -->

    <owl:Class rdf:about="http://www.cubrc.org/ontologies/KDD/Mid/EventOntology#ActOfRequesting">
        <rdfs:label rdf:datatype="&xsd;string">Act Of Requesting</rdfs:label>
        <rdfs:subClassOf rdf:resource="http://www.cubrc.org/ontologies/KDD/Mid/EventOntology#ActOfDirectiveCommunication"/>
    </owl:Class>
    


    <!-- http://www.cubrc.org/ontologies/KDD/Mid/EventOntology#ActOfRoadMarch -->

    <owl:Class rdf:about="http://www.cubrc.org/ontologies/KDD/Mid/EventOntology#ActOfRoadMarch">
        <rdfs:label>Road March</rdfs:label>
        <rdfs:subClassOf rdf:resource="http://www.cubrc.org/ontologies/KDD/Mid/EventOntology#ActOfForceMovement"/>
        <rdfs:comment>Definition: An Act Of Force Movement in which a rapid movement is used to relocate units within an Area of Operations in order to prepare for combat operations (derived from The Army Universal Task List FM 7-15 February 2009).</rdfs:comment>
    </owl:Class>
    


    <!-- http://www.cubrc.org/ontologies/KDD/Mid/EventOntology#ActOfRobbery -->

    <owl:Class rdf:about="http://www.cubrc.org/ontologies/KDD/Mid/EventOntology#ActOfRobbery">
        <rdfs:label>Act Of Robbery</rdfs:label>
        <rdfs:subClassOf rdf:resource="http://www.cubrc.org/ontologies/KDD/Mid/EventOntology#CriminalActAgainstProperty"/>
        <rdfs:comment>Definition: A Criminal Act Against Property  involving a trespassory taking and carrying away of the personal property of another with the intent to steal from the person or presence of the victim by force or threat of force. (derived from http:/en.wikipedia.org/wiki/Robbery)</rdfs:comment>
    </owl:Class>
    


    <!-- http://www.cubrc.org/ontologies/KDD/Mid/EventOntology#ActOfRouteClearance -->

    <owl:Class rdf:about="http://www.cubrc.org/ontologies/KDD/Mid/EventOntology#ActOfRouteClearance">
        <rdfs:label>Conduct Route Clearance</rdfs:label>
        <rdfs:subClassOf rdf:resource="http://www.cubrc.org/ontologies/KDD/Mid/EventOntology#ActOfClearing"/>
        <rdfs:comment>Definition: An Act of Clearance is a combined arms operation conducted to remove mines and other obstacles along preexisting roads and trails (derived from The Army Universal Task List FM 7-15 February 2009).</rdfs:comment>
    </owl:Class>
    


    <!-- http://www.cubrc.org/ontologies/KDD/Mid/EventOntology#ActOfRouteReconnaissance -->

    <owl:Class rdf:about="http://www.cubrc.org/ontologies/KDD/Mid/EventOntology#ActOfRouteReconnaissance">
        <rdfs:label>Conduct a Route Reconnaissance</rdfs:label>
        <rdfs:subClassOf rdf:resource="http://www.cubrc.org/ontologies/KDD/Mid/EventOntology#ActOfReconnaissance"/>
        <rdfs:comment>Definition: An Act of Route Reconnaissance in which a reconnaissance operation is focused along a specific route�such as a road, railway, or waterway�to provide new or updated information on route conditions and activities (derived from The Army Universal Task List FM 7-15 February 2009).</rdfs:comment>
    </owl:Class>
    


    <!-- http://www.cubrc.org/ontologies/KDD/Mid/EventOntology#ActOfRouteSecurityOperation -->

    <owl:Class rdf:about="http://www.cubrc.org/ontologies/KDD/Mid/EventOntology#ActOfRouteSecurityOperation">
        <rdfs:label>Conduct Route Security Operation</rdfs:label>
        <rdfs:subClassOf rdf:resource="http://www.cubrc.org/ontologies/KDD/Mid/EventOntology#ActOfOperationalAreaSecurity"/>
        <rdfs:comment>Definition: An Act of Operational Area Security in which enemy ground forces are prevented from moving into direct fire range of the protected route (including highway, pipeline, rail, and water) . Route security operations are defensive in nature and terrain-oriented (derived from The Army Universal Task List FM 7-15 February 2009).</rdfs:comment>
    </owl:Class>
    


    <!-- http://www.cubrc.org/ontologies/KDD/Mid/EventOntology#ActOfSentencing -->

    <owl:Class rdf:about="http://www.cubrc.org/ontologies/KDD/Mid/EventOntology#ActOfSentencing">
        <rdfs:label>Act Of Sentencing</rdfs:label>
        <rdfs:subClassOf rdf:resource="http://www.cubrc.org/ontologies/KDD/Mid/EventOntology#LegalSystemAct"/>
        <rdfs:comment>Definition: A Legal System Act in which a punishment is ordered by a court for a person that has been convicted of committing a Criminal Act. (derived from http://www.id.uscourts.gov/glossary.htm)</rdfs:comment>
    </owl:Class>
    


    <!-- http://www.cubrc.org/ontologies/KDD/Mid/EventOntology#ActOfSexTrafficking -->

    <owl:Class rdf:about="http://www.cubrc.org/ontologies/KDD/Mid/EventOntology#ActOfSexTrafficking">
        <rdfs:label rdf:datatype="&xsd;string">Definition: An Act of Human Trafficking in which a commercial sex act is induced by force, fraud, or coercion, or in which the person induced to perform such an act is under the age of 18 years. (Source: http://www.acf.hhs.gov/programs/orr/resource/fact-sheet-sex-trafficking-english)</rdfs:label>
        <rdfs:subClassOf rdf:resource="http://www.cubrc.org/ontologies/KDD/Mid/EventOntology#ActOfHumanTrafficking"/>
    </owl:Class>
    


    <!-- http://www.cubrc.org/ontologies/KDD/Mid/EventOntology#ActOfSexualAssault -->

    <owl:Class rdf:about="http://www.cubrc.org/ontologies/KDD/Mid/EventOntology#ActOfSexualAssault">
        <rdfs:label>Act Of Sexual Assault</rdfs:label>
        <rdfs:subClassOf rdf:resource="http://www.cubrc.org/ontologies/KDD/Mid/EventOntology#ActOfAssault"/>
        <rdfs:comment>Definition: An Act of Assault of a sexual nature on another person. (derived from http://en.wikipedia.org/wiki/Sexual_assault)</rdfs:comment>
    </owl:Class>
    


    <!-- http://www.cubrc.org/ontologies/KDD/Mid/EventOntology#ActOfSmuggling -->

    <owl:Class rdf:about="http://www.cubrc.org/ontologies/KDD/Mid/EventOntology#ActOfSmuggling">
        <rdfs:subClassOf rdf:resource="http://www.cubrc.org/ontologies/KDD/Mid/EventOntology#CriminalAct"/>
        <rdfs:comment rdf:datatype="&xsd;string">Definition: A criminal act in which goods or persons are illegally transported out of a building, into a prison, or across an international border, in violation of applicable laws or other regulations. (Source: http://en.wikipedia.org/wiki/Smuggling)</rdfs:comment>
    </owl:Class>
    


    <!-- http://www.cubrc.org/ontologies/KDD/Mid/EventOntology#ActOfSniperCountermeasure -->

    <owl:Class rdf:about="http://www.cubrc.org/ontologies/KDD/Mid/EventOntology#ActOfSniperCountermeasure">
        <rdfs:label>Conduct Sniper Countermeasure</rdfs:label>
        <rdfs:subClassOf rdf:resource="http://www.cubrc.org/ontologies/KDD/Mid/EventOntology#ActOfForceManeuver"/>
        <rdfs:comment>Definition: An Act of Force Maneuver in which a sniper is detected and destroyed before firing, engaged and neutralized after firing, prevented from acquiring a clear target or in some other way prevented from inflicting casualties (derived from The Army Universal Task List FM 7-15 February 2009).</rdfs:comment>
    </owl:Class>
    


    <!-- http://www.cubrc.org/ontologies/KDD/Mid/EventOntology#ActOfSocialGroupMembership -->

    <owl:Class rdf:about="http://www.cubrc.org/ontologies/KDD/Mid/EventOntology#ActOfSocialGroupMembership">
        <rdfs:label rdf:datatype="&xsd;string">Act Of Social Group Membership</rdfs:label>
        <rdfs:subClassOf rdf:resource="http://www.cubrc.org/ontologies/KDD/Mid/EventOntology#ActOfAssociation"/>
        <rdfs:comment rdf:datatype="&xsd;string">Definition: An Act of Association wherein a Person belongs to some Social Group</rdfs:comment>
    </owl:Class>
    


    <!-- http://www.cubrc.org/ontologies/KDD/Mid/EventOntology#ActOfSocialMovement -->

    <owl:Class rdf:about="http://www.cubrc.org/ontologies/KDD/Mid/EventOntology#ActOfSocialMovement">
        <rdfs:label rdf:datatype="&xsd;string">Act of social movement</rdfs:label>
        <rdfs:subClassOf rdf:resource="http://www.cubrc.org/ontologies/KDD/Mid/EventOntology#SocialAct"/>
        <rdfs:comment rdf:datatype="&xsd;string">Definition: A Social Act composed of a series of performances, displays and campaigns directed at implementing, resisting or undoing a change in society (derived from http://en.wikipedia.org/wiki/Social_movement)</rdfs:comment>
    </owl:Class>
    


    <!-- http://www.cubrc.org/ontologies/KDD/Mid/EventOntology#ActOfSolicitation -->

    <owl:Class rdf:about="http://www.cubrc.org/ontologies/KDD/Mid/EventOntology#ActOfSolicitation">
        <rdfs:label>Act Of Solicitation</rdfs:label>
        <rdfs:subClassOf rdf:resource="http://www.cubrc.org/ontologies/KDD/Mid/EventOntology#InchoateCriminalAct"/>
        <rdfs:comment>Definition: An Inchoate Criminal Act of a person offering money or other inducement to another to commit a crime with the specific intent that the person solicited commit the crime. (derived from http://en.wikipedia.org/wiki/Solicitation)</rdfs:comment>
    </owl:Class>
    


    <!-- http://www.cubrc.org/ontologies/KDD/Mid/EventOntology#ActOfSpaceOperationsIntegration -->

    <owl:Class rdf:about="http://www.cubrc.org/ontologies/KDD/Mid/EventOntology#ActOfSpaceOperationsIntegration">
        <rdfs:label>Integrate  Space Operations</rdfs:label>
        <rdfs:subClassOf rdf:resource="http://www.cubrc.org/ontologies/KDD/Mid/EventOntology#ActOfCommandAndControlWarfighting"/>
        <rdfs:comment>Definition: An Act of Command and Control Warfighting in which space capabilities are integrated thoroughly into the force structure to enable Army operations, and are essential for mission accomplishment. Staffs down to brigade level integrate space capabilities and vulnerabilities into their mission analysis process (derived from The Army Universal Task List FM 7-15 February 2009).</rdfs:comment>
    </owl:Class>
    


    <!-- http://www.cubrc.org/ontologies/KDD/Mid/EventOntology#ActOfStabilityOperation -->

    <owl:Class rdf:about="http://www.cubrc.org/ontologies/KDD/Mid/EventOntology#ActOfStabilityOperation">
        <rdfs:label>Conduct Stability Operation</rdfs:label>
        <rdfs:subClassOf rdf:resource="http://www.cubrc.org/ontologies/KDD/Mid/EventOntology#ActOfMilitaryForce"/>
        <rdfs:comment>Definition: An Act of Military Force that encompasses various military missions, tasks, and activities conducted outside the United States in coordination with elements of combat to maintain or reestablish a safe and secure environment, provide essential government services, emergency infrastructure reconstruction, and humanitarian relief (derived from The Army Universal Task List FM 7-15 February 2009).</rdfs:comment>
    </owl:Class>
    


    <!-- http://www.cubrc.org/ontologies/KDD/Mid/EventOntology#ActOfSuicide -->

    <owl:Class rdf:about="http://www.cubrc.org/ontologies/KDD/Mid/EventOntology#ActOfSuicide">
        <rdfs:label rdf:datatype="&xsd;string">Suicide</rdfs:label>
        <rdfs:subClassOf rdf:resource="http://www.cubrc.org/ontologies/KDD/Mid/EventOntology#ActOfViolence"/>
        <rdfs:comment rdf:datatype="&xsd;string">An Act of Violence in which some Agent causes their own death.</rdfs:comment>
    </owl:Class>
    


    <!-- http://www.cubrc.org/ontologies/KDD/Mid/EventOntology#ActOfSupplyProvision -->

    <owl:Class rdf:about="http://www.cubrc.org/ontologies/KDD/Mid/EventOntology#ActOfSupplyProvision">
        <rdfs:label>Supply Support</rdfs:label>
        <rdfs:subClassOf rdf:resource="http://www.cubrc.org/ontologies/KDD/Mid/EventOntology#ActOfLogisticSupport"/>
        <rdfs:comment>Definition: An Act of Logistic Support in which any type of supply necessary to equip, maintain, and operate military units is issued, delivered or received (derived from The Army Universal Task List FM 7-15 February 2009).</rdfs:comment>
    </owl:Class>
    


    <!-- http://www.cubrc.org/ontologies/KDD/Mid/EventOntology#ActOfSurfaceToAirFire -->

    <owl:Class rdf:about="http://www.cubrc.org/ontologies/KDD/Mid/EventOntology#ActOfSurfaceToAirFire">
        <rdfs:label>Surface to Air Attack</rdfs:label>
        <rdfs:subClassOf rdf:resource="http://www.cubrc.org/ontologies/KDD/Mid/EventOntology#ActOfIndirectFire"/>
        <rdfs:comment>Definition: An Act of Indirect Fire in which some ground-based, indirect-fire weapon system is used to destroy aircraft or missiles (derived from The Army Universal Task List FM 7-15 February 2009).</rdfs:comment>
    </owl:Class>
    


    <!-- http://www.cubrc.org/ontologies/KDD/Mid/EventOntology#ActOfSurfaceToSurfaceFire -->

    <owl:Class rdf:about="http://www.cubrc.org/ontologies/KDD/Mid/EventOntology#ActOfSurfaceToSurfaceFire">
        <rdfs:label>Surface to Surface Attack</rdfs:label>
        <rdfs:subClassOf rdf:resource="http://www.cubrc.org/ontologies/KDD/Mid/EventOntology#ActOfIndirectFire"/>
        <rdfs:comment>Definition: An Act of Indirect Fire in which some ground-based, indirect-fire weapon system is used to destroy, suppress, or neutralize enemy equipment (including aircraft on the ground), materiel, personnel, fortifications, and facilities (derived from The Army Universal Task List FM 7-15 February 2009).</rdfs:comment>
    </owl:Class>
    


    <!-- http://www.cubrc.org/ontologies/KDD/Mid/EventOntology#ActOfSurveillance -->

    <owl:Class rdf:about="http://www.cubrc.org/ontologies/KDD/Mid/EventOntology#ActOfSurveillance">
        <rdfs:label>Conduct Surveillance</rdfs:label>
        <rdfs:subClassOf rdf:resource="http://www.cubrc.org/ontologies/KDD/Mid/EventOntology#ActOfIntelligenceSurveillanceAndReconnaisance"/>
        <rdfs:comment>Definition: An Act of Military Intelligence that is the systematic observation of aerospace, surface, or subsurface areas, places, persons, or things by visual, aural, electronic, photographic, or other means (derived from The Army Universal Task List FM 7-15 February 2009).</rdfs:comment>
    </owl:Class>
    


    <!-- http://www.cubrc.org/ontologies/KDD/Mid/EventOntology#ActOfSurvivabilityOperation -->

    <owl:Class rdf:about="http://www.cubrc.org/ontologies/KDD/Mid/EventOntology#ActOfSurvivabilityOperation">
        <rdfs:label>Survivability Operation</rdfs:label>
        <rdfs:subClassOf rdf:resource="http://www.cubrc.org/ontologies/KDD/Mid/EventOntology#ActOfProtectionWarfighting"/>
        <rdfs:comment>Definition: An Act of Military Force which includes all aspects of protecting personnel, weapons, and supplies while simultaneously deceiving the enemy. Examples include building a good defense; employing frequent movement; using concealment, deception, and camouflage; and constructing fighting and protective positions for both individuals and equipment (derived from The Army Universal Task List FM 7-15 February 2009).</rdfs:comment>
    </owl:Class>
    


    <!-- http://www.cubrc.org/ontologies/KDD/Mid/EventOntology#ActOfSustainmentWarfighting -->

    <owl:Class rdf:about="http://www.cubrc.org/ontologies/KDD/Mid/EventOntology#ActOfSustainmentWarfighting">
        <rdfs:label>Realize the Sustainment Warfighting Function</rdfs:label>
        <rdfs:subClassOf rdf:resource="http://www.cubrc.org/ontologies/KDD/Mid/EventOntology#ActOfMilitaryForce"/>
        <rdfs:comment>Definition: An Act of Military Force that provides support and services to ensure freedom of action, extend operational reach, and prolong endurance (derived from The Army Universal Task List FM 7-15 February 2009).</rdfs:comment>
    </owl:Class>
    


    <!-- http://www.cubrc.org/ontologies/KDD/Mid/EventOntology#ActOfTacticalConvoy -->

    <owl:Class rdf:about="http://www.cubrc.org/ontologies/KDD/Mid/EventOntology#ActOfTacticalConvoy">
        <rdfs:label>Tactical Convoy</rdfs:label>
        <rdfs:subClassOf rdf:resource="http://www.cubrc.org/ontologies/KDD/Mid/EventOntology#ActOfForceMovement"/>
        <rdfs:comment>Definition: An Act of Force Movement in which forces and materiel are moved overland from one location on the battlefield to another while maintaining the ability to aggressively respond to enemy attempts to impede, disrupt, or destroy elements of the convoy (derived from The Army Universal Task List FM 7-15 February 2009).</rdfs:comment>
    </owl:Class>
    


    <!-- http://www.cubrc.org/ontologies/KDD/Mid/EventOntology#ActOfTacticalMissionTask -->

    <owl:Class rdf:about="http://www.cubrc.org/ontologies/KDD/Mid/EventOntology#ActOfTacticalMissionTask">
        <rdfs:label>Conduct Tactical Mission Tasks</rdfs:label>
        <rdfs:subClassOf rdf:resource="http://www.cubrc.org/ontologies/KDD/Mid/EventOntology#ActOfMilitaryForce"/>
        <rdfs:comment>Definition: An Act of Military Force that are the lethal and nonlethal results or effects the commander wants to generate or create to accomplish the mission. (derived from The Army Universal Task List FM 7-15 February 2009).</rdfs:comment>
    </owl:Class>
    


    <!-- http://www.cubrc.org/ontologies/KDD/Mid/EventOntology#ActOfTaxEvasion -->

    <owl:Class rdf:about="http://www.cubrc.org/ontologies/KDD/Mid/EventOntology#ActOfTaxEvasion">
        <rdfs:label>Act of Tax Evasion</rdfs:label>
        <rdfs:subClassOf rdf:resource="http://www.cubrc.org/ontologies/KDD/Mid/EventOntology#ActOfFraud"/>
        <rdfs:comment rdf:datatype="&xsd;string">Definition: An Act of Fraud that is very broadly defined to include a person&apos;s attempt in any manner to evade or defeat any tax imposed by [Title 26] or payment thereof. (Source: http://www.irs.gov/pub/irs-utl/tax_crimes_handbook.pdf)</rdfs:comment>
    </owl:Class>
    


    <!-- http://www.cubrc.org/ontologies/KDD/Mid/EventOntology#ActOfTerrorism -->

    <owl:Class rdf:about="http://www.cubrc.org/ontologies/KDD/Mid/EventOntology#ActOfTerrorism">
        <rdfs:label rdf:datatype="&xsd;string">Act Of Terrorism</rdfs:label>
        <rdfs:subClassOf rdf:resource="http://www.cubrc.org/ontologies/KDD/Mid/EventOntology#IntentionalAct"/>
        <rdfs:subClassOf>
            <owl:Class>
                <owl:unionOf rdf:parseType="Collection">
                    <rdf:Description rdf:about="http://www.cubrc.org/ontologies/KDD/Mid/EventOntology#ActOfViolence"/>
                    <rdf:Description rdf:about="http://www.cubrc.org/ontologies/KDD/Mid/EventOntology#CriminalAct"/>
                    <owl:Class>
                        <owl:intersectionOf rdf:parseType="Collection">
                            <rdf:Description rdf:about="http://www.cubrc.org/ontologies/KDD/Mid/EventOntology#ActOfWeaponUse"/>
                            <owl:Restriction>
                                <owl:onProperty rdf:resource="&ero;is_cause_of"/>
                                <owl:someValuesFrom rdf:resource="http://www.cubrc.org/ontologies/KDD/Mid/EventOntology#Damage"/>
                            </owl:Restriction>
                        </owl:intersectionOf>
                    </owl:Class>
                </owl:unionOf>
            </owl:Class>
        </rdfs:subClassOf>
        <rdfs:comment rdf:datatype="&xsd;string">An Act of Violence which creates fear and which is prescribed by religious, political or ideological objectives, and which deliberately target or disregard the safety of civilians and are committed by members of non-government organizations (derived from http://en.wikipedia.org/wiki/Terrorism)</rdfs:comment>
    </owl:Class>
    


    <!-- http://www.cubrc.org/ontologies/KDD/Mid/EventOntology#ActOfTerroristTrainingAcquisition -->

    <owl:Class rdf:about="http://www.cubrc.org/ontologies/KDD/Mid/EventOntology#ActOfTerroristTrainingAcquisition">
        <rdfs:label rdf:datatype="&xsd;string">Act Of Terrorist Training Acquisition</rdfs:label>
        <rdfs:subClassOf rdf:resource="http://www.cubrc.org/ontologies/KDD/Mid/EventOntology#ActOfTrainingAcquisition"/>
        <rdfs:comment rdf:datatype="&xsd;string">Definition: An Act of Training performed by an Agent by acquiring knowledge of the tactics, techniques, and/or strategies of the use of violence against civilians in order to attain goals that are political, religous, or ideological in nature from an Agent or communication medium affiliated with a Terrorist Organization. (derived from http://wordnetweb.princeton.edu/perl/webwn?s=terrorism)</rdfs:comment>
    </owl:Class>
    


    <!-- http://www.cubrc.org/ontologies/KDD/Mid/EventOntology#ActOfTerroristTrainingInstruction -->

    <owl:Class rdf:about="http://www.cubrc.org/ontologies/KDD/Mid/EventOntology#ActOfTerroristTrainingInstruction">
        <rdfs:label rdf:datatype="&xsd;string">Act Of Terrorist Training Instruction</rdfs:label>
        <rdfs:subClassOf rdf:resource="http://www.cubrc.org/ontologies/KDD/Mid/EventOntology#ActOfTrainingInstruction"/>
        <rdfs:comment rdf:datatype="&xsd;string">Definition: An Act of Training performed by an Agent affiliated with some Terrorist Organization by imparting knowledge of the tactics, techniques, and/or strategies of the use of violence against civilians in order to attain goals that are political, religous, or ideological in nature to an Agent either directly or indirectly through some communication medium. (derived from http://wordnetweb.princeton.edu/perl/webwn?s=terrorism)</rdfs:comment>
    </owl:Class>
    


    <!-- http://www.cubrc.org/ontologies/KDD/Mid/EventOntology#ActOfTestifying -->

    <owl:Class rdf:about="http://www.cubrc.org/ontologies/KDD/Mid/EventOntology#ActOfTestifying">
        <rdfs:label rdf:datatype="&xsd;string">Act Of Asserting</rdfs:label>
        <rdfs:subClassOf rdf:resource="http://www.cubrc.org/ontologies/KDD/Mid/EventOntology#ActOfRepresentativeCommunication"/>
    </owl:Class>
    


    <!-- http://www.cubrc.org/ontologies/KDD/Mid/EventOntology#ActOfThanking -->

    <owl:Class rdf:about="http://www.cubrc.org/ontologies/KDD/Mid/EventOntology#ActOfThanking">
        <rdfs:label rdf:datatype="&xsd;string">Act Of Thanking</rdfs:label>
        <rdfs:subClassOf rdf:resource="http://www.cubrc.org/ontologies/KDD/Mid/EventOntology#ActOfExpressiveCommunication"/>
    </owl:Class>
    


    <!-- http://www.cubrc.org/ontologies/KDD/Mid/EventOntology#ActOfToolUse -->

    <owl:Class rdf:about="http://www.cubrc.org/ontologies/KDD/Mid/EventOntology#ActOfToolUse">
        <rdfs:label rdf:datatype="&xsd;string">Act Of Tool Use</rdfs:label>
        <rdfs:subClassOf rdf:resource="http://www.cubrc.org/ontologies/KDD/Mid/EventOntology#ActOfInstrumentUse"/>
        <rdfs:comment rdf:datatype="&xsd;string">An Act Of Instrument Use in which some Agent uses some Tool</rdfs:comment>
    </owl:Class>
    


    <!-- http://www.cubrc.org/ontologies/KDD/Mid/EventOntology#ActOfTraining -->

    <owl:Class rdf:about="http://www.cubrc.org/ontologies/KDD/Mid/EventOntology#ActOfTraining">
        <rdfs:label rdf:datatype="&xsd;string">Act Of Training</rdfs:label>
        <rdfs:subClassOf rdf:resource="http://www.cubrc.org/ontologies/KDD/Mid/EventOntology#IntentionalAct"/>
        <rdfs:comment rdf:datatype="&xsd;string">Definition: An Intentional Act in which knowledge, skills or values are imparted from one (or more) Agents to at least one other Agent. (derived from http://en.wikipedia.org/wiki/Education).</rdfs:comment>
    </owl:Class>
    


    <!-- http://www.cubrc.org/ontologies/KDD/Mid/EventOntology#ActOfTrainingAcquisition -->

    <owl:Class rdf:about="http://www.cubrc.org/ontologies/KDD/Mid/EventOntology#ActOfTrainingAcquisition">
        <rdfs:label rdf:datatype="&xsd;string">Act Of Training Acquisition</rdfs:label>
        <rdfs:subClassOf rdf:resource="http://www.cubrc.org/ontologies/KDD/Mid/EventOntology#ActOfTraining"/>
        <rdfs:comment rdf:datatype="&xsd;string">Definition: An Act of Training performed by an Agent by acquiring knowledge from another Agent.</rdfs:comment>
    </owl:Class>
    


    <!-- http://www.cubrc.org/ontologies/KDD/Mid/EventOntology#ActOfTrainingInstruction -->

    <owl:Class rdf:about="http://www.cubrc.org/ontologies/KDD/Mid/EventOntology#ActOfTrainingInstruction">
        <rdfs:label rdf:datatype="&xsd;string">Act Of Training Instruction</rdfs:label>
        <rdfs:subClassOf rdf:resource="http://www.cubrc.org/ontologies/KDD/Mid/EventOntology#ActOfTraining"/>
        <rdfs:comment rdf:datatype="&xsd;string">Definition: An Act of Training performed by an Agent by imparting knowledge to another Agent.</rdfs:comment>
    </owl:Class>
    


    <!-- http://www.cubrc.org/ontologies/KDD/Mid/EventOntology#ActOfTransportationSupport -->

    <owl:Class rdf:about="http://www.cubrc.org/ontologies/KDD/Mid/EventOntology#ActOfTransportationSupport">
        <rdfs:label>Transportation Support</rdfs:label>
        <rdfs:subClassOf rdf:resource="http://www.cubrc.org/ontologies/KDD/Mid/EventOntology#ActOfLogisticSupport"/>
        <rdfs:comment>Definition: An Act of Logistic Support in which equipment, materiel, or personnel are moved by towing, self-propulsion, or any means of carrier such as railways, highways, waterways, oceans, joint logistics over-the-shore, and airways (derived from The Army Universal Task List FM 7-15 February 2009).</rdfs:comment>
    </owl:Class>
    


    <!-- http://www.cubrc.org/ontologies/KDD/Mid/EventOntology#ActOfTravel -->

    <owl:Class rdf:about="http://www.cubrc.org/ontologies/KDD/Mid/EventOntology#ActOfTravel">
        <rdfs:label rdf:datatype="&xsd;string">Act Of Travel</rdfs:label>
        <rdfs:subClassOf rdf:resource="http://www.cubrc.org/ontologies/KDD/Mid/EventOntology#ActOfMovement"/>
        <rdfs:comment rdf:datatype="&xsd;string">Definition: An Act Of Movement wherein Persons move between relatively distant geographical locations for any purpose and any duration, with or without any means of transport. (derived from http://en.wikipedia.org/wiki/Travel)</rdfs:comment>
    </owl:Class>
    


    <!-- http://www.cubrc.org/ontologies/KDD/Mid/EventOntology#ActOfTurningManeuver -->

    <owl:Class rdf:about="http://www.cubrc.org/ontologies/KDD/Mid/EventOntology#ActOfTurningManeuver">
        <rdfs:label>Conduct a Turning Movement</rdfs:label>
        <rdfs:subClassOf rdf:resource="http://www.cubrc.org/ontologies/KDD/Mid/EventOntology#ActOfForceManeuver"/>
        <rdfs:comment>Definition: An Act of Force Maneuver in which an attacking force seeks to avoid the enemy�s principal defensive positions by seizing objectives to the enemy rear and causing the enemy to move out of his current positions or divert major forces to meet the threat (derived from The Army Universal Task List FM 7-15 February 2009).</rdfs:comment>
    </owl:Class>
    


    <!-- http://www.cubrc.org/ontologies/KDD/Mid/EventOntology#ActOfUnlading -->

    <owl:Class rdf:about="http://www.cubrc.org/ontologies/KDD/Mid/EventOntology#ActOfUnlading">
        <rdfs:label xml:lang="en">ActOfUnlading</rdfs:label>
        <rdfs:subClassOf rdf:resource="http://www.cubrc.org/ontologies/KDD/Mid/EventOntology#ActOfFreightHandling"/>
    </owl:Class>
    


    <!-- http://www.cubrc.org/ontologies/KDD/Mid/EventOntology#ActOfUnlawfulFlightFromJustice -->

    <owl:Class rdf:about="http://www.cubrc.org/ontologies/KDD/Mid/EventOntology#ActOfUnlawfulFlightFromJustice">
        <rdfs:label>Act Of Unlawful Flight From Justice</rdfs:label>
        <rdfs:subClassOf rdf:resource="http://www.cubrc.org/ontologies/KDD/Mid/EventOntology#CriminalActAgainstJustice"/>
        <rdfs:comment>Definition: A Criminal Act Against Justice wherein the offender travels to avoid prosecution for a crime or providing testimony in criminal proceedings</rdfs:comment>
    </owl:Class>
    


    <!-- http://www.cubrc.org/ontologies/KDD/Mid/EventOntology#ActOfVandalism -->

    <owl:Class rdf:about="http://www.cubrc.org/ontologies/KDD/Mid/EventOntology#ActOfVandalism">
        <rdfs:subClassOf rdf:resource="http://www.cubrc.org/ontologies/KDD/Mid/EventOntology#CriminalActAgainstProperty"/>
        <rdfs:comment rdf:datatype="&xsd;string">Definition: A Criminal Act Against Property in which public or private property is willfully or maliciously destroyed, injured, disfigured, or defaced, without the consent of the owner or person having custody or control by cutting, tearing, breaking, marking, painting, drawing, covering with filth, or any other such means as may be specified by local law. Attempts are included. (Source: http://www2.fbi.gov/ucr/cius2009/about/offense_definitions.html)</rdfs:comment>
    </owl:Class>
    


    <!-- http://www.cubrc.org/ontologies/KDD/Mid/EventOntology#ActOfVehicleRegistration -->

    <owl:Class rdf:about="http://www.cubrc.org/ontologies/KDD/Mid/EventOntology#ActOfVehicleRegistration">
        <rdfs:label xml:lang="en">ActOfVehicleRegistration</rdfs:label>
        <rdfs:subClassOf rdf:resource="http://www.cubrc.org/ontologies/KDD/Mid/EventOntology#ActOfGovernment"/>
    </owl:Class>
    


    <!-- http://www.cubrc.org/ontologies/KDD/Mid/EventOntology#ActOfVehicleUse -->

    <owl:Class rdf:about="http://www.cubrc.org/ontologies/KDD/Mid/EventOntology#ActOfVehicleUse">
        <rdfs:label rdf:datatype="&xsd;string">Act Of Vehicle Use</rdfs:label>
        <rdfs:subClassOf rdf:resource="http://www.cubrc.org/ontologies/KDD/Mid/EventOntology#ActOfInstrumentUse"/>
        <rdfs:comment rdf:datatype="&xsd;string">An Act Of Instrument Use in which some Agent uses some Vehicle.</rdfs:comment>
    </owl:Class>
    


    <!-- http://www.cubrc.org/ontologies/KDD/Mid/EventOntology#ActOfViolence -->

    <owl:Class rdf:about="http://www.cubrc.org/ontologies/KDD/Mid/EventOntology#ActOfViolence">
        <rdfs:label rdf:datatype="&xsd;string">Act Of Violence</rdfs:label>
        <rdfs:subClassOf rdf:resource="http://www.cubrc.org/ontologies/KDD/Mid/EventOntology#IntentionalAct"/>
        <rdfs:comment rdf:datatype="&xsd;string">An Intentional Act of causing harm to oneself or to another through the use of physical or verbal force (derived from http://en.wikipedia.org/wiki/Violence).</rdfs:comment>
    </owl:Class>
    


    <!-- http://www.cubrc.org/ontologies/KDD/Mid/EventOntology#ActOfVocationalTrainingAcquisition -->

    <owl:Class rdf:about="http://www.cubrc.org/ontologies/KDD/Mid/EventOntology#ActOfVocationalTrainingAcquisition">
        <rdfs:label rdf:datatype="&xsd;string">Act Of Vocational Training Acquisition</rdfs:label>
        <rdfs:subClassOf rdf:resource="http://www.cubrc.org/ontologies/KDD/Mid/EventOntology#ActOfTrainingAcquisition"/>
        <rdfs:comment rdf:datatype="&xsd;string">Definition: An Act of Training performed by an Agent by acquiring skills required for a specific occupation in industry, agriculture or trade from an Agent or communication medium affiliated with a Vocational School, Technical School, Trade Organization, or Industry Educational Program Provider. (derived from http://wordnetweb.princeton.edu/perl/webwn?s=vocational%20training)</rdfs:comment>
    </owl:Class>
    


    <!-- http://www.cubrc.org/ontologies/KDD/Mid/EventOntology#ActOfVocationalTrainingInstruction -->

    <owl:Class rdf:about="http://www.cubrc.org/ontologies/KDD/Mid/EventOntology#ActOfVocationalTrainingInstruction">
        <rdfs:label rdf:datatype="&xsd;string">Act Of Vocational Training Instruction</rdfs:label>
        <rdfs:subClassOf rdf:resource="http://www.cubrc.org/ontologies/KDD/Mid/EventOntology#ActOfTrainingInstruction"/>
        <rdfs:comment rdf:datatype="&xsd;string">Definition: An Act of Training performed by an Agent affiliated with a Vocational School, Technical School, Trade Organization, or Industry Educational Program Provider by imparting skills required for a specific occupation in industry, agriculture or trade to an Agent either directly or indirectly through some communication medium. (derived from http://wordnetweb.princeton.edu/perl/webwn?s=vocational%20training)</rdfs:comment>
    </owl:Class>
    


    <!-- http://www.cubrc.org/ontologies/KDD/Mid/EventOntology#ActOfVoluntaryManslaughter -->

    <owl:Class rdf:about="http://www.cubrc.org/ontologies/KDD/Mid/EventOntology#ActOfVoluntaryManslaughter">
        <rdfs:label>Act Of Voluntary Manslaughter</rdfs:label>
        <rdfs:subClassOf rdf:resource="http://www.cubrc.org/ontologies/KDD/Mid/EventOntology#ActOfManslaughter"/>
        <rdfs:comment>Definition: An Act of Manslaughter that occurs either when the offender kills with malice aforethought (intention to kill or cause serious harm), but there are mitigating circumstances which reduce culpability, or when the offender kills only with an intent to cause serious bodily harm (derived from http://en.wikipedia.org/wiki/Manslaughter).</rdfs:comment>
    </owl:Class>
    


    <!-- http://www.cubrc.org/ontologies/KDD/Mid/EventOntology#ActOfVolunteering -->

    <owl:Class rdf:about="http://www.cubrc.org/ontologies/KDD/Mid/EventOntology#ActOfVolunteering">
        <rdfs:label rdf:datatype="&xsd;string">Act Of Volunteering</rdfs:label>
        <rdfs:subClassOf rdf:resource="http://www.cubrc.org/ontologies/KDD/Mid/EventOntology#ActOfCommissiveCommunication"/>
    </owl:Class>
    


    <!-- http://www.cubrc.org/ontologies/KDD/Mid/EventOntology#ActOfWarning -->

    <owl:Class rdf:about="http://www.cubrc.org/ontologies/KDD/Mid/EventOntology#ActOfWarning">
        <rdfs:label rdf:datatype="&xsd;string">Act Of Warning</rdfs:label>
        <rdfs:subClassOf rdf:resource="http://www.cubrc.org/ontologies/KDD/Mid/EventOntology#ActOfDirectiveCommunication"/>
    </owl:Class>
    


    <!-- http://www.cubrc.org/ontologies/KDD/Mid/EventOntology#ActOfWeaponUse -->

    <owl:Class rdf:about="http://www.cubrc.org/ontologies/KDD/Mid/EventOntology#ActOfWeaponUse">
        <rdfs:label rdf:datatype="&xsd;string">Act Of Weapon Use</rdfs:label>
        <rdfs:subClassOf rdf:resource="http://www.cubrc.org/ontologies/KDD/Mid/EventOntology#ActOfInstrumentUse"/>
        <rdfs:comment rdf:datatype="&xsd;string">An Act Of Instrument Use in which some Agent uses some Weapon.</rdfs:comment>
    </owl:Class>
    


    <!-- http://www.cubrc.org/ontologies/KDD/Mid/EventOntology#ActOfZoneReconnaissance -->

    <owl:Class rdf:about="http://www.cubrc.org/ontologies/KDD/Mid/EventOntology#ActOfZoneReconnaissance">
        <rdfs:label>Conduct a Zone Reconnaissance</rdfs:label>
        <rdfs:subClassOf rdf:resource="http://www.cubrc.org/ontologies/KDD/Mid/EventOntology#ActOfReconnaissance"/>
        <rdfs:comment>Definition: An Act of Reconnaissance in which a directed effort is made to obtain detailed information about all routes, obstacles (to include chemical, biological, radiological, and nuclear contamination), terrain, and enemy forces in an area defined by boundaries (derived from The Army Universal Task List FM 7-15 February 2009).</rdfs:comment>
    </owl:Class>
    


    <!-- http://www.cubrc.org/ontologies/KDD/Mid/EventOntology#ActofMurder -->

    <owl:Class rdf:about="http://www.cubrc.org/ontologies/KDD/Mid/EventOntology#ActofMurder">
        <rdfs:label>Act of Murder</rdfs:label>
        <rdfs:subClassOf rdf:resource="http://www.cubrc.org/ontologies/KDD/Mid/EventOntology#ActOfCriminalHomicide"/>
        <rdfs:comment>Definition: An Act of Criminal Homicide in which the person acts with malice aforethought. (derived from http://en.wikipedia.org/wiki/Murder)</rdfs:comment>
    </owl:Class>
    


    <!-- http://www.cubrc.org/ontologies/KDD/Mid/EventOntology#Annulment -->

    <owl:Class rdf:about="http://www.cubrc.org/ontologies/KDD/Mid/EventOntology#Annulment">
        <rdfs:label rdf:datatype="&xsd;string">Annulment</rdfs:label>
        <rdfs:subClassOf rdf:resource="http://www.cubrc.org/ontologies/KDD/Mid/EventOntology#LegalSystemAct"/>
        <rdfs:comment rdf:datatype="&xsd;string">Definition: A Legal System Act for declaring a Marriage null and void. It is usually retroactive, meaning that an annulled marriage is considered to be invalid from the beginning almost as if it had never taken place (though some jurisdictions provide that the marriage is only void from the date of the annulment). (derived from http://en.wikipedia.org/wiki/Annulment)</rdfs:comment>
    </owl:Class>
    


    <!-- http://www.cubrc.org/ontologies/KDD/Mid/EventOntology#Appeal -->

    <owl:Class rdf:about="http://www.cubrc.org/ontologies/KDD/Mid/EventOntology#Appeal">
        <rdfs:label>Appeal</rdfs:label>
        <rdfs:subClassOf rdf:resource="http://www.cubrc.org/ontologies/KDD/Mid/EventOntology#LegalSystemAct"/>
        <rdfs:comment>Definition: A Legal System Act involving a higher court review of a lower court decision. (derived from http://www.id.uscourts.gov/glossary.htm)</rdfs:comment>
    </owl:Class>
    


    <!-- http://www.cubrc.org/ontologies/KDD/Mid/EventOntology#Arrest -->

    <owl:Class rdf:about="http://www.cubrc.org/ontologies/KDD/Mid/EventOntology#Arrest">
        <rdfs:label>Arrest</rdfs:label>
        <rdfs:subClassOf rdf:resource="http://www.cubrc.org/ontologies/KDD/Mid/EventOntology#LegalSystemAct"/>
        <rdfs:comment>Definition: A Legal System Act of taking a person into custody by some legal authority (derived from http://www.id.uscourts.gov/glossary.htm)</rdfs:comment>
    </owl:Class>
    


    <!-- http://www.cubrc.org/ontologies/KDD/Mid/EventOntology#BiographicalLife -->

    <owl:Class rdf:about="http://www.cubrc.org/ontologies/KDD/Mid/EventOntology#BiographicalLife">
        <rdfs:label rdf:datatype="&xsd;string">Biographical Life</rdfs:label>
        <rdfs:subClassOf rdf:resource="http://www.cubrc.org/ontologies/KDD/Mid/EventOntology#Act"/>
        <rdfs:comment rdf:datatype="&xsd;string">An Act composed of the Life Events that occur during the course of existence of an Agent (i.e. person, Organization).</rdfs:comment>
    </owl:Class>
    


    <!-- http://www.cubrc.org/ontologies/KDD/Mid/EventOntology#Birth -->

    <owl:Class rdf:about="http://www.cubrc.org/ontologies/KDD/Mid/EventOntology#Birth">
        <rdfs:label rdf:datatype="&xsd;string">Birth</rdfs:label>
        <rdfs:subClassOf rdf:resource="http://www.ifomis.org/bfo/1.1/span#ProcessBoundary"/>
        <rdfs:comment rdf:datatype="&xsd;string">The originating Process Boundary of Biographical Life. </rdfs:comment>
    </owl:Class>
    


    <!-- http://www.cubrc.org/ontologies/KDD/Mid/EventOntology#Cause -->

    <owl:Class rdf:about="http://www.cubrc.org/ontologies/KDD/Mid/EventOntology#Cause">
        <rdfs:label rdf:datatype="&xsd;string">Cause</rdfs:label>
        <owl:equivalentClass>
            <owl:Restriction>
                <owl:onProperty rdf:resource="&ero;is_cause_of"/>
                <owl:someValuesFrom rdf:resource="http://www.ifomis.org/bfo/1.1/span#ProcessualEntity"/>
            </owl:Restriction>
        </owl:equivalentClass>
        <rdfs:subClassOf rdf:resource="http://www.ifomis.org/bfo/1.1/span#Process"/>
        <rdfs:comment rdf:datatype="&xsd;string">A Process that is cause of some other Process</rdfs:comment>
    </owl:Class>
    


    <!-- http://www.cubrc.org/ontologies/KDD/Mid/EventOntology#Concert -->

    <owl:Class rdf:about="http://www.cubrc.org/ontologies/KDD/Mid/EventOntology#Concert">
        <rdfs:label rdf:datatype="&xsd;string">Concert</rdfs:label>
        <rdfs:subClassOf rdf:resource="http://www.cubrc.org/ontologies/KDD/Mid/EventOntology#ActOfEntertainment"/>
        <rdfs:comment rdf:datatype="&xsd;string">An Act of Entertainment that is a public musical performance in which a number of singers or instrumentalists, or both, participate.</rdfs:comment>
    </owl:Class>
    


    <!-- http://www.cubrc.org/ontologies/KDD/Mid/EventOntology#CriminalAct -->

    <owl:Class rdf:about="http://www.cubrc.org/ontologies/KDD/Mid/EventOntology#CriminalAct">
        <rdfs:label>Criminal Act</rdfs:label>
        <rdfs:subClassOf rdf:resource="http://www.cubrc.org/ontologies/KDD/Mid/EventOntology#IntentionalAct"/>
        <rdfs:comment>Definition: An Intentional Act committed in violation of rules or laws for which some governing authority (via mechanisms such as legal systems) can prescribe a conviction (derived from http://en.wikipedia.org/wiki/Crime).</rdfs:comment>
    </owl:Class>
    


    <!-- http://www.cubrc.org/ontologies/KDD/Mid/EventOntology#CriminalActAgainstJustice -->

    <owl:Class rdf:about="http://www.cubrc.org/ontologies/KDD/Mid/EventOntology#CriminalActAgainstJustice">
        <rdfs:label>Criminal Act Against Justice</rdfs:label>
        <rdfs:subClassOf rdf:resource="http://www.cubrc.org/ontologies/KDD/Mid/EventOntology#CriminalAct"/>
        <rdfs:comment>Definition: A Criminal Act which involves interfering with the operations of the legal system.</rdfs:comment>
    </owl:Class>
    


    <!-- http://www.cubrc.org/ontologies/KDD/Mid/EventOntology#CriminalActAgainstProperty -->

    <owl:Class rdf:about="http://www.cubrc.org/ontologies/KDD/Mid/EventOntology#CriminalActAgainstProperty">
        <rdfs:label>Criminal Act Against Property</rdfs:label>
        <rdfs:subClassOf rdf:resource="http://www.cubrc.org/ontologies/KDD/Mid/EventOntology#CriminalAct"/>
        <rdfs:comment>Definition: A Criminal Act of the taking of money or property without the use of force or threat of force against a victim. (derived from http://en.wikipedia.org/wiki/Property_crime).</rdfs:comment>
    </owl:Class>
    


    <!-- http://www.cubrc.org/ontologies/KDD/Mid/EventOntology#CriminalActAgainstThePerson -->

    <owl:Class rdf:about="http://www.cubrc.org/ontologies/KDD/Mid/EventOntology#CriminalActAgainstThePerson">
        <rdfs:label>Criminal Act Against The Person</rdfs:label>
        <rdfs:subClassOf rdf:resource="http://www.cubrc.org/ontologies/KDD/Mid/EventOntology#CriminalAct"/>
        <rdfs:comment>Definition: A Criminal Act of direct physical harm or force being applied to another person. (derived from http://en.wikipedia.org/wiki/Offence_against_the_person)</rdfs:comment>
    </owl:Class>
    


    <!-- http://www.cubrc.org/ontologies/KDD/Mid/EventOntology#CriminalTrial -->

    <owl:Class rdf:about="http://www.cubrc.org/ontologies/KDD/Mid/EventOntology#CriminalTrial">
        <rdfs:label>Criminal Trial</rdfs:label>
        <rdfs:subClassOf rdf:resource="http://www.cubrc.org/ontologies/KDD/Mid/EventOntology#Trial"/>
        <rdfs:comment>Definition: A Trial involving a judicial examination of a claim that a person has violated criminal law (derived from http://www.id.uscourts.gov/glossary.htm)</rdfs:comment>
    </owl:Class>
    


    <!-- http://www.cubrc.org/ontologies/KDD/Mid/EventOntology#Damage -->

    <owl:Class rdf:about="http://www.cubrc.org/ontologies/KDD/Mid/EventOntology#Damage">
        <rdfs:label rdf:datatype="&xsd;string">Damage</rdfs:label>
        <rdfs:subClassOf rdf:resource="http://www.cubrc.org/ontologies/KDD/Mid/EventOntology#DecreaseOfSpecificallyDependentContinuant"/>
        <rdfs:comment rdf:datatype="&xsd;string">Definition: A Decrease of Specifically Dependent Continuant in which some Independent Continuant suffers an Intentional Act that causes a loss of Function or a Quality of Structural Integrity</rdfs:comment>
    </owl:Class>
    


    <!-- http://www.cubrc.org/ontologies/KDD/Mid/EventOntology#Death -->

    <owl:Class rdf:about="http://www.cubrc.org/ontologies/KDD/Mid/EventOntology#Death">
        <rdfs:label rdf:datatype="&xsd;string">Death</rdfs:label>
        <rdfs:subClassOf rdf:resource="http://www.ifomis.org/bfo/1.1/span#ProcessBoundary"/>
        <rdfs:comment rdf:datatype="&xsd;string">The terminating Process Boundary of some Biographical Life.</rdfs:comment>
    </owl:Class>
    


    <!-- http://www.cubrc.org/ontologies/KDD/Mid/EventOntology#DecreaseOfDependentContinuant -->

    <owl:Class rdf:about="http://www.cubrc.org/ontologies/KDD/Mid/EventOntology#DecreaseOfDependentContinuant">
        <rdfs:label rdf:datatype="&xsd;string">Decrease of Dependent Continuant</rdfs:label>
        <rdfs:subClassOf rdf:resource="http://www.cubrc.org/ontologies/KDD/Mid/EventOntology#DynamicState"/>
        <rdfs:comment rdf:datatype="&xsd;string">Definition: A Dynamic State in which some Independent Continuant has a decrease in the level of some Dependent Continuant that it bears.</rdfs:comment>
    </owl:Class>
    


    <!-- http://www.cubrc.org/ontologies/KDD/Mid/EventOntology#DecreaseOfDisposition -->

    <owl:Class rdf:about="http://www.cubrc.org/ontologies/KDD/Mid/EventOntology#DecreaseOfDisposition">
        <rdfs:label rdf:datatype="&xsd;string">Decrease of Disposition</rdfs:label>
        <rdfs:subClassOf rdf:resource="http://www.cubrc.org/ontologies/KDD/Mid/EventOntology#DecreaseOfRealizableEntity"/>
        <rdfs:comment rdf:datatype="&xsd;string">Definition: A Decrease of Realizable Entity in which some Independent Continuant has a decrease of some Disposition it bears</rdfs:comment>
    </owl:Class>
    


    <!-- http://www.cubrc.org/ontologies/KDD/Mid/EventOntology#DecreaseOfFunction -->

    <owl:Class rdf:about="http://www.cubrc.org/ontologies/KDD/Mid/EventOntology#DecreaseOfFunction">
        <rdfs:label rdf:datatype="&xsd;string">Decrease of Function</rdfs:label>
        <rdfs:subClassOf rdf:resource="http://www.cubrc.org/ontologies/KDD/Mid/EventOntology#DecreaseOfRealizableEntity"/>
        <rdfs:comment rdf:datatype="&xsd;string">Definition: A Decrease of Realizable Entity in which some Independent Continuant has a decrease of some Function that it bears.</rdfs:comment>
    </owl:Class>
    


    <!-- http://www.cubrc.org/ontologies/KDD/Mid/EventOntology#DecreaseOfGenericallyDependentContinuant -->

    <owl:Class rdf:about="http://www.cubrc.org/ontologies/KDD/Mid/EventOntology#DecreaseOfGenericallyDependentContinuant">
        <rdfs:label rdf:datatype="&xsd;string">Decrease of Generically Dependent Continuant</rdfs:label>
        <rdfs:subClassOf rdf:resource="http://www.cubrc.org/ontologies/KDD/Mid/EventOntology#DecreaseOfDependentContinuant"/>
        <rdfs:comment rdf:datatype="&xsd;string">Comment: For the most part Generically Dependent Continuants do not inhere in their bearers over some continuous scale. The primary exception is religion and this class allows annotation of those cases where an Agent is described as becoming less religious. Other cases would include the decrease of an organization&apos;s bearing of some objective.</rdfs:comment>
        <rdfs:comment rdf:datatype="&xsd;string">Definition: A Decrease of Dependent Continuant in which some Independent Continuant has a decrease in the level of a Generically Dependent Continuant that it bears.</rdfs:comment>
    </owl:Class>
    


    <!-- http://www.cubrc.org/ontologies/KDD/Mid/EventOntology#DecreaseOfQuality -->

    <owl:Class rdf:about="http://www.cubrc.org/ontologies/KDD/Mid/EventOntology#DecreaseOfQuality">
        <rdfs:label rdf:datatype="&xsd;string">Decrease of Quality</rdfs:label>
        <rdfs:subClassOf rdf:resource="http://www.cubrc.org/ontologies/KDD/Mid/EventOntology#DecreaseOfSpecificallyDependentContinuant"/>
        <rdfs:comment rdf:datatype="&xsd;string">Definition: A Decrease of Specifically Dependent Continuant in which some Independent Continuant has a decrease of some Quality that it bears.</rdfs:comment>
        <rdfs:comment rdf:datatype="&xsd;string">Examples: Weight Loss, Decreasing Temperature, decreasing color intensity, loss of structural integrity</rdfs:comment>
    </owl:Class>
    


    <!-- http://www.cubrc.org/ontologies/KDD/Mid/EventOntology#DecreaseOfRealizableEntity -->

    <owl:Class rdf:about="http://www.cubrc.org/ontologies/KDD/Mid/EventOntology#DecreaseOfRealizableEntity">
        <rdfs:label rdf:datatype="&xsd;string">Decrease of Realizable Entity</rdfs:label>
        <rdfs:subClassOf rdf:resource="http://www.cubrc.org/ontologies/KDD/Mid/EventOntology#DecreaseOfSpecificallyDependentContinuant"/>
        <rdfs:comment rdf:datatype="&xsd;string">Definition: A Decrease of Specifically Dependent Continuant in which some Independent Continuant has a decrease of some Realizable Entity that it bears.</rdfs:comment>
    </owl:Class>
    


    <!-- http://www.cubrc.org/ontologies/KDD/Mid/EventOntology#DecreaseOfRole -->

    <owl:Class rdf:about="http://www.cubrc.org/ontologies/KDD/Mid/EventOntology#DecreaseOfRole">
        <rdfs:label rdf:datatype="&xsd;string">Decrease of Role</rdfs:label>
        <rdfs:subClassOf rdf:resource="http://www.cubrc.org/ontologies/KDD/Mid/EventOntology#DecreaseOfRealizableEntity"/>
        <rdfs:comment rdf:datatype="&xsd;string">Definition: A Decrease of Realizable Entity in which some Independent Continuant has a decrease of some Role that it bears.</rdfs:comment>
    </owl:Class>
    


    <!-- http://www.cubrc.org/ontologies/KDD/Mid/EventOntology#DecreaseOfSpecificallyDependentContinuant -->

    <owl:Class rdf:about="http://www.cubrc.org/ontologies/KDD/Mid/EventOntology#DecreaseOfSpecificallyDependentContinuant">
        <rdfs:label rdf:datatype="&xsd;string">Decrease of Specifically Dependent Continuant</rdfs:label>
        <rdfs:subClassOf rdf:resource="http://www.cubrc.org/ontologies/KDD/Mid/EventOntology#DecreaseOfDependentContinuant"/>
        <rdfs:comment rdf:datatype="&xsd;string">Definition: A Decrease of Dependent Continuant in which some Independent Continuant has a decrease in some Specifically Dependent Continuant that it bears.</rdfs:comment>
    </owl:Class>
    


    <!-- http://www.cubrc.org/ontologies/KDD/Mid/EventOntology#Divorce -->

    <owl:Class rdf:about="http://www.cubrc.org/ontologies/KDD/Mid/EventOntology#Divorce">
        <rdfs:label>Divorce</rdfs:label>
        <rdfs:subClassOf rdf:resource="http://www.cubrc.org/ontologies/KDD/Mid/EventOntology#LegalSystemAct"/>
        <rdfs:comment>Definition: A Legal System Act that dissolves a contract of Marriage between people.</rdfs:comment>
    </owl:Class>
    


    <!-- http://www.cubrc.org/ontologies/KDD/Mid/EventOntology#DynamicState -->

    <owl:Class rdf:about="http://www.cubrc.org/ontologies/KDD/Mid/EventOntology#DynamicState">
        <rdfs:label rdf:datatype="&xsd;string">Dynamic State</rdfs:label>
        <rdfs:subClassOf rdf:resource="http://www.cubrc.org/ontologies/KDD/Mid/EventOntology#State"/>
        <rdfs:comment rdf:datatype="&xsd;string">A State in which some Quality, Disposition, Function, or Role of an Entity is altered during a Temporal Interval.</rdfs:comment>
    </owl:Class>
    


    <!-- http://www.cubrc.org/ontologies/KDD/Mid/EventOntology#Economy -->

    <owl:Class rdf:about="http://www.cubrc.org/ontologies/KDD/Mid/EventOntology#Economy">
        <rdfs:label rdf:datatype="&xsd;string">Economy</rdfs:label>
        <rdfs:subClassOf rdf:resource="http://www.ifomis.org/bfo/1.1/span#ProcessAggregate"/>
        <rdfs:comment rdf:datatype="&xsd;string">Definition: A Process Aggregate comprising the production, exchange, distribution and consumption of goods that occurs at some Geopolitical Entity</rdfs:comment>
    </owl:Class>
    


    <!-- http://www.cubrc.org/ontologies/KDD/Mid/EventOntology#Effect -->

    <owl:Class rdf:about="http://www.cubrc.org/ontologies/KDD/Mid/EventOntology#Effect">
        <rdfs:label rdf:datatype="&xsd;string">Effect</rdfs:label>
        <owl:equivalentClass>
            <owl:Restriction>
                <owl:onProperty rdf:resource="&ero;caused_by"/>
                <owl:someValuesFrom rdf:resource="http://www.ifomis.org/bfo/1.1/span#ProcessualEntity"/>
            </owl:Restriction>
        </owl:equivalentClass>
        <rdfs:subClassOf rdf:resource="http://www.ifomis.org/bfo/1.1/span#Process"/>
    </owl:Class>
    


    <!-- http://www.cubrc.org/ontologies/KDD/Mid/EventOntology#Election -->

    <owl:Class rdf:about="http://www.cubrc.org/ontologies/KDD/Mid/EventOntology#Election">
        <rdfs:label rdf:datatype="&xsd;string">Election</rdfs:label>
        <rdfs:subClassOf rdf:resource="http://www.cubrc.org/ontologies/KDD/Mid/EventOntology#SocialAct"/>
        <rdfs:comment rdf:datatype="&xsd;string">Definition: A Social Act by which a population chooses an individual to hold public office (derived from http://en.wikipedia.org/wiki/Election)</rdfs:comment>
    </owl:Class>
    


    <!-- http://www.cubrc.org/ontologies/KDD/Mid/EventOntology#EmailMessaging -->

    <owl:Class rdf:about="http://www.cubrc.org/ontologies/KDD/Mid/EventOntology#EmailMessaging">
        <rdfs:label rdf:datatype="&xsd;string">Email Messaging</rdfs:label>
        <rdfs:subClassOf rdf:resource="http://www.cubrc.org/ontologies/KDD/Mid/EventOntology#ActOfCommunicationByMedia"/>
        <rdfs:comment rdf:datatype="&xsd;string">Definition: An Act of Communication in which text-based communication occurs between two or more people using personal computers or other devices using some Email Client Software conveyed over the Internet (derived from http://en.wikipedia.org/wiki/Email)</rdfs:comment>
    </owl:Class>
    


    <!-- http://www.cubrc.org/ontologies/KDD/Mid/EventOntology#EssentialServiceProvision -->

    <owl:Class rdf:about="http://www.cubrc.org/ontologies/KDD/Mid/EventOntology#EssentialServiceProvision">
        <rdfs:label rdf:datatype="&xsd;string">Essential Service Provision</rdfs:label>
        <rdfs:subClassOf rdf:resource="http://www.ifomis.org/bfo/1.1/span#ProcessAggregate"/>
        <rdfs:comment rdf:datatype="&xsd;string">Definition: A Process Aggregate comprising the delivery of one or more essential services (defined here as being one of: medical care, food and water, shelter, and sanitation).</rdfs:comment>
    </owl:Class>
    


    <!-- http://www.cubrc.org/ontologies/KDD/Mid/EventOntology#ExplosiveDeviceBlownInPlace -->

    <owl:Class rdf:about="http://www.cubrc.org/ontologies/KDD/Mid/EventOntology#ExplosiveDeviceBlownInPlace">
        <rdfs:label>Explosive Device Blown in Place</rdfs:label>
        <rdfs:subClassOf rdf:resource="http://www.cubrc.org/ontologies/KDD/Mid/EventOntology#ActOfExplosiveOrdnanceDisposalSupport"/>
        <rdfs:comment>Definition: An Act of Explosive Ordnance Disposal Support in which an explosive ordnance disposal (EOD) unit performs a controlled detonation of some Explosive Device so as to minimize its destructive effects (derived from the Weapons Technical Intelligence (WTI) Improvised Explosive Device (IED) Lexicon 3rd Edition May 2010).</rdfs:comment>
    </owl:Class>
    


    <!-- http://www.cubrc.org/ontologies/KDD/Mid/EventOntology#ExplosiveDeviceRenderedSafe -->

    <owl:Class rdf:about="http://www.cubrc.org/ontologies/KDD/Mid/EventOntology#ExplosiveDeviceRenderedSafe">
        <rdfs:label>Explosive Device Rendered Safe</rdfs:label>
        <rdfs:subClassOf rdf:resource="http://www.cubrc.org/ontologies/KDD/Mid/EventOntology#ActOfExplosiveOrdnanceDisposalSupport"/>
        <rdfs:comment>Definition: An Act Of Explosive Ordnance Disposal Support in which an explosive ordnance disposal (EOD) unit disables the destructive function of some Explosive Device (derived from the Weapons Technical Intelligence (WTI) Improvised Explosive Device (IED) Lexicon 3rd Edition May 2010).</rdfs:comment>
    </owl:Class>
    


    <!-- http://www.cubrc.org/ontologies/KDD/Mid/EventOntology#FacsimileTransmission -->

    <owl:Class rdf:about="http://www.cubrc.org/ontologies/KDD/Mid/EventOntology#FacsimileTransmission">
        <rdfs:label rdf:datatype="&xsd;string">Facsimile Transmission</rdfs:label>
        <rdfs:subClassOf rdf:resource="http://www.cubrc.org/ontologies/KDD/Mid/EventOntology#ActOfCommunicationByMedia"/>
        <rdfs:comment rdf:datatype="&xsd;string">Definition: An Act of Communication in which a document is transmitted over a Telephone Network. (derived from http://en.wikipedia.org/wiki/Facsimile_machine)</rdfs:comment>
    </owl:Class>
    


    <!-- http://www.cubrc.org/ontologies/KDD/Mid/EventOntology#FixedLineNetworkTelephoneCall -->

    <owl:Class rdf:about="http://www.cubrc.org/ontologies/KDD/Mid/EventOntology#FixedLineNetworkTelephoneCall">
        <rdfs:label rdf:datatype="&xsd;string">Fixed Line Network Telephone Call</rdfs:label>
        <rdfs:subClassOf rdf:resource="http://www.cubrc.org/ontologies/KDD/Mid/EventOntology#TelephoneCall"/>
        <rdfs:comment rdf:datatype="&xsd;string">Definition: A Telephone Call transmitted over a telephone network where the telephones are wired into a single telephone exchange. (derived from http://en.wikipedia.org/wiki/Telephone_network)</rdfs:comment>
    </owl:Class>
    


    <!-- http://www.cubrc.org/ontologies/KDD/Mid/EventOntology#Funeral -->

    <owl:Class rdf:about="http://www.cubrc.org/ontologies/KDD/Mid/EventOntology#Funeral">
        <rdfs:label>Funeral</rdfs:label>
        <rdfs:subClassOf rdf:resource="http://www.cubrc.org/ontologies/KDD/Mid/EventOntology#ActOfCeremony"/>
        <rdfs:comment>Definition: An Act Of Ceremony in which the Life of a Person who has died is celebrated, sanctified, or remembered (derived from http://en.wikipedia.org/wiki/Funeral) </rdfs:comment>
    </owl:Class>
    


    <!-- http://www.cubrc.org/ontologies/KDD/Mid/EventOntology#GainOfDependentContinuant -->

    <owl:Class rdf:about="http://www.cubrc.org/ontologies/KDD/Mid/EventOntology#GainOfDependentContinuant">
        <rdfs:label rdf:datatype="&xsd;string">Gain of Dependent Continuant</rdfs:label>
        <rdfs:subClassOf rdf:resource="http://www.cubrc.org/ontologies/KDD/Mid/EventOntology#State"/>
        <rdfs:subClassOf>
            <owl:Restriction>
                <owl:onProperty rdf:resource="http://www.obofoundry.org/ro/ro.owl#has_participant"/>
                <owl:someValuesFrom>
                    <owl:Class>
                        <owl:intersectionOf rdf:parseType="Collection">
                            <rdf:Description rdf:about="http://www.ifomis.org/bfo/1.1/snap#IndependentContinuant"/>
                            <owl:Restriction>
                                <owl:onProperty rdf:resource="&ero;bearer_of"/>
                                <owl:someValuesFrom rdf:resource="http://www.ifomis.org/bfo/1.1/snap#DependentContinuant"/>
                            </owl:Restriction>
                        </owl:intersectionOf>
                    </owl:Class>
                </owl:someValuesFrom>
            </owl:Restriction>
        </rdfs:subClassOf>
        <rdfs:comment rdf:datatype="&xsd;string">Definition: A State in which an Independent Continuant becomes the bearer of some Dependent Continuant.</rdfs:comment>
    </owl:Class>
    


    <!-- http://www.cubrc.org/ontologies/KDD/Mid/EventOntology#GainOfDisposition -->

    <owl:Class rdf:about="http://www.cubrc.org/ontologies/KDD/Mid/EventOntology#GainOfDisposition">
        <rdfs:label rdf:datatype="&xsd;string">Gain of Disposition</rdfs:label>
        <rdfs:subClassOf rdf:resource="http://www.cubrc.org/ontologies/KDD/Mid/EventOntology#GainOfRealizableEntity"/>
        <rdfs:subClassOf>
            <owl:Restriction>
                <owl:onProperty rdf:resource="http://www.obofoundry.org/ro/ro.owl#has_participant"/>
                <owl:someValuesFrom>
                    <owl:Class>
                        <owl:intersectionOf rdf:parseType="Collection">
                            <rdf:Description rdf:about="http://www.ifomis.org/bfo/1.1/snap#IndependentContinuant"/>
                            <owl:Restriction>
                                <owl:onProperty rdf:resource="&ero;has_disposition"/>
                                <owl:someValuesFrom rdf:resource="http://www.ifomis.org/bfo/1.1/snap#Disposition"/>
                            </owl:Restriction>
                        </owl:intersectionOf>
                    </owl:Class>
                </owl:someValuesFrom>
            </owl:Restriction>
        </rdfs:subClassOf>
        <rdfs:comment rdf:datatype="&xsd;string">Comment: This class should be used to demarcate the start of the temporal interval (through the occurs_on property) that the Entity bears the disposition.</rdfs:comment>
        <rdfs:comment rdf:datatype="&xsd;string">Definition: A Gain of Realizable Entity in which some Independent Continuant becomes the bearer of (has_disposition) some Disposition, it should be used to demarcate the start of the temporal interval (through the occurs_on property) that the Entity bears the disposition.</rdfs:comment>
    </owl:Class>
    


    <!-- http://www.cubrc.org/ontologies/KDD/Mid/EventOntology#GainOfFunction -->

    <owl:Class rdf:about="http://www.cubrc.org/ontologies/KDD/Mid/EventOntology#GainOfFunction">
        <rdfs:label rdf:datatype="&xsd;string">Gain of Function</rdfs:label>
        <rdfs:subClassOf rdf:resource="http://www.cubrc.org/ontologies/KDD/Mid/EventOntology#GainOfRealizableEntity"/>
        <rdfs:subClassOf>
            <owl:Restriction>
                <owl:onProperty rdf:resource="http://www.obofoundry.org/ro/ro.owl#has_participant"/>
                <owl:someValuesFrom>
                    <owl:Class>
                        <owl:intersectionOf rdf:parseType="Collection">
                            <rdf:Description rdf:about="http://www.ifomis.org/bfo/1.1/snap#IndependentContinuant"/>
                            <owl:Restriction>
                                <owl:onProperty rdf:resource="&ero;has_function"/>
                                <owl:someValuesFrom rdf:resource="http://www.ifomis.org/bfo/1.1/snap#Function"/>
                            </owl:Restriction>
                        </owl:intersectionOf>
                    </owl:Class>
                </owl:someValuesFrom>
            </owl:Restriction>
        </rdfs:subClassOf>
        <rdfs:comment rdf:datatype="&xsd;string">Comment: This class should be used to demarcate the start of the temporal interval (through the occurs_on property) that the Entity bears the function.</rdfs:comment>
        <rdfs:comment rdf:datatype="&xsd;string">Definition: A Gain of Realizable Entity in which some Independent Continuant becomes the bearer of (has_function) some Function, it should be used to demarcate the start of the temporal interval (through the occurs_on property) that the Entity bears the function.</rdfs:comment>
    </owl:Class>
    


    <!-- http://www.cubrc.org/ontologies/KDD/Mid/EventOntology#GainOfGenericallyDependentContinuant -->

    <owl:Class rdf:about="http://www.cubrc.org/ontologies/KDD/Mid/EventOntology#GainOfGenericallyDependentContinuant">
        <rdfs:label rdf:datatype="&xsd;string">Gain of Generically Dependent Continuant</rdfs:label>
        <rdfs:subClassOf rdf:resource="http://www.cubrc.org/ontologies/KDD/Mid/EventOntology#GainOfDependentContinuant"/>
        <rdfs:subClassOf>
            <owl:Restriction>
                <owl:onProperty rdf:resource="http://www.obofoundry.org/ro/ro.owl#has_participant"/>
                <owl:someValuesFrom>
                    <owl:Class>
                        <owl:intersectionOf rdf:parseType="Collection">
                            <rdf:Description rdf:about="http://www.ifomis.org/bfo/1.1/snap#IndependentContinuant"/>
                            <owl:Restriction>
                                <owl:onProperty rdf:resource="&ero;bearer_of"/>
                                <owl:someValuesFrom rdf:resource="http://www.ifomis.org/bfo/1.1/snap#GenericallyDependentContinuant"/>
                            </owl:Restriction>
                        </owl:intersectionOf>
                    </owl:Class>
                </owl:someValuesFrom>
            </owl:Restriction>
        </rdfs:subClassOf>
        <rdfs:comment rdf:datatype="&xsd;string">Definition: A Gain of Dependent Continuant wherein some Independent Continuant becomes the bearer of some Generically Dependent Continuant.</rdfs:comment>
        <rdfs:comment rdf:datatype="&xsd;string">Examples: A Person forms a Plan, A Person is initiated into a Religion, A photgraphic image is produced.</rdfs:comment>
    </owl:Class>
    


    <!-- http://www.cubrc.org/ontologies/KDD/Mid/EventOntology#GainOfQuality -->

    <owl:Class rdf:about="http://www.cubrc.org/ontologies/KDD/Mid/EventOntology#GainOfQuality">
        <rdfs:label rdf:datatype="&xsd;string">Gain of Quality</rdfs:label>
        <rdfs:subClassOf rdf:resource="http://www.cubrc.org/ontologies/KDD/Mid/EventOntology#GainOfSpecificallyDependentContinuant"/>
        <rdfs:subClassOf>
            <owl:Restriction>
                <owl:onProperty rdf:resource="http://www.obofoundry.org/ro/ro.owl#has_participant"/>
                <owl:someValuesFrom>
                    <owl:Class>
                        <owl:intersectionOf rdf:parseType="Collection">
                            <rdf:Description rdf:about="http://www.ifomis.org/bfo/1.1/snap#IndependentContinuant"/>
                            <owl:Restriction>
                                <owl:onProperty rdf:resource="&ero;has_quality"/>
                                <owl:someValuesFrom rdf:resource="http://www.ifomis.org/bfo/1.1/snap#Quality"/>
                            </owl:Restriction>
                        </owl:intersectionOf>
                    </owl:Class>
                </owl:someValuesFrom>
            </owl:Restriction>
        </rdfs:subClassOf>
        <rdfs:comment rdf:datatype="&xsd;string">Comment: Examples include A person becoming pregnant.</rdfs:comment>
        <rdfs:comment rdf:datatype="&xsd;string">Definition: A Gain of Specifically Dependent Continuant in which an Independent Continuant becomes bearer of (has_quality_of) some Quality.</rdfs:comment>
    </owl:Class>
    


    <!-- http://www.cubrc.org/ontologies/KDD/Mid/EventOntology#GainOfRealizableEntity -->

    <owl:Class rdf:about="http://www.cubrc.org/ontologies/KDD/Mid/EventOntology#GainOfRealizableEntity">
        <rdfs:label rdf:datatype="&xsd;string">Gain of Realizable Entity</rdfs:label>
        <rdfs:subClassOf rdf:resource="http://www.cubrc.org/ontologies/KDD/Mid/EventOntology#GainOfSpecificallyDependentContinuant"/>
        <rdfs:subClassOf>
            <owl:Restriction>
                <owl:onProperty rdf:resource="http://www.obofoundry.org/ro/ro.owl#has_participant"/>
                <owl:someValuesFrom>
                    <owl:Class>
                        <owl:intersectionOf rdf:parseType="Collection">
                            <rdf:Description rdf:about="http://www.ifomis.org/bfo/1.1/snap#IndependentContinuant"/>
                            <owl:Restriction>
                                <owl:onProperty rdf:resource="&ero;bearer_of"/>
                                <owl:someValuesFrom rdf:resource="http://www.ifomis.org/bfo/1.1/snap#RealizableEntity"/>
                            </owl:Restriction>
                        </owl:intersectionOf>
                    </owl:Class>
                </owl:someValuesFrom>
            </owl:Restriction>
        </rdfs:subClassOf>
        <rdfs:comment rdf:datatype="&xsd;string">Comment: Examples: An informant becomes unreliable (disposition), A person begins to speak French (function), a person becomes a welder (role).</rdfs:comment>
        <rdfs:comment rdf:datatype="&xsd;string">Definition: A Gain of Specifically Dependent Continuant in which some Independent Continuant becomes the bearer_of some Realizable Entity</rdfs:comment>
    </owl:Class>
    


    <!-- http://www.cubrc.org/ontologies/KDD/Mid/EventOntology#GainOfRole -->

    <owl:Class rdf:about="http://www.cubrc.org/ontologies/KDD/Mid/EventOntology#GainOfRole">
        <rdfs:label rdf:datatype="&xsd;string">Gain of Role</rdfs:label>
        <rdfs:subClassOf rdf:resource="http://www.cubrc.org/ontologies/KDD/Mid/EventOntology#GainOfRealizableEntity"/>
        <rdfs:subClassOf>
            <owl:Restriction>
                <owl:onProperty rdf:resource="http://www.obofoundry.org/ro/ro.owl#has_participant"/>
                <owl:someValuesFrom>
                    <owl:Class>
                        <owl:intersectionOf rdf:parseType="Collection">
                            <rdf:Description rdf:about="http://www.ifomis.org/bfo/1.1/snap#IndependentContinuant"/>
                            <owl:Restriction>
                                <owl:onProperty rdf:resource="&ero;has_role"/>
                                <owl:someValuesFrom rdf:resource="http://www.ifomis.org/bfo/1.1/snap#Role"/>
                            </owl:Restriction>
                        </owl:intersectionOf>
                    </owl:Class>
                </owl:someValuesFrom>
            </owl:Restriction>
        </rdfs:subClassOf>
        <rdfs:comment rdf:datatype="&xsd;string">Comment: This class should be used to demarcate the start of the temporal interval (through the occurs_on property) that the Entity bears the Role.</rdfs:comment>
        <rdfs:comment rdf:datatype="&xsd;string">Definition: A Gain of Realizable Entity in which some Independent Continuant becomes bearer of (role_of) some Role.</rdfs:comment>
    </owl:Class>
    


    <!-- http://www.cubrc.org/ontologies/KDD/Mid/EventOntology#GainOfSpecificallyDependentContinuant -->

    <owl:Class rdf:about="http://www.cubrc.org/ontologies/KDD/Mid/EventOntology#GainOfSpecificallyDependentContinuant">
        <rdfs:label rdf:datatype="&xsd;string">Gain of Specifically Dependent Continuant</rdfs:label>
        <rdfs:subClassOf rdf:resource="http://www.cubrc.org/ontologies/KDD/Mid/EventOntology#GainOfDependentContinuant"/>
        <rdfs:subClassOf>
            <owl:Restriction>
                <owl:onProperty rdf:resource="http://www.obofoundry.org/ro/ro.owl#has_participant"/>
                <owl:someValuesFrom>
                    <owl:Class>
                        <owl:intersectionOf rdf:parseType="Collection">
                            <rdf:Description rdf:about="http://www.ifomis.org/bfo/1.1/snap#IndependentContinuant"/>
                            <owl:Restriction>
                                <owl:onProperty rdf:resource="&ero;bearer_of"/>
                                <owl:someValuesFrom rdf:resource="http://www.ifomis.org/bfo/1.1/snap#SpecificallyDependentContinuant"/>
                            </owl:Restriction>
                        </owl:intersectionOf>
                    </owl:Class>
                </owl:someValuesFrom>
            </owl:Restriction>
        </rdfs:subClassOf>
        <rdfs:comment rdf:datatype="&xsd;string">Comment: Examples: A Person becomes pregnant (gain of quality), A person becomes forgetful (gain of disposition), A vehicle becomes amphibious (gain of function), A Person becomes a Database Administrator (gain of role).</rdfs:comment>
        <rdfs:comment rdf:datatype="&xsd;string">Definition: A Gain of Dependent Continuant in which some Independent Continuant becomes the bearer of some Specifically Dependent Continuant.</rdfs:comment>
    </owl:Class>
    


    <!-- http://www.cubrc.org/ontologies/KDD/Mid/EventOntology#Hearing -->

    <owl:Class rdf:about="http://www.cubrc.org/ontologies/KDD/Mid/EventOntology#Hearing">
        <rdfs:label>Hearing</rdfs:label>
        <rdfs:subClassOf rdf:resource="http://www.cubrc.org/ontologies/KDD/Mid/EventOntology#LegalSystemAct"/>
        <rdfs:comment>Definition: A Legal System Act  that is a formal proceeding (generally less formal than a Trial) with definite issues of law or of fact to be heard. (derived from http://www.id.uscourts.gov/glossary.htm)</rdfs:comment>
    </owl:Class>
    


    <!-- http://www.cubrc.org/ontologies/KDD/Mid/EventOntology#InchoateCriminalAct -->

    <owl:Class rdf:about="http://www.cubrc.org/ontologies/KDD/Mid/EventOntology#InchoateCriminalAct">
        <rdfs:label>Inchoate Criminal Act</rdfs:label>
        <rdfs:subClassOf rdf:resource="http://www.cubrc.org/ontologies/KDD/Mid/EventOntology#CriminalAct"/>
        <rdfs:comment>Definition: A Criminal Act  of preparing for or seeking to commit another crime (derived from http://en.wikipedia.org/wiki/Inchoate_offense)</rdfs:comment>
    </owl:Class>
    


    <!-- http://www.cubrc.org/ontologies/KDD/Mid/EventOntology#IncreaseOfDependentContinuant -->

    <owl:Class rdf:about="http://www.cubrc.org/ontologies/KDD/Mid/EventOntology#IncreaseOfDependentContinuant">
        <rdfs:label rdf:datatype="&xsd;string">Increase of Dependent Continuant</rdfs:label>
        <rdfs:subClassOf rdf:resource="http://www.cubrc.org/ontologies/KDD/Mid/EventOntology#DynamicState"/>
        <rdfs:comment rdf:datatype="&xsd;string">Definition:</rdfs:comment>
    </owl:Class>
    


    <!-- http://www.cubrc.org/ontologies/KDD/Mid/EventOntology#IncreaseOfDisposition -->

    <owl:Class rdf:about="http://www.cubrc.org/ontologies/KDD/Mid/EventOntology#IncreaseOfDisposition">
        <rdfs:label rdf:datatype="&xsd;string">Increase of Disposition</rdfs:label>
        <rdfs:subClassOf rdf:resource="http://www.cubrc.org/ontologies/KDD/Mid/EventOntology#IncreaseOfRealizableEntity"/>
        <rdfs:comment rdf:datatype="&xsd;string">Definition: An Increase of Realizable Entity in which some Independent Continuant has an increase of some Disposition that it bears.</rdfs:comment>
    </owl:Class>
    


    <!-- http://www.cubrc.org/ontologies/KDD/Mid/EventOntology#IncreaseOfFunction -->

    <owl:Class rdf:about="http://www.cubrc.org/ontologies/KDD/Mid/EventOntology#IncreaseOfFunction">
        <rdfs:label rdf:datatype="&xsd;string">Increase of Function</rdfs:label>
        <rdfs:subClassOf rdf:resource="http://www.cubrc.org/ontologies/KDD/Mid/EventOntology#IncreaseOfRealizableEntity"/>
        <rdfs:comment rdf:datatype="&xsd;string">Definition: An Increase of Realizable Entity in which some Independent Continuant has an increase of some Function that it bears.</rdfs:comment>
    </owl:Class>
    


    <!-- http://www.cubrc.org/ontologies/KDD/Mid/EventOntology#IncreaseOfGenericallyDependentContinuant -->

    <owl:Class rdf:about="http://www.cubrc.org/ontologies/KDD/Mid/EventOntology#IncreaseOfGenericallyDependentContinuant">
        <rdfs:label rdf:datatype="&xsd;string">Increase of Generically Dependent Continuant</rdfs:label>
        <rdfs:subClassOf rdf:resource="http://www.cubrc.org/ontologies/KDD/Mid/EventOntology#IncreaseOfDependentContinuant"/>
        <rdfs:comment rdf:datatype="&xsd;string">Definition: An Increase of Dependent Continuant in which some Independent Continuant has an increase of some Generically Dependent Continuant that it bears.</rdfs:comment>
    </owl:Class>
    


    <!-- http://www.cubrc.org/ontologies/KDD/Mid/EventOntology#IncreaseOfQuality -->

    <owl:Class rdf:about="http://www.cubrc.org/ontologies/KDD/Mid/EventOntology#IncreaseOfQuality">
        <rdfs:label rdf:datatype="&xsd;string">Increase of Quality</rdfs:label>
        <rdfs:subClassOf rdf:resource="http://www.cubrc.org/ontologies/KDD/Mid/EventOntology#IncreaseOfSpecificallyDependentContinuant"/>
        <rdfs:comment rdf:datatype="&xsd;string">Definition: An Increase of Specifically Dependent Continuant in which some Indpendent Continuant has an increase of some Quality that it bears.</rdfs:comment>
    </owl:Class>
    


    <!-- http://www.cubrc.org/ontologies/KDD/Mid/EventOntology#IncreaseOfRealizableEntity -->

    <owl:Class rdf:about="http://www.cubrc.org/ontologies/KDD/Mid/EventOntology#IncreaseOfRealizableEntity">
        <rdfs:label rdf:datatype="&xsd;string">Increase of Realizable Entity</rdfs:label>
        <rdfs:subClassOf rdf:resource="http://www.cubrc.org/ontologies/KDD/Mid/EventOntology#IncreaseOfSpecificallyDependentContinuant"/>
        <rdfs:comment rdf:datatype="&xsd;string">Definition: An Increase of Specifically Dependent Continuant in which some Independent Continuant has an increase of some Realizable Entity that it bears.</rdfs:comment>
    </owl:Class>
    


    <!-- http://www.cubrc.org/ontologies/KDD/Mid/EventOntology#IncreaseOfRole -->

    <owl:Class rdf:about="http://www.cubrc.org/ontologies/KDD/Mid/EventOntology#IncreaseOfRole">
        <rdfs:label rdf:datatype="&xsd;string">Increase of Role</rdfs:label>
        <rdfs:subClassOf rdf:resource="http://www.cubrc.org/ontologies/KDD/Mid/EventOntology#IncreaseOfRealizableEntity"/>
        <rdfs:comment rdf:datatype="&xsd;string">Definition: An Increase of Realizable Entity in which some Independent Continuant has an increase of some Role that it bears.</rdfs:comment>
    </owl:Class>
    


    <!-- http://www.cubrc.org/ontologies/KDD/Mid/EventOntology#IncreaseOfSpecificallyDependentContinuant -->

    <owl:Class rdf:about="http://www.cubrc.org/ontologies/KDD/Mid/EventOntology#IncreaseOfSpecificallyDependentContinuant">
        <rdfs:label rdf:datatype="&xsd;string">Increase of Specifically Dependent Continuant</rdfs:label>
        <rdfs:subClassOf rdf:resource="http://www.cubrc.org/ontologies/KDD/Mid/EventOntology#IncreaseOfDependentContinuant"/>
        <rdfs:comment rdf:datatype="&xsd;string">Definition: An Increase of Dependent Continuant in which some Independent Continuant has an increase of some Specifically Dependent Continuant that it bears.</rdfs:comment>
    </owl:Class>
    


    <!-- http://www.cubrc.org/ontologies/KDD/Mid/EventOntology#InstantMessaging -->

    <owl:Class rdf:about="http://www.cubrc.org/ontologies/KDD/Mid/EventOntology#InstantMessaging">
        <rdfs:label rdf:datatype="&xsd;string">Instant Messaging</rdfs:label>
        <rdfs:subClassOf rdf:resource="http://www.cubrc.org/ontologies/KDD/Mid/EventOntology#ActOfCommunicationByMedia"/>
        <rdfs:comment rdf:datatype="&xsd;string">Definition: An Act of Communication in which real-time direct text-based communication occurs between two or more people using personal computers or other devices, along with shared Instant Messaging Client Software conveyed over a network, such as the Internet (derived from http://en.wikipedia.org/wiki/Instant_messaging#Clients)</rdfs:comment>
    </owl:Class>
    


    <!-- http://www.cubrc.org/ontologies/KDD/Mid/EventOntology#IntellectualPropertyFraud -->

    <owl:Class rdf:about="http://www.cubrc.org/ontologies/KDD/Mid/EventOntology#IntellectualPropertyFraud">
        <rdfs:label>Act of Intellecutual Property Fraud</rdfs:label>
        <rdfs:subClassOf rdf:resource="http://www.cubrc.org/ontologies/KDD/Mid/EventOntology#ActOfFraud"/>
        <rdfs:comment rdf:datatype="&xsd;string">Definition: Intellectual property crime refers to the violation of criminal laws that protect copyrights, patents, trademarks, other forms of intellectual property, and trade secrets, both in the United States and abroad. (Source: https://www.bja.gov/ProgramDetails.aspx?Program_ID=64)</rdfs:comment>
    </owl:Class>
    


    <!-- http://www.cubrc.org/ontologies/KDD/Mid/EventOntology#IntentionalAct -->

    <owl:Class rdf:about="http://www.cubrc.org/ontologies/KDD/Mid/EventOntology#IntentionalAct">
        <rdfs:label rdf:datatype="&xsd;string">Intentional Act</rdfs:label>
        <rdfs:subClassOf rdf:resource="http://www.cubrc.org/ontologies/KDD/Mid/EventOntology#Act"/>
        <rdfs:comment rdf:datatype="&xsd;string">An Act in which at least one Agent plays a causative role and which is prescribed by some Objective (synonym: Directive Information Content Entity) held by at least one of the Agents.</rdfs:comment>
    </owl:Class>
    


    <!-- http://www.cubrc.org/ontologies/KDD/Mid/EventOntology#Killing -->

    <owl:Class rdf:about="http://www.cubrc.org/ontologies/KDD/Mid/EventOntology#Killing">
        <rdfs:label rdf:datatype="&xsd;string">Killing</rdfs:label>
        <rdfs:subClassOf rdf:resource="http://www.cubrc.org/ontologies/KDD/Mid/EventOntology#Damage"/>
        <rdfs:comment rdf:datatype="&xsd;string">A type of Damage in which some Agent suffers death from some external force.</rdfs:comment>
    </owl:Class>
    


    <!-- http://www.cubrc.org/ontologies/KDD/Mid/EventOntology#Lawsuit -->

    <owl:Class rdf:about="http://www.cubrc.org/ontologies/KDD/Mid/EventOntology#Lawsuit">
        <rdfs:label>Lawsuit</rdfs:label>
        <rdfs:subClassOf rdf:resource="http://www.cubrc.org/ontologies/KDD/Mid/EventOntology#Trial"/>
        <rdfs:comment>Definition: A Trial involving a judicial examination of a claim that a person actions have inflicted damages on another and should be responsible for a legal or equitable remedy. (derived from http://www.id.uscourts.gov/glossary.htm)</rdfs:comment>
    </owl:Class>
    


    <!-- http://www.cubrc.org/ontologies/KDD/Mid/EventOntology#LegalSystemAct -->

    <owl:Class rdf:about="http://www.cubrc.org/ontologies/KDD/Mid/EventOntology#LegalSystemAct">
        <rdfs:label>Legal System Act</rdfs:label>
        <rdfs:subClassOf rdf:resource="http://www.cubrc.org/ontologies/KDD/Mid/EventOntology#IntentionalAct"/>
        <rdfs:comment>Definition: An Intentional Act performed by an Agent that realizes their role within the context of a legal system of some jurisdiction. (derived from http://www.id.uscourts.gov/glossary.htm)</rdfs:comment>
    </owl:Class>
    


    <!-- http://www.cubrc.org/ontologies/KDD/Mid/EventOntology#LifeEvent -->

    <owl:Class rdf:about="http://www.cubrc.org/ontologies/KDD/Mid/EventOntology#LifeEvent">
        <rdfs:label rdf:datatype="&xsd;string">Life Event</rdfs:label>
        <rdfs:subClassOf rdf:resource="http://www.ifomis.org/bfo/1.1/span#FiatProcessPart"/>
        <rdfs:subClassOf>
            <owl:Restriction>
                <owl:onProperty rdf:resource="http://www.obofoundry.org/ro/ro.owl#part_of"/>
                <owl:someValuesFrom rdf:resource="http://www.cubrc.org/ontologies/KDD/Mid/EventOntology#BiographicalLife"/>
            </owl:Restriction>
        </rdfs:subClassOf>
        <rdfs:comment rdf:datatype="&xsd;string">A Fiat Process Part participated in by the agent of some Biographical Life.</rdfs:comment>
    </owl:Class>
    


    <!-- http://www.cubrc.org/ontologies/KDD/Mid/EventOntology#LossOfDependentContinuant -->

    <owl:Class rdf:about="http://www.cubrc.org/ontologies/KDD/Mid/EventOntology#LossOfDependentContinuant">
        <rdfs:label rdf:datatype="&xsd;string">Loss of dependent continuant</rdfs:label>
        <rdfs:subClassOf rdf:resource="http://www.cubrc.org/ontologies/KDD/Mid/EventOntology#State"/>
        <rdfs:comment rdf:datatype="&xsd;string">Definition: A State in which some Independent Continuant ceases to be the bearer of some Dependent Continuant.</rdfs:comment>
    </owl:Class>
    


    <!-- http://www.cubrc.org/ontologies/KDD/Mid/EventOntology#LossOfDisposition -->

    <owl:Class rdf:about="http://www.cubrc.org/ontologies/KDD/Mid/EventOntology#LossOfDisposition">
        <rdfs:label rdf:datatype="&xsd;string">Loss of disposition</rdfs:label>
        <rdfs:subClassOf rdf:resource="http://www.cubrc.org/ontologies/KDD/Mid/EventOntology#LossOfRealizableEntity"/>
        <rdfs:comment rdf:datatype="&xsd;string">Definition: A Loss of Specifically Dependent Continuant in which some Independent Continuant ceases to be the bearer of some Disposition.</rdfs:comment>
    </owl:Class>
    


    <!-- http://www.cubrc.org/ontologies/KDD/Mid/EventOntology#LossOfFunction -->

    <owl:Class rdf:about="http://www.cubrc.org/ontologies/KDD/Mid/EventOntology#LossOfFunction">
        <rdfs:label rdf:datatype="&xsd;string">Loss of function</rdfs:label>
        <rdfs:subClassOf rdf:resource="http://www.cubrc.org/ontologies/KDD/Mid/EventOntology#LossOfRealizableEntity"/>
        <rdfs:comment rdf:datatype="&xsd;string">Definition: A Loss of Specifically Dependent Continuant in which some Independent Continuant ceases to be the bearer of some Function.</rdfs:comment>
    </owl:Class>
    


    <!-- http://www.cubrc.org/ontologies/KDD/Mid/EventOntology#LossOfGenericallyDependentContinuant -->

    <owl:Class rdf:about="http://www.cubrc.org/ontologies/KDD/Mid/EventOntology#LossOfGenericallyDependentContinuant">
        <rdfs:label rdf:datatype="&xsd;string">Loss of generically dependent continuant</rdfs:label>
        <rdfs:subClassOf rdf:resource="http://www.cubrc.org/ontologies/KDD/Mid/EventOntology#LossOfDependentContinuant"/>
        <rdfs:comment rdf:datatype="&xsd;string">Definition: A Loss of Dependent Continuant in which some Independent Continuant ceases to be the bearer of some Generically Dependent Continuant.</rdfs:comment>
    </owl:Class>
    


    <!-- http://www.cubrc.org/ontologies/KDD/Mid/EventOntology#LossOfQuality -->

    <owl:Class rdf:about="http://www.cubrc.org/ontologies/KDD/Mid/EventOntology#LossOfQuality">
        <rdfs:label rdf:datatype="&xsd;string">Loss of quality</rdfs:label>
        <rdfs:subClassOf rdf:resource="http://www.cubrc.org/ontologies/KDD/Mid/EventOntology#LossOfSpecificallyDependentContinuant"/>
        <rdfs:comment rdf:datatype="&xsd;string">Definition: A Loss of Specifically Dependent Continuant in which some Independent Continuant ceases to be the bearer of some Quality.</rdfs:comment>
    </owl:Class>
    


    <!-- http://www.cubrc.org/ontologies/KDD/Mid/EventOntology#LossOfRealizableEntity -->

    <owl:Class rdf:about="http://www.cubrc.org/ontologies/KDD/Mid/EventOntology#LossOfRealizableEntity">
        <rdfs:label rdf:datatype="&xsd;string">Loss of realizable entity</rdfs:label>
        <rdfs:subClassOf rdf:resource="http://www.cubrc.org/ontologies/KDD/Mid/EventOntology#LossOfSpecificallyDependentContinuant"/>
        <rdfs:comment rdf:datatype="&xsd;string">Definition: A Loss of Specifically Dependent Continuant in which some Independent Continuant ceases to be the bearer of some Realizable Entity.</rdfs:comment>
    </owl:Class>
    


    <!-- http://www.cubrc.org/ontologies/KDD/Mid/EventOntology#LossOfRole -->

    <owl:Class rdf:about="http://www.cubrc.org/ontologies/KDD/Mid/EventOntology#LossOfRole">
        <rdfs:label rdf:datatype="&xsd;string">Loss of role</rdfs:label>
        <rdfs:subClassOf rdf:resource="http://www.cubrc.org/ontologies/KDD/Mid/EventOntology#LossOfRealizableEntity"/>
        <rdfs:comment rdf:datatype="&xsd;string">Definition: A Loss of Specifically Dependent Continuant in which some Independent Continuant ceases to be the bearer of some Role.</rdfs:comment>
    </owl:Class>
    


    <!-- http://www.cubrc.org/ontologies/KDD/Mid/EventOntology#LossOfSpecificallyDependentContinuant -->

    <owl:Class rdf:about="http://www.cubrc.org/ontologies/KDD/Mid/EventOntology#LossOfSpecificallyDependentContinuant">
        <rdfs:label rdf:datatype="&xsd;string">Loss of specifically dependent continuant</rdfs:label>
        <rdfs:subClassOf rdf:resource="http://www.cubrc.org/ontologies/KDD/Mid/EventOntology#LossOfDependentContinuant"/>
        <rdfs:comment rdf:datatype="&xsd;string">Definition: A Loss of Dependent Continuant in which some Independent Continuant ceases to be the bearer of some Specifically Dependent Continuant.</rdfs:comment>
    </owl:Class>
    


    <!-- http://www.cubrc.org/ontologies/KDD/Mid/EventOntology#Mailing -->

    <owl:Class rdf:about="http://www.cubrc.org/ontologies/KDD/Mid/EventOntology#Mailing">
        <rdfs:label rdf:datatype="&xsd;string">Mailing</rdfs:label>
        <rdfs:subClassOf rdf:resource="http://www.cubrc.org/ontologies/KDD/Mid/EventOntology#ActOfCommunicationByMedia"/>
        <rdfs:comment rdf:datatype="&xsd;string">Definition: An Act of Communication in which information and tangible objects, usually written documents, are delivered to destinations around the world. (derived from http://en.wikipedia.org/wiki/Mail)</rdfs:comment>
    </owl:Class>
    


    <!-- http://www.cubrc.org/ontologies/KDD/Mid/EventOntology#Marriage -->

    <owl:Class rdf:about="http://www.cubrc.org/ontologies/KDD/Mid/EventOntology#Marriage">
        <rdfs:label>Marriage</rdfs:label>
        <rdfs:subClassOf rdf:resource="http://www.cubrc.org/ontologies/KDD/Mid/EventOntology#LegalSystemAct"/>
        <rdfs:subClassOf>
            <owl:Restriction>
                <owl:onProperty rdf:resource="http://www.obofoundry.org/ro/ro.owl#preceded_by"/>
                <owl:someValuesFrom rdf:resource="http://www.cubrc.org/ontologies/KDD/Mid/EventOntology#ActOfMarrying"/>
            </owl:Restriction>
        </rdfs:subClassOf>
        <rdfs:comment rdf:datatype="&xsd;string">Definition: A Legal System Act between two people during which a kinship relationship exists between them (derived from http://en.wikipedia.org/wiki/Marriage).</rdfs:comment>
    </owl:Class>
    


    <!-- http://www.cubrc.org/ontologies/KDD/Mid/EventOntology#Mistrial -->

    <owl:Class rdf:about="http://www.cubrc.org/ontologies/KDD/Mid/EventOntology#Mistrial">
        <rdfs:label>Mistrial</rdfs:label>
        <rdfs:subClassOf rdf:resource="http://www.cubrc.org/ontologies/KDD/Mid/EventOntology#LegalSystemAct"/>
        <rdfs:comment>Definition: A Legal System Act that is an invalid Trial, caused by some fundamental error. (derived from http://www.id.uscourts.gov/glossary.htm)</rdfs:comment>
    </owl:Class>
    


    <!-- http://www.cubrc.org/ontologies/KDD/Mid/EventOntology#NaturalProcess -->

    <owl:Class rdf:about="http://www.cubrc.org/ontologies/KDD/Mid/EventOntology#NaturalProcess">
        <rdfs:label rdf:datatype="&xsd;string">Natural Process</rdfs:label>
        <rdfs:subClassOf rdf:resource="http://www.ifomis.org/bfo/1.1/span#Process"/>
        <rdfs:comment rdf:datatype="&xsd;string">A Process existing in or derived from nature; not made, caused by, or processed by humankind. [Derived from Concise Oxford English Dictionary, 11th Edition, 2008].</rdfs:comment>
    </owl:Class>
    


    <!-- http://www.cubrc.org/ontologies/KDD/Mid/EventOntology#PrivateNetworkTelephoneCall -->

    <owl:Class rdf:about="http://www.cubrc.org/ontologies/KDD/Mid/EventOntology#PrivateNetworkTelephoneCall">
        <rdfs:label rdf:datatype="&xsd;string">Private Network Telephone Call</rdfs:label>
        <rdfs:subClassOf rdf:resource="http://www.cubrc.org/ontologies/KDD/Mid/EventOntology#TelephoneCall"/>
        <rdfs:comment rdf:datatype="&xsd;string">Definition: A Telephone Call transmitted over a network where a closed group of telephones are connected primarily to each other and use a gateway to reach the outside world, usually used inside companies and call centers (a.k.a. private branch exchange (PBX)). (derived from http://en.wikipedia.org/wiki/Telephone_network)</rdfs:comment>
    </owl:Class>
    


    <!-- http://www.cubrc.org/ontologies/KDD/Mid/EventOntology#RadioBroadcast -->

    <owl:Class rdf:about="http://www.cubrc.org/ontologies/KDD/Mid/EventOntology#RadioBroadcast">
        <rdfs:label rdf:datatype="&xsd;string">Radio Broadcast</rdfs:label>
        <rdfs:subClassOf rdf:resource="http://www.cubrc.org/ontologies/KDD/Mid/EventOntology#ActOfCommunicationByMedia"/>
        <rdfs:comment rdf:datatype="&xsd;string">Definition: An Act of Communciation that is transmitted to an audience through a radio network. (derived from http://en.wikipedia.org/wiki/Radio_network)</rdfs:comment>
    </owl:Class>
    


    <!-- http://www.cubrc.org/ontologies/KDD/Mid/EventOntology#Riot -->

    <owl:Class rdf:about="http://www.cubrc.org/ontologies/KDD/Mid/EventOntology#Riot">
        <rdfs:label rdf:datatype="&xsd;string">Riot</rdfs:label>
        <rdfs:subClassOf rdf:resource="http://www.cubrc.org/ontologies/KDD/Mid/EventOntology#ActOfCivilDisorder"/>
        <rdfs:comment rdf:datatype="&xsd;string">Definition: An Act of Civil Disorder characterized often by disorganized groups lashing out in a sudden and intense rash of violence against authority, property or people. While individuals may attempt to lead or control a riot, riots are typically chaotic and exhibit herd behavior, and usually generated by civil unrest. (derived from http://en.wikipedia.org/wiki/Riot).</rdfs:comment>
    </owl:Class>
    


    <!-- http://www.cubrc.org/ontologies/KDD/Mid/EventOntology#SocialAct -->

    <owl:Class rdf:about="http://www.cubrc.org/ontologies/KDD/Mid/EventOntology#SocialAct">
        <rdfs:label>Social Act</rdfs:label>
        <rdfs:subClassOf rdf:resource="http://www.cubrc.org/ontologies/KDD/Mid/EventOntology#IntentionalAct"/>
        <rdfs:comment>Definition: An Intentional Act having an objective that affects, is performed by, or is performed on behalf of, a community or group of Persons (derived from http://en.wiktionary.org/wiki/commually)</rdfs:comment>
    </owl:Class>
    


    <!-- http://www.cubrc.org/ontologies/KDD/Mid/EventOntology#SocietalOrder -->

    <owl:Class rdf:about="http://www.cubrc.org/ontologies/KDD/Mid/EventOntology#SocietalOrder">
        <rdfs:label rdf:datatype="&xsd;string">Societal Order</rdfs:label>
        <rdfs:subClassOf rdf:resource="http://www.cubrc.org/ontologies/KDD/Mid/EventOntology#StaticStateOfDependentContinuant"/>
        <rdfs:comment rdf:datatype="&xsd;string">Definition: The established customary state of a Society (wordnet (order%1:26:00::))</rdfs:comment>
    </owl:Class>
    


    <!-- http://www.cubrc.org/ontologies/KDD/Mid/EventOntology#Sojourn -->

    <owl:Class rdf:about="http://www.cubrc.org/ontologies/KDD/Mid/EventOntology#Sojourn">
        <rdfs:label rdf:datatype="&xsd;string">Sojourn</rdfs:label>
        <rdfs:subClassOf rdf:resource="http://www.cubrc.org/ontologies/KDD/Mid/EventOntology#ActOfInhabitancy"/>
        <rdfs:comment rdf:datatype="&xsd;string">Definition: An Act of Inhabitancy in which a Person resides in a dwelling temporarily, often during stages of an Act Of Travel.</rdfs:comment>
    </owl:Class>
    


    <!-- http://www.cubrc.org/ontologies/KDD/Mid/EventOntology#State -->

    <owl:Class rdf:about="http://www.cubrc.org/ontologies/KDD/Mid/EventOntology#State">
        <rdfs:label rdf:datatype="&xsd;string">State</rdfs:label>
        <rdfs:subClassOf rdf:resource="http://www.ifomis.org/bfo/1.1/span#Process"/>
        <rdfs:comment rdf:datatype="&xsd;string">A Process of temporal change of Qualities, Dispositions, Functions, and Roles of an Entity.</rdfs:comment>
    </owl:Class>
    


    <!-- http://www.cubrc.org/ontologies/KDD/Mid/EventOntology#StaticStateOfDependentContinuant -->

    <owl:Class rdf:about="http://www.cubrc.org/ontologies/KDD/Mid/EventOntology#StaticStateOfDependentContinuant">
        <rdfs:label rdf:datatype="&xsd;string">Static State of Dependent Continuant</rdfs:label>
        <rdfs:subClassOf rdf:resource="http://www.cubrc.org/ontologies/KDD/Mid/EventOntology#State"/>
        <rdfs:comment rdf:datatype="&xsd;string">Definition: A State in which some Independent Continuant that bears some Dependent Continuant and remains unchanged during a Temporal Interval.</rdfs:comment>
    </owl:Class>
    


    <!-- http://www.cubrc.org/ontologies/KDD/Mid/EventOntology#StaticStateOfDisposition -->

    <owl:Class rdf:about="http://www.cubrc.org/ontologies/KDD/Mid/EventOntology#StaticStateOfDisposition">
        <rdfs:label rdf:datatype="&xsd;string">Static State of Disposition</rdfs:label>
        <rdfs:subClassOf rdf:resource="http://www.cubrc.org/ontologies/KDD/Mid/EventOntology#StaticStateOfRealizableEntity"/>
        <rdfs:comment rdf:datatype="&xsd;string">Definition: A Static State of Realizable Entity in which some Independent Continuant that bears some Disposition and remains unchanged during a Temporal Interval.</rdfs:comment>
    </owl:Class>
    


    <!-- http://www.cubrc.org/ontologies/KDD/Mid/EventOntology#StaticStateOfFunction -->

    <owl:Class rdf:about="http://www.cubrc.org/ontologies/KDD/Mid/EventOntology#StaticStateOfFunction">
        <rdfs:label rdf:datatype="&xsd;string">Static State of Function</rdfs:label>
        <rdfs:subClassOf rdf:resource="http://www.cubrc.org/ontologies/KDD/Mid/EventOntology#StaticStateOfRealizableEntity"/>
        <rdfs:comment rdf:datatype="&xsd;string">Definition: A Static State of Function in which some Independent Continuant that bears some Function and remains unchanged during a Temporal Interval.</rdfs:comment>
    </owl:Class>
    


    <!-- http://www.cubrc.org/ontologies/KDD/Mid/EventOntology#StaticStateOfGenericallyDependentContinuant -->

    <owl:Class rdf:about="http://www.cubrc.org/ontologies/KDD/Mid/EventOntology#StaticStateOfGenericallyDependentContinuant">
        <rdfs:label rdf:datatype="&xsd;string">Static State of Generically Dependent Continuant</rdfs:label>
        <rdfs:subClassOf rdf:resource="http://www.cubrc.org/ontologies/KDD/Mid/EventOntology#StaticStateOfDependentContinuant"/>
        <rdfs:comment rdf:datatype="&xsd;string">Definition: A Static State of Dependent Continuant in which some Independent Continuant that bears some Generically Dependent Continuant and remains unchanged during a Temporal Interval.</rdfs:comment>
    </owl:Class>
    


    <!-- http://www.cubrc.org/ontologies/KDD/Mid/EventOntology#StaticStateOfQuality -->

    <owl:Class rdf:about="http://www.cubrc.org/ontologies/KDD/Mid/EventOntology#StaticStateOfQuality">
        <rdfs:label rdf:datatype="&xsd;string">Gain of</rdfs:label>
        <rdfs:subClassOf rdf:resource="http://www.cubrc.org/ontologies/KDD/Mid/EventOntology#StaticStateOfSpecificallyDependentContinuant"/>
        <rdfs:comment rdf:datatype="&xsd;string">Definition: A Static State of Specifically Dependent Continuant in which some Independent Continuant that bears some Quality and remains unchanged during a Temporal Interval.</rdfs:comment>
    </owl:Class>
    


    <!-- http://www.cubrc.org/ontologies/KDD/Mid/EventOntology#StaticStateOfRealizableEntity -->

    <owl:Class rdf:about="http://www.cubrc.org/ontologies/KDD/Mid/EventOntology#StaticStateOfRealizableEntity">
        <rdfs:label rdf:datatype="&xsd;string">Static State of Realizable Entity</rdfs:label>
        <rdfs:subClassOf rdf:resource="http://www.cubrc.org/ontologies/KDD/Mid/EventOntology#StaticStateOfSpecificallyDependentContinuant"/>
        <rdfs:comment rdf:datatype="&xsd;string">Definition: A Static State of Specifically Dependent Continuant in which some Independent Continuant that bears some Realizable Entity and remains unchanged during a Temporal Interval.</rdfs:comment>
    </owl:Class>
    


    <!-- http://www.cubrc.org/ontologies/KDD/Mid/EventOntology#StaticStateOfRole -->

    <owl:Class rdf:about="http://www.cubrc.org/ontologies/KDD/Mid/EventOntology#StaticStateOfRole">
        <rdfs:label rdf:datatype="&xsd;string">Static State of Role</rdfs:label>
        <rdfs:subClassOf rdf:resource="http://www.cubrc.org/ontologies/KDD/Mid/EventOntology#StaticStateOfRealizableEntity"/>
        <rdfs:comment rdf:datatype="&xsd;string">Definition: A Static State of Realizable Entity in which some Independent Continuant that bears some Role and remains unchanged during a Temporal Interval.</rdfs:comment>
    </owl:Class>
    


    <!-- http://www.cubrc.org/ontologies/KDD/Mid/EventOntology#StaticStateOfSpecificallyDependentContinuant -->

    <owl:Class rdf:about="http://www.cubrc.org/ontologies/KDD/Mid/EventOntology#StaticStateOfSpecificallyDependentContinuant">
        <rdfs:label rdf:datatype="&xsd;string">Static State of Specifically Dependent Continuant</rdfs:label>
        <rdfs:subClassOf rdf:resource="http://www.cubrc.org/ontologies/KDD/Mid/EventOntology#StaticStateOfDependentContinuant"/>
        <rdfs:comment rdf:datatype="&xsd;string">Definition: A Static State of Dependent Continuant in which some Independent Continuant that bears some Specifically Dependent Continuant and remains unchanged during a Temporal Interval.</rdfs:comment>
    </owl:Class>
    


    <!-- http://www.cubrc.org/ontologies/KDD/Mid/EventOntology#TacticalRole -->

    <owl:Class rdf:about="http://www.cubrc.org/ontologies/KDD/Mid/EventOntology#TacticalRole">
        <rdfs:label rdf:datatype="&xsd;string">Tactical Role</rdfs:label>
        <rdfs:subClassOf rdf:resource="http://www.ifomis.org/bfo/1.1/snap#Role"/>
        <rdfs:comment rdf:datatype="&xsd;string">Definition: A Role of some Entity by virtue of its participation in some Intentional Act or description in some Plan.</rdfs:comment>
    </owl:Class>
    


    <!-- http://www.cubrc.org/ontologies/KDD/Mid/EventOntology#Target -->

    <owl:Class rdf:about="http://www.cubrc.org/ontologies/KDD/Mid/EventOntology#Target">
        <rdfs:label rdf:datatype="&xsd;string">Target</rdfs:label>
        <rdfs:subClassOf rdf:resource="http://www.ifomis.org/bfo/1.1#Entity"/>
        <rdfs:comment rdf:datatype="&xsd;string">Definition: An Entity that has the role of Target in virtue of its being involved in the Objective of some Intentional Act or in the described outcome of some Plan.</rdfs:comment>
    </owl:Class>
    


    <!-- http://www.cubrc.org/ontologies/KDD/Mid/EventOntology#TargetRole -->

    <owl:Class rdf:about="http://www.cubrc.org/ontologies/KDD/Mid/EventOntology#TargetRole">
        <rdfs:label rdf:datatype="&xsd;string">Target Role</rdfs:label>
        <rdfs:subClassOf rdf:resource="http://www.cubrc.org/ontologies/KDD/Mid/EventOntology#TacticalRole"/>
        <rdfs:comment rdf:datatype="&xsd;string">Definition: A Tactical Role that is the role of some Entity by virtue of some Intentional Act having an objective or Plan describing some outcome that involves that Entity, typically the outcome is to reduce or destroy the Functions of the Entity.</rdfs:comment>
    </owl:Class>
    


    <!-- http://www.cubrc.org/ontologies/KDD/Mid/EventOntology#TelephoneCall -->

    <owl:Class rdf:about="http://www.cubrc.org/ontologies/KDD/Mid/EventOntology#TelephoneCall">
        <rdfs:label rdf:datatype="&xsd;string">Telephone Call</rdfs:label>
        <rdfs:subClassOf rdf:resource="http://www.cubrc.org/ontologies/KDD/Mid/EventOntology#ActOfCommunicationByMedia"/>
        <rdfs:comment rdf:datatype="&xsd;string">Definition: An Act of Communciation transmitted over a telephone network to two or more Persons. (derived from http://en.wikipedia.org/wiki/Telephone_network)</rdfs:comment>
    </owl:Class>
    


    <!-- http://www.cubrc.org/ontologies/KDD/Mid/EventOntology#TelevisionBroadcast -->

    <owl:Class rdf:about="http://www.cubrc.org/ontologies/KDD/Mid/EventOntology#TelevisionBroadcast">
        <rdfs:label rdf:datatype="&xsd;string">Television Broadcast</rdfs:label>
        <rdfs:subClassOf rdf:resource="http://www.cubrc.org/ontologies/KDD/Mid/EventOntology#ActOfCommunicationByMedia"/>
        <rdfs:comment rdf:datatype="&xsd;string">Definition: An Act of Communciation that is transmitted to an audience through a television network. (derived from http://en.wikipedia.org/wiki/Television_network)</rdfs:comment>
    </owl:Class>
    


    <!-- http://www.cubrc.org/ontologies/KDD/Mid/EventOntology#TextMessaging -->

    <owl:Class rdf:about="http://www.cubrc.org/ontologies/KDD/Mid/EventOntology#TextMessaging">
        <rdfs:label rdf:datatype="&xsd;string">Text Messaging</rdfs:label>
        <rdfs:subClassOf rdf:resource="http://www.cubrc.org/ontologies/KDD/Mid/EventOntology#ActOfCommunicationByMedia"/>
        <rdfs:comment rdf:datatype="&xsd;string">Definition: An Act of Communication involving the exchange of brief written messages between fixed-line phone or mobile phone and fixed or portable devices over a network. (derived from http://en.wikipedia.org/wiki/Text_messaging)</rdfs:comment>
    </owl:Class>
    


    <!-- http://www.cubrc.org/ontologies/KDD/Mid/EventOntology#Trial -->

    <owl:Class rdf:about="http://www.cubrc.org/ontologies/KDD/Mid/EventOntology#Trial">
        <rdfs:label>Trial</rdfs:label>
        <rdfs:subClassOf rdf:resource="http://www.cubrc.org/ontologies/KDD/Mid/EventOntology#LegalSystemAct"/>
        <rdfs:comment>Definition: A Legal System Act involving a judicial examination of issues between parties to an action (derived from http://www.id.uscourts.gov/glossary.htm)</rdfs:comment>
    </owl:Class>
    


    <!-- http://www.cubrc.org/ontologies/KDD/Mid/EventOntology#UnintentionalAct -->

    <owl:Class rdf:about="http://www.cubrc.org/ontologies/KDD/Mid/EventOntology#UnintentionalAct">
        <rdfs:label rdf:datatype="&xsd;string">Unintentional Act</rdfs:label>
        <rdfs:subClassOf rdf:resource="http://www.cubrc.org/ontologies/KDD/Mid/EventOntology#Act"/>
        <rdfs:comment rdf:datatype="&xsd;string">An Act in which at least one Agent plays a causative role and which is not prescribed by some Objective held by any of the Agents.</rdfs:comment>
    </owl:Class>
    


    <!-- http://www.cubrc.org/ontologies/KDD/Mid/EventOntology#Webcast -->

    <owl:Class rdf:about="http://www.cubrc.org/ontologies/KDD/Mid/EventOntology#Webcast">
        <rdfs:label rdf:datatype="&xsd;string">Webcast</rdfs:label>
        <rdfs:subClassOf rdf:resource="http://www.cubrc.org/ontologies/KDD/Mid/EventOntology#ActOfCommunicationByMedia"/>
        <rdfs:comment rdf:datatype="&xsd;string">Definition: An Act of Communciation transmitted to an audience over the Internet using streaming media technology to distribute a single content source that may be distributed live or on demand. Essentially, webcasting is “broadcasting” over the Internet.. (derived from http://en.wikipedia.org/wiki/Webcast)</rdfs:comment>
    </owl:Class>
    


    <!-- http://www.cubrc.org/ontologies/KDD/Mid/EventOntology#Wedding -->

    <owl:Class rdf:about="http://www.cubrc.org/ontologies/KDD/Mid/EventOntology#Wedding">
        <rdfs:label>Wedding</rdfs:label>
        <rdfs:subClassOf rdf:resource="http://www.cubrc.org/ontologies/KDD/Mid/EventOntology#ActOfCeremony"/>
        <rdfs:subClassOf>
            <owl:Restriction>
                <owl:onProperty rdf:resource="http://www.obofoundry.org/ro/ro.owl#has_part"/>
                <owl:someValuesFrom rdf:resource="http://www.cubrc.org/ontologies/KDD/Mid/EventOntology#ActOfMarrying"/>
            </owl:Restriction>
        </rdfs:subClassOf>
        <rdfs:comment>Definition: An Act Of Ceremony in which two Persons are united in Marriage or a similar institution. (derived from http://en.wikipedia.org/wiki/Wedding)</rdfs:comment>
    </owl:Class>
    


    <!-- http://www.cubrc.org/ontologies/KDD/Mid/EventOntology#WirelessNetworkTelephoneCall -->

    <owl:Class rdf:about="http://www.cubrc.org/ontologies/KDD/Mid/EventOntology#WirelessNetworkTelephoneCall">
        <rdfs:label rdf:datatype="&xsd;string">Wireless Network Telephone Call</rdfs:label>
        <rdfs:subClassOf rdf:resource="http://www.cubrc.org/ontologies/KDD/Mid/EventOntology#TelephoneCall"/>
        <rdfs:comment rdf:datatype="&xsd;string">Definition: A Telephone Call transmitted over a network where the telephones are mobile and can move anywhere within the coverage area. (derived from http://en.wikipedia.org/wiki/Telephone_network)</rdfs:comment>
    </owl:Class>
    


    <!-- http://www.cubrc.org/ontologies/KDD/Mid/EventOntology#Wounding -->

    <owl:Class rdf:about="http://www.cubrc.org/ontologies/KDD/Mid/EventOntology#Wounding">
        <rdfs:label rdf:datatype="&xsd;string">Wounding</rdfs:label>
        <rdfs:subClassOf rdf:resource="http://www.cubrc.org/ontologies/KDD/Mid/EventOntology#Damage"/>
        <rdfs:comment rdf:datatype="&xsd;string">A type of Damage in which some Agent suffers an injury from some external force.</rdfs:comment>
    </owl:Class>
</rdf:RDF>



<!-- Generated by the OWL API (version 3.4.2) http://owlapi.sourceforge.net -->

